midend/ValueDomainSSA.v
@@ -14,6 +14,34 @@ Require Import FunInd.
 Require Import Zwf Coqlib Maps Zbits Integers Floats Lattice.
 Require Import Compopts AST.
 Require Import Values Memory Globalenvs Builtins Events.
+Require Import Registers SSA.
+
+(** The abstract domains for value analysis *)
+
+Inductive block_class : Type :=
+  | BCinvalid
+  | BCglob (id: ident)
+  | BCstack
+  | BCother.
+
+Definition block_class_eq: forall (x y: block_class), {x=y} + {x<>y}.
+Proof. decide equality. apply peq. Defined.
+
+Record block_classification : Type := BC {
+  bc_img :> block -> block_class;
+  bc_stack: forall b1 b2, bc_img b1 = BCstack -> bc_img b2 = BCstack -> b1 = b2;
+  bc_glob: forall b1 b2 id, bc_img b1 = BCglob id -> bc_img b2 = BCglob id -> b1 = b2
+}.
+
+Definition bc_below (bc: block_classification) (bound: block) : Prop :=
+  forall b, bc b <> BCinvalid -> Plt b bound.
+
+Lemma bc_below_invalid:
+  forall b bc bound, ~Plt b bound -> bc_below bc bound -> bc b = BCinvalid.
+Proof.
+  intros. destruct (block_class_eq (bc b) BCinvalid); auto.
+  elim H. apply H0; auto.
+Qed.
 
 Hint Extern 2 (_ = _) => congruence : va.
 Hint Extern 2 (_ <> _) => congruence : va.
@@ -22,27 +50,506 @@ Hint Extern 2 (_ <= _) => xomega : va.
 Hint Extern 2 (_ > _) => xomega : va.
 Hint Extern 2 (_ >= _) => xomega : va.
 
-(** The abstract domains for scalar value analysis (no alias analysis) *)
-
-Require Import ValueDomain.
-
 Section MATCH.
+
+Variable bc: block_classification.
+
+(** * Abstracting the result of conditions (type [option bool]) *)
+
+Inductive abool :=
+  | Bnone               (**r always [None] (undefined) *)
+  | Just (b: bool)      (**r always [Some b] (defined and known to be [b]) *)
+  | Maybe (b: bool)     (**r either [None] or [Some b] (known to be [b] if defined) *)
+  | Btop.               (**r unknown, all results are possible *)
+
+Inductive cmatch: option bool -> abool -> Prop :=
+  | cmatch_none: cmatch None Bnone
+  | cmatch_just: forall b, cmatch (Some b) (Just b)
+  | cmatch_maybe_none: forall b, cmatch None (Maybe b)
+  | cmatch_maybe_some: forall b, cmatch (Some b) (Maybe b)
+  | cmatch_top: forall ob, cmatch ob Btop.
+
+Hint Constructors cmatch : va.
+
+Definition club (x y: abool) : abool :=
+  match x, y with
+  | Bnone, Bnone => Bnone
+  | Bnone, (Just b | Maybe b) => Maybe b
+  | (Just b | Maybe b), Bnone => Maybe b
+  | Just b1, Just b2 => if eqb b1 b2 then x else Btop
+  | Maybe b1, Maybe b2 => if eqb b1 b2 then x else Btop
+  | Maybe b1, Just b2 => if eqb b1 b2 then x else Btop
+  | Just b1, Maybe b2 => if eqb b1 b2 then y else Btop
+  | _, _ => Btop
+  end.
+
+Lemma cmatch_lub_l:
+  forall ob x y, cmatch ob x -> cmatch ob (club x y).
+Proof.
+  intros. unfold club; inv H; destruct y; try constructor;
+  destruct (eqb b b0) eqn:EQ; try constructor.
+  replace b0 with b by (apply eqb_prop; auto). constructor.
+Qed.
+
+Lemma cmatch_lub_r:
+  forall ob x y, cmatch ob y -> cmatch ob (club x y).
+Proof.
+  intros. unfold club; inv H; destruct x; try constructor;
+  destruct (eqb b0 b) eqn:EQ; try constructor.
+  replace b with b0 by (apply eqb_prop; auto). constructor.
+  replace b with b0 by (apply eqb_prop; auto). constructor.
+  replace b with b0 by (apply eqb_prop; auto). constructor.
+Qed.
+
+Definition cnot (x: abool) : abool :=
+  match x with
+  | Just b => Just (negb b)
+  | Maybe b => Maybe (negb b)
+  | _ => x
+  end.
+
+Lemma cnot_sound:
+  forall ob x, cmatch ob x -> cmatch (option_map negb ob) (cnot x).
+Proof.
+  destruct 1; constructor.
+Qed.
+
+(** * Abstracting pointers *)
+
+Inductive aptr : Type :=
+  | Pbot                         (**r bottom (empty set of pointers) *)
+  | Gl (id: ident) (ofs: ptrofs) (**r pointer into the block for global variable [id] at offset [ofs] *)
+  | Glo (id: ident)              (**r pointer anywhere into the block for global [id] *)
+  | Glob                         (**r pointer into any global variable *)
+  | Stk (ofs: ptrofs)            (**r pointer into the current stack frame at offset [ofs] *)
+  | Stack                        (**r pointer anywhere into the current stack frame *)
+  | Nonstack                     (**r pointer anywhere but into the current stack frame *)
+  | Ptop.                        (**r any valid pointer *)
+
+Definition eq_aptr: forall (p1 p2: aptr), {p1=p2} + {p1<>p2}.
+Proof.
+  intros. generalize ident_eq, Ptrofs.eq_dec; intros. decide equality.
+Defined.
+
+Inductive pmatch (b: block) (ofs: ptrofs): aptr -> Prop :=
+  | pmatch_gl: forall id,
+      bc b = BCglob id ->
+      pmatch b ofs (Gl id ofs)
+  | pmatch_glo: forall id,
+      bc b = BCglob id ->
+      pmatch b ofs (Glo id)
+  | pmatch_glob: forall id,
+      bc b = BCglob id ->
+      pmatch b ofs Glob
+  | pmatch_stk:
+      bc b = BCstack ->
+      pmatch b ofs (Stk ofs)
+  | pmatch_stack:
+      bc b = BCstack ->
+      pmatch b ofs Stack
+  | pmatch_nonstack:
+      bc b <> BCstack -> bc b <> BCinvalid ->
+      pmatch b ofs Nonstack
+  | pmatch_top:
+      bc b <> BCinvalid ->
+      pmatch b ofs Ptop.
+
+Hint Constructors pmatch: va.
+
+Inductive pge: aptr -> aptr -> Prop :=
+  | pge_top: forall p, pge Ptop p
+  | pge_bot: forall p, pge p Pbot
+  | pge_refl: forall p, pge p p
+  | pge_glo_gl: forall id ofs, pge (Glo id) (Gl id ofs)
+  | pge_glob_gl: forall id ofs, pge Glob (Gl id ofs)
+  | pge_glob_glo: forall id, pge Glob (Glo id)
+  | pge_ns_gl: forall id ofs, pge Nonstack (Gl id ofs)
+  | pge_ns_glo: forall id, pge Nonstack (Glo id)
+  | pge_ns_glob: pge Nonstack Glob
+  | pge_stack_stk: forall ofs, pge Stack (Stk ofs).
+
+Hint Constructors pge: va.
+
+Lemma pge_trans:
+  forall p q, pge p q -> forall r, pge q r -> pge p r.
+Proof.
+  induction 1; intros r PM; inv PM; auto with va.
+Qed.
+
+Lemma pmatch_ge:
+  forall b ofs p q, pge p q -> pmatch b ofs q -> pmatch b ofs p.
+Proof.
+  induction 1; intros PM; inv PM; eauto with va.
+Qed.
+
+Lemma pmatch_top': forall b ofs p, pmatch b ofs p -> pmatch b ofs Ptop.
+Proof.
+  intros. apply pmatch_ge with p; auto with va.
+Qed.
+
+Definition plub (p q: aptr) : aptr :=
+  match p, q with
+  | Pbot, _ => q
+  | _, Pbot => p
+  | Gl id1 ofs1, Gl id2 ofs2 =>
+      if ident_eq id1 id2 then if Ptrofs.eq_dec ofs1 ofs2 then p else Glo id1 else Glob
+  | Gl id1 ofs1, Glo id2 =>
+      if ident_eq id1 id2 then q else Glob
+  | Glo id1, Gl id2 ofs2 =>
+      if ident_eq id1 id2 then p else Glob
+  | Glo id1, Glo id2 =>
+      if ident_eq id1 id2 then p else Glob
+  | (Gl _ _ | Glo _ | Glob), Glob => Glob
+  | Glob, (Gl _ _ | Glo _) => Glob
+  | (Gl _ _ | Glo _ | Glob | Nonstack), Nonstack =>
+      Nonstack
+  | Nonstack, (Gl _ _ | Glo _ | Glob) =>
+      Nonstack
+  | Stk ofs1, Stk ofs2 =>
+      if Ptrofs.eq_dec ofs1 ofs2 then p else Stack
+  | (Stk _ | Stack), Stack =>
+      Stack
+  | Stack, Stk _ =>
+      Stack
+  | _, _ => Ptop
+  end.
+
+Lemma plub_comm:
+  forall p q, plub p q = plub q p.
+Proof.
+  intros; unfold plub; destruct p; destruct q; auto.
+  destruct (ident_eq id id0). subst id0.
+  rewrite dec_eq_true.
+  destruct (Ptrofs.eq_dec ofs ofs0). subst ofs0. rewrite dec_eq_true. auto.
+  rewrite dec_eq_false by auto. auto.
+  rewrite dec_eq_false by auto. auto.
+  destruct (ident_eq id id0). subst id0.
+  rewrite dec_eq_true; auto.
+  rewrite dec_eq_false; auto.
+  destruct (ident_eq id id0). subst id0.
+  rewrite dec_eq_true; auto.
+  rewrite dec_eq_false; auto.
+  destruct (ident_eq id id0). subst id0.
+  rewrite dec_eq_true; auto.
+  rewrite dec_eq_false; auto.
+  destruct (Ptrofs.eq_dec ofs ofs0). subst ofs0. rewrite dec_eq_true; auto.
+  rewrite dec_eq_false; auto.
+Qed.
+
+Lemma pge_lub_l:
+  forall p q, pge (plub p q) p.
+Proof.
+  unfold plub; destruct p, q; auto with va.
+- destruct (ident_eq id id0).
+  destruct (Ptrofs.eq_dec ofs ofs0); subst; constructor.
+  constructor.
+- destruct (ident_eq id id0); subst; constructor.
+- destruct (ident_eq id id0); subst; constructor.
+- destruct (ident_eq id id0); subst; constructor.
+- destruct (Ptrofs.eq_dec ofs ofs0); subst; constructor.
+Qed.
+
+Lemma pge_lub_r:
+  forall p q, pge (plub p q) q.
+Proof.
+  intros. rewrite plub_comm. apply pge_lub_l.
+Qed.
+
+Lemma pmatch_lub_l:
+  forall b ofs p q, pmatch b ofs p -> pmatch b ofs (plub p q).
+Proof.
+  intros. eapply pmatch_ge; eauto. apply pge_lub_l.
+Qed.
+
+Lemma pmatch_lub_r:
+  forall b ofs p q, pmatch b ofs q -> pmatch b ofs (plub p q).
+Proof.
+  intros. eapply pmatch_ge; eauto. apply pge_lub_r.
+Qed.
+
+Lemma plub_least:
+  forall r p q, pge r p -> pge r q -> pge r (plub p q).
+Proof.
+  intros. inv H; inv H0; simpl; try constructor.
+- destruct p; constructor.
+- unfold plub; destruct q; repeat rewrite dec_eq_true; constructor.
+- rewrite dec_eq_true; constructor.
+- rewrite dec_eq_true; constructor.
+- rewrite dec_eq_true. destruct (Ptrofs.eq_dec ofs ofs0); constructor.
+- destruct (ident_eq id id0). destruct (Ptrofs.eq_dec ofs ofs0); constructor. constructor.
+- destruct (ident_eq id id0); constructor.
+- destruct (ident_eq id id0); constructor.
+- destruct (ident_eq id id0); constructor.
+- destruct (ident_eq id id0). destruct (Ptrofs.eq_dec ofs ofs0); constructor. constructor.
+- destruct (ident_eq id id0); constructor.
+- destruct (ident_eq id id0); constructor.
+- destruct (ident_eq id id0); constructor.
+- destruct (Ptrofs.eq_dec ofs ofs0); constructor.
+Qed.
+
+Definition pincl (p q: aptr) : bool :=
+  match p, q with
+  | Pbot, _ => true
+  | Gl id1 ofs1, Gl id2 ofs2 => peq id1 id2 && Ptrofs.eq_dec ofs1 ofs2
+  | Gl id1 ofs1, Glo id2 => peq id1 id2
+  | Glo id1, Glo id2 => peq id1 id2
+  | (Gl _ _ | Glo _ | Glob), Glob => true
+  | (Gl _ _ | Glo _ | Glob | Nonstack), Nonstack => true
+  | Stk ofs1, Stk ofs2 => Ptrofs.eq_dec ofs1 ofs2
+  | Stk ofs1, Stack => true
+  | Stack, Stack => true
+  | _, Ptop => true
+  | _, _ => false
+  end.
+
+Lemma pincl_ge: forall p q, pincl p q = true -> pge q p.
+Proof.
+  unfold pincl; destruct p, q; intros; try discriminate; auto with va;
+  InvBooleans; subst; auto with va.
+Qed.
+
+Lemma pincl_ge_2: forall p q, pge p q -> pincl q p = true.
+Proof.
+  destruct 1; simpl; auto.
+- destruct p; auto.
+- destruct p; simpl; auto; rewrite ! proj_sumbool_is_true; auto.
+- rewrite ! proj_sumbool_is_true; auto.
+Qed.
+
+Lemma pincl_sound:
+  forall b ofs p q,
+  pincl p q = true -> pmatch b ofs p -> pmatch b ofs q.
+Proof.
+  intros. eapply pmatch_ge; eauto. apply pincl_ge; auto.
+Qed.
+
+Definition padd (p: aptr) (n: ptrofs) : aptr :=
+  match p with
+  | Gl id ofs => Gl id (Ptrofs.add ofs n)
+  | Stk ofs => Stk (Ptrofs.add ofs n)
+  | _ => p
+  end.
+
+Lemma padd_sound:
+  forall b ofs p delta,
+  pmatch b ofs p ->
+  pmatch b (Ptrofs.add ofs delta) (padd p delta).
+Proof.
+  intros. inv H; simpl padd; eauto with va.
+Qed.
+
+Definition psub (p: aptr) (n: ptrofs) : aptr :=
+  match p with
+  | Gl id ofs => Gl id (Ptrofs.sub ofs n)
+  | Stk ofs => Stk (Ptrofs.sub ofs n)
+  | _ => p
+  end.
+
+Lemma psub_sound:
+  forall b ofs p delta,
+  pmatch b ofs p ->
+  pmatch b (Ptrofs.sub ofs delta) (psub p delta).
+Proof.
+  intros. inv H; simpl psub; eauto with va.
+Qed.
+
+Definition poffset (p: aptr) : aptr :=
+  match p with
+  | Gl id ofs => Glo id
+  | Stk ofs => Stack
+  | _ => p
+  end.
+
+Lemma poffset_sound:
+  forall b ofs1 ofs2 p,
+  pmatch b ofs1 p ->
+  pmatch b ofs2 (poffset p).
+Proof.
+  intros. inv H; simpl poffset; eauto with va.
+Qed.
+
+Definition cmp_different_blocks (c: comparison) : abool :=
+  match c with
+  | Ceq => Maybe false
+  | Cne => Maybe true
+  | _   => Bnone
+  end.
+
+Lemma cmp_different_blocks_none:
+  forall c, cmatch None (cmp_different_blocks c).
+Proof.
+  intros; destruct c; constructor.
+Qed.
+
+Lemma cmp_different_blocks_sound:
+  forall c, cmatch (Val.cmp_different_blocks c) (cmp_different_blocks c).
+Proof.
+  intros; destruct c; constructor.
+Qed.
+
+Definition pcmp (c: comparison) (p1 p2: aptr) : abool :=
+  match p1, p2 with
+  | Pbot, _ | _, Pbot => Bnone
+  | Gl id1 ofs1, Gl id2 ofs2 =>
+      if peq id1 id2 then Maybe (Ptrofs.cmpu c ofs1 ofs2)
+      else cmp_different_blocks c
+  | Gl id1 ofs1, Glo id2 =>
+      if peq id1 id2 then Btop else cmp_different_blocks c
+  | Glo id1, Gl id2 ofs2 =>
+      if peq id1 id2 then Btop else cmp_different_blocks c
+  | Glo id1, Glo id2 =>
+      if peq id1 id2 then Btop else cmp_different_blocks c
+  | Stk ofs1, Stk ofs2 => Maybe (Ptrofs.cmpu c ofs1 ofs2)
+  | (Gl _ _ | Glo _ | Glob | Nonstack), (Stk _ | Stack) => cmp_different_blocks c
+  | (Stk _ | Stack), (Gl _ _ | Glo _ | Glob | Nonstack) => cmp_different_blocks c
+  | _, _ => Btop
+  end.
+
+Lemma pcmp_sound:
+  forall valid c b1 ofs1 p1 b2 ofs2 p2,
+  pmatch b1 ofs1 p1 -> pmatch b2 ofs2 p2 ->
+  cmatch (Val.cmpu_bool valid c (Vptr b1 ofs1) (Vptr b2 ofs2)) (pcmp c p1 p2).
+Proof.
+  intros.
+  assert (DIFF: b1 <> b2 ->
+            cmatch (Val.cmpu_bool valid c (Vptr b1 ofs1) (Vptr b2 ofs2))
+                   (cmp_different_blocks c)).
+  {
+    intros. simpl. rewrite dec_eq_false by assumption.
+    destruct Archi.ptr64.
+    apply cmp_different_blocks_none.
+    destruct (valid b1 (Ptrofs.unsigned ofs1) && valid b2 (Ptrofs.unsigned ofs2)); simpl.
+    apply cmp_different_blocks_sound.
+    apply cmp_different_blocks_none.
+  }
+  assert (SAME: b1 = b2 ->
+            cmatch (Val.cmpu_bool valid c (Vptr b1 ofs1) (Vptr b2 ofs2))
+                   (Maybe (Ptrofs.cmpu c ofs1 ofs2))).
+  {
+    intros. subst b2. simpl. destruct Archi.ptr64.
+    constructor.
+    rewrite dec_eq_true.
+    destruct ((valid b1 (Ptrofs.unsigned ofs1) || valid b1 (Ptrofs.unsigned ofs1 - 1)) &&
+         (valid b1 (Ptrofs.unsigned ofs2) || valid b1 (Ptrofs.unsigned ofs2 - 1))); simpl.
+    constructor.
+    constructor.
+  }
+  unfold pcmp; inv H; inv H0; (apply cmatch_top || (apply DIFF; congruence) || idtac).
+  - destruct (peq id id0). subst id0. apply SAME. eapply bc_glob; eauto.
+    auto with va.
+  - destruct (peq id id0); auto with va.
+  - destruct (peq id id0); auto with va.
+  - destruct (peq id id0); auto with va.
+  - apply SAME. eapply bc_stack; eauto.
+Qed.
+
+Lemma pcmp_sound_64:
+  forall valid c b1 ofs1 p1 b2 ofs2 p2,
+  pmatch b1 ofs1 p1 -> pmatch b2 ofs2 p2 ->
+  cmatch (Val.cmplu_bool valid c (Vptr b1 ofs1) (Vptr b2 ofs2)) (pcmp c p1 p2).
+Proof.
+  intros.
+  assert (DIFF: b1 <> b2 ->
+            cmatch (Val.cmplu_bool valid c (Vptr b1 ofs1) (Vptr b2 ofs2))
+                   (cmp_different_blocks c)).
+  {
+    intros. simpl. rewrite dec_eq_false by assumption.
+    destruct Archi.ptr64; simpl.
+    destruct (valid b1 (Ptrofs.unsigned ofs1) && valid b2 (Ptrofs.unsigned ofs2)); simpl.
+    apply cmp_different_blocks_sound.
+    apply cmp_different_blocks_none.
+    apply cmp_different_blocks_none.
+  }
+  assert (SAME: b1 = b2 ->
+            cmatch (Val.cmplu_bool valid c (Vptr b1 ofs1) (Vptr b2 ofs2))
+                   (Maybe (Ptrofs.cmpu c ofs1 ofs2))).
+  {
+    intros. subst b2. simpl. destruct Archi.ptr64.
+    rewrite dec_eq_true.
+    destruct ((valid b1 (Ptrofs.unsigned ofs1) || valid b1 (Ptrofs.unsigned ofs1 - 1)) &&
+         (valid b1 (Ptrofs.unsigned ofs2) || valid b1 (Ptrofs.unsigned ofs2 - 1))); simpl.
+    constructor.
+    constructor.
+    constructor.
+  }
+  unfold pcmp; inv H; inv H0; (apply cmatch_top || (apply DIFF; congruence) || idtac).
+  - destruct (peq id id0). subst id0. apply SAME. eapply bc_glob; eauto.
+    auto with va.
+  - destruct (peq id id0); auto with va.
+  - destruct (peq id id0); auto with va.
+  - destruct (peq id id0); auto with va.
+  - apply SAME. eapply bc_stack; eauto.
+Qed.
+
+Lemma pcmp_none:
+  forall c p1 p2, cmatch None (pcmp c p1 p2).
+Proof.
+  intros.
+  unfold pcmp; destruct p1; try constructor; destruct p2;
+  try (destruct (peq id id0));  try constructor; try (apply cmp_different_blocks_none).
+Qed.
+
+Definition pdisjoint (p1: aptr) (sz1: Z) (p2: aptr) (sz2: Z) : bool :=
+  match p1, p2 with
+  | Pbot, _ => true
+  | _, Pbot => true
+  | Gl id1 ofs1, Gl id2 ofs2 =>
+      if peq id1 id2
+      then zle (Ptrofs.unsigned ofs1 + sz1) (Ptrofs.unsigned ofs2)
+           || zle (Ptrofs.unsigned ofs2 + sz2) (Ptrofs.unsigned ofs1)
+      else true
+  | Gl id1 ofs1, Glo id2 => negb(peq id1 id2)
+  | Glo id1, Gl id2 ofs2 => negb(peq id1 id2)
+  | Glo id1, Glo id2 => negb(peq id1 id2)
+  | Stk ofs1, Stk ofs2 =>
+      zle (Ptrofs.unsigned ofs1 + sz1) (Ptrofs.unsigned ofs2)
+      || zle (Ptrofs.unsigned ofs2 + sz2) (Ptrofs.unsigned ofs1)
+  | (Gl _ _ | Glo _ | Glob | Nonstack), (Stk _ | Stack) => true
+  | (Stk _ | Stack), (Gl _ _ | Glo _ | Glob | Nonstack) => true
+  | _, _ => false
+  end.
+
+Lemma pdisjoint_sound:
+  forall sz1 b1 ofs1 p1 sz2 b2 ofs2 p2,
+  pdisjoint p1 sz1 p2 sz2 = true ->
+  pmatch b1 ofs1 p1 -> pmatch b2 ofs2 p2 ->
+  b1 <> b2 \/ Ptrofs.unsigned ofs1 + sz1 <= Ptrofs.unsigned ofs2 \/ Ptrofs.unsigned ofs2 + sz2 <= Ptrofs.unsigned ofs1.
+Proof.
+  intros. inv H0; inv H1; simpl in H; try discriminate; try (left; congruence).
+- destruct (peq id id0). subst id0. destruct (orb_true_elim _ _ H); InvBooleans; auto.
+  left; congruence.
+- destruct (peq id id0); try discriminate. left; congruence.
+- destruct (peq id id0); try discriminate. left; congruence.
+- destruct (peq id id0); try discriminate. left; congruence.
+- destruct (orb_true_elim _ _ H); InvBooleans; auto.
+Qed.
 
 (** * Abstracting values *)
 
 Inductive aval : Type :=
   | Vbot                     (**r bottom (empty set of values) *)
   | I (n: int)               (**r exactly [Vint n] *)
-  | Uns (n: Z)               (**r a [n]-bit unsigned integer, or [Vundef] *)
-  | Sgn (n: Z)               (**r a [n]-bit signed integer, or [Vundef] *)
+  | Uns (p: aptr) (n: Z)     (**r a [n]-bit unsigned integer, or [Vundef] *)
+  | Sgn (p: aptr) (n: Z)     (**r a [n]-bit signed integer, or [Vundef] *)
   | L (n: int64)             (**r exactly [Vlong n] *)
   | F (f: float)             (**r exactly [Vfloat f] *)
   | FS (f: float32)          (**r exactly [Vsingle f] *)
-  | Vtop.
+  | Ptr (p: aptr)            (**r a pointer from the set [p], or [Vundef] *)
+  | Ifptr (p: aptr).         (**r a pointer from the set [p], or a number, or [Vundef] *)
+
+(** The "top" of the value domain is defined as any pointer, or any
+    number, or [Vundef]. *)
+
+Definition Vtop := Ifptr Ptop.
+
+(** The [p] parameter (an abstract pointer) to [Uns] and [Sgn] helps keeping
+  track of pointers that leak through arithmetic operations such as shifts.
+  See the section "Tracking leakage of pointers" below.
+  In strict analysis mode, [p] is always [Pbot]. *)
 
 Definition eq_aval: forall (v1 v2: aval), {v1=v2} + {v1<>v2}.
 Proof.
-  intros. generalize zeq Int.eq_dec Int64.eq_dec Float.eq_dec Float32.eq_dec; intros.
+  intros. generalize zeq Int.eq_dec Int64.eq_dec Float.eq_dec Float32.eq_dec eq_aptr; intros.
   decide equality.
 Defined.
 
@@ -53,18 +560,33 @@ Definition is_sgn (n: Z) (i: int) : Prop :=
 
 Inductive vmatch : val -> aval -> Prop :=
   | vmatch_i: forall i, vmatch (Vint i) (I i)
-  | vmatch_Uns: forall i n, 0 <= n -> is_uns n i -> vmatch (Vint i) (Uns n)
-  | vmatch_Uns_undef: forall n, vmatch Vundef (Uns n)
-  | vmatch_Sgn: forall i n, 0 < n -> is_sgn n i -> vmatch (Vint i) (Sgn n)
-  | vmatch_Sgn_undef: forall n, vmatch Vundef (Sgn n)
+  | vmatch_Uns: forall p i n, 0 <= n -> is_uns n i -> vmatch (Vint i) (Uns p n)
+  | vmatch_Uns_undef: forall p n, vmatch Vundef (Uns p n)
+  | vmatch_Sgn: forall p i n, 0 < n -> is_sgn n i -> vmatch (Vint i) (Sgn p n)
+  | vmatch_Sgn_undef: forall p n, vmatch Vundef (Sgn p n)
   | vmatch_l: forall i, vmatch (Vlong i) (L i)
   | vmatch_f: forall f, vmatch (Vfloat f) (F f)
   | vmatch_s: forall f, vmatch (Vsingle f) (FS f)
-  | vmatch_vtop: forall v, vmatch v Vtop.
+  | vmatch_ptr: forall b ofs p, pmatch b ofs p -> vmatch (Vptr b ofs) (Ptr p)
+  | vmatch_ptr_undef: forall p, vmatch Vundef (Ptr p)
+  | vmatch_ifptr_undef: forall p, vmatch Vundef (Ifptr p)
+  | vmatch_ifptr_i: forall i p, vmatch (Vint i) (Ifptr p)
+  | vmatch_ifptr_l: forall i p, vmatch (Vlong i) (Ifptr p)
+  | vmatch_ifptr_f: forall f p, vmatch (Vfloat f) (Ifptr p)
+  | vmatch_ifptr_s: forall f p, vmatch (Vsingle f) (Ifptr p)
+  | vmatch_ifptr_p: forall b ofs p, pmatch b ofs p -> vmatch (Vptr b ofs) (Ifptr p).
 
-Lemma vmatch_top: forall v, vmatch v Vtop.
+Lemma vmatch_ifptr:
+  forall v p,
+  (forall b ofs, v = Vptr b ofs -> pmatch b ofs p) ->
+  vmatch v (Ifptr p).
 Proof.
-  intros. constructor. 
+  intros. destruct v; constructor; auto.
+Qed.
+
+Lemma vmatch_top: forall v x, vmatch v x -> vmatch v Vtop.
+Proof.
+  intros. apply vmatch_ifptr. intros. subst v. inv H; eapply pmatch_top'; eauto.
 Qed.
 
 Hint Extern 1 (vmatch _ _) => constructor : va.
@@ -183,22 +705,53 @@ Proof.
   rewrite Int.bits_zero. destruct (zeq i 0). subst i; auto. apply H; omega.
 Qed.
 
+(** Tracking leakage of pointers through arithmetic operations.
+
+In the CompCert semantics, arithmetic operations (e.g. "xor") applied
+to pointer values are undefined or produce the [Vundef] result.
+So, in strict mode, we can abstract the result values of such operations
+as [Ifptr Pbot], namely: [Vundef], or any number, but not a pointer.
+
+In real code, such arithmetic over pointers occurs, so we need to be
+more prudent.  The policy we take, inspired by that of GCC, is that
+"undefined" arithmetic operations involving pointer arguments can
+produce a pointer, but not any pointer: rather, a pointer to the same
+block, but possibly with a different offset.  Hence, if the operation
+has a pointer to abstract region [p] as argument, the result value
+can be a pointer to abstract region [poffset p].  In other words,
+the result value is abstracted as [Ifptr (poffset p)].
+
+We encapsulate this reasoning in the following [ntop1] and [ntop2] functions
+("numerical top"). *)
+
+Definition provenance (x: aval) : aptr :=
+  if va_strict tt then Pbot else
+    match x with
+    | Ptr p | Ifptr p | Uns p _ | Sgn p _ => poffset p
+    | _ => Pbot
+    end.
+
+Definition ntop : aval := Ifptr Pbot.
+
+Definition ntop1 (x: aval) : aval := Ifptr (provenance x).
+
+Definition ntop2 (x y: aval) : aval := Ifptr (plub (provenance x) (provenance y)).
 
 (** Smart constructors for [Uns] and [Sgn]. *)
 
-Definition uns  (n: Z) : aval :=
-  if zle n 1 then Uns 1
-  else if zle n 7 then Uns 7
-  else if zle n 8 then Uns 8
-  else if zle n 15 then Uns 15
-  else if zle n 16 then Uns 16
-  else Vtop.
+Definition uns (p: aptr) (n: Z) : aval :=
+  if zle n 1 then Uns p 1
+  else if zle n 7 then Uns p 7
+  else if zle n 8 then Uns p 8
+  else if zle n 15 then Uns p 15
+  else if zle n 16 then Uns p 16
+  else Ifptr p.
 
-Definition sgn (n: Z) : aval :=
-  if zle n 8 then Sgn 8 else if zle n 16 then Sgn 16 else Vtop.
+Definition sgn (p: aptr) (n: Z) : aval :=
+  if zle n 8 then Sgn p 8 else if zle n 16 then Sgn p 16 else Ifptr p.
 
 Lemma vmatch_uns':
-  forall i n, is_uns (Z.max 0 n) i -> vmatch (Vint i) (uns n).
+  forall p i n, is_uns (Z.max 0 n) i -> vmatch (Vint i) (uns p n).
 Proof.
   intros.
   assert (A: forall n', n' >= 0 -> n' >= n -> is_uns n' i) by (eauto with va).
@@ -212,12 +765,12 @@ Proof.
 Qed.
 
 Lemma vmatch_uns:
-  forall i n, is_uns n i -> vmatch (Vint i) (uns n).
+  forall p i n, is_uns n i -> vmatch (Vint i) (uns p n).
 Proof.
   intros. apply vmatch_uns'. eauto with va.
 Qed.
 
-Lemma vmatch_uns_undef: forall n, vmatch Vundef (uns n).
+Lemma vmatch_uns_undef: forall p n, vmatch Vundef (uns p n).
 Proof.
   intros. unfold uns.
   destruct (zle n 1). auto with va.
@@ -228,7 +781,7 @@ Proof.
 Qed.
 
 Lemma vmatch_sgn':
-  forall i n, is_sgn (Z.max 1 n) i -> vmatch (Vint i) (sgn n).
+  forall p i n, is_sgn (Z.max 1 n) i -> vmatch (Vint i) (sgn p n).
 Proof.
   intros.
   assert (A: forall n', n' >= 1 -> n' >= n -> is_sgn n' i) by (eauto with va).
@@ -238,12 +791,12 @@ Proof.
 Qed.
 
 Lemma vmatch_sgn:
-  forall i n, is_sgn n i -> vmatch (Vint i) (sgn n).
+  forall p i n, is_sgn n i -> vmatch (Vint i) (sgn p n).
 Proof.
   intros. apply vmatch_sgn'. eauto with va.
 Qed.
 
-Lemma vmatch_sgn_undef: forall n, vmatch Vundef (sgn n).
+Lemma vmatch_sgn_undef: forall p n, vmatch Vundef (sgn p n).
 Proof.
   intros. unfold sgn.
   destruct (zle n 8). auto with va.
@@ -253,7 +806,7 @@ Qed.
 Hint Resolve vmatch_uns vmatch_uns_undef vmatch_sgn vmatch_sgn_undef : va.
 
 Lemma vmatch_Uns_1:
-  forall v, vmatch v (Uns 1) -> v = Vundef \/ v = Vint Int.zero \/ v = Vint Int.one.
+  forall p v, vmatch v (Uns p 1) -> v = Vundef \/ v = Vint Int.zero \/ v = Vint Int.one.
 Proof.
   intros. inv H; auto. right. exploit is_uns_1; eauto. intuition congruence.
 Qed.
@@ -266,12 +819,20 @@ Inductive vge: aval -> aval -> Prop :=
   | vge_l: forall i, vge (L i) (L i)
   | vge_f: forall f, vge (F f) (F f)
   | vge_s: forall f, vge (FS f) (FS f)
-  | vge_uns_i: forall n i, 0 <= n -> is_uns n i -> vge (Uns n) (I i)
-  | vge_uns_uns: forall n1 n2, n1 >= n2  -> vge (Uns n1) (Uns n2)
-  | vge_sgn_i: forall n i, 0 < n -> is_sgn n i -> vge (Sgn n) (I i)
-  | vge_sgn_sgn: forall n1 n2, n1 >= n2 -> vge (Sgn n1) (Sgn n2)
-  | vge_sgn_uns: forall n1 n2, n1 > n2 -> vge (Sgn n1) (Uns n2)
-  | vge_top_v: forall av, vge Vtop av.
+  | vge_uns_i: forall p n i, 0 <= n -> is_uns n i -> vge (Uns p n) (I i)
+  | vge_uns_uns: forall p1 n1 p2 n2, n1 >= n2 -> pge p1 p2 -> vge (Uns p1 n1) (Uns p2 n2)
+  | vge_sgn_i: forall p n i, 0 < n -> is_sgn n i -> vge (Sgn p n) (I i)
+  | vge_sgn_sgn: forall p1 n1 p2 n2, n1 >= n2 -> pge p1 p2 -> vge (Sgn p1 n1) (Sgn p2 n2)
+  | vge_sgn_uns: forall p1 n1 p2 n2, n1 > n2 -> pge p1 p2 -> vge (Sgn p1 n1) (Uns p2 n2)
+  | vge_p_p: forall p q, pge p q -> vge (Ptr p) (Ptr q)
+  | vge_ip_p: forall p q, pge p q -> vge (Ifptr p) (Ptr q)
+  | vge_ip_ip: forall p q, pge p q -> vge (Ifptr p) (Ifptr q)
+  | vge_ip_i: forall p i, vge (Ifptr p) (I i)
+  | vge_ip_l: forall p i, vge (Ifptr p) (L i)
+  | vge_ip_f: forall p f, vge (Ifptr p) (F f)
+  | vge_ip_s: forall p f, vge (Ifptr p) (FS f)
+  | vge_ip_uns: forall p q n, pge p q -> vge (Ifptr p) (Uns q n)
+  | vge_ip_sgn: forall p q n, pge p q -> vge (Ifptr p) (Sgn q n).
 
 Hint Constructors vge : va.
 
@@ -289,13 +850,13 @@ Qed.
 
 Lemma vge_trans: forall u v, vge u v -> forall w, vge v w -> vge u w.
 Proof.
-  induction 1; intros w V; inv V; eauto with va. 
+  induction 1; intros w V; inv V; eauto using pge_trans with va.
 Qed.
 
 Lemma vmatch_ge:
   forall v x y, vge x y -> vmatch v y -> vmatch v x.
 Proof.
-  induction 1; intros V; inv V; eauto  with va.
+  induction 1; intros V; inv V; eauto using pmatch_ge with va.
 Qed.
 
 (** Least upper bound *)
@@ -307,24 +868,33 @@ Definition vlub (v w: aval) : aval :=
   | I i1, I i2 =>
       if Int.eq i1 i2 then v else
       if Int.lt i1 Int.zero || Int.lt i2 Int.zero
-      then sgn (Z.max (ssize i1) (ssize i2))
-      else uns (Z.max (usize i1) (usize i2))
-  | I i, Uns n | Uns n, I i =>
+      then sgn Pbot (Z.max (ssize i1) (ssize i2))
+      else uns Pbot (Z.max (usize i1) (usize i2))
+  | I i, Uns p n | Uns p n, I i =>
       if Int.lt i Int.zero
-      then sgn (Z.max (ssize i) (n + 1))
-      else uns (Z.max (usize i) n)
-  | I i, Sgn n | Sgn n, I i =>
-      sgn (Z.max (ssize i) n)
-  | Uns n1, Uns n2 => Uns (Z.max n1 n2)
-  | Uns n1, Sgn n2 => sgn (Z.max (n1 + 1) n2)
-  | Sgn n1, Uns n2 => sgn (Z.max n1 (n2 + 1))
-  | Sgn n1, Sgn n2 => sgn (Z.max n1 n2)
+      then sgn p (Z.max (ssize i) (n + 1))
+      else uns p (Z.max (usize i) n)
+  | I i, Sgn p n | Sgn p n, I i =>
+      sgn p (Z.max (ssize i) n)
+  | I i, (Ptr p | Ifptr p) | (Ptr p | Ifptr p), I i =>
+      if va_strict tt || Int.eq i Int.zero then Ifptr p else Vtop
+  | Uns p1 n1, Uns p2 n2 => Uns (plub p1 p2) (Z.max n1 n2)
+  | Uns p1 n1, Sgn p2 n2 => sgn (plub p1 p2) (Z.max (n1 + 1) n2)
+  | Sgn p1 n1, Uns p2 n2 => sgn (plub p1 p2) (Z.max n1 (n2 + 1))
+  | Sgn p1 n1, Sgn p2 n2 => sgn (plub p1 p2) (Z.max n1 n2)
   | F f1, F f2 =>
-      if Float.eq_dec f1 f2 then v else Vtop
+      if Float.eq_dec f1 f2 then v else ntop
   | FS f1, FS f2 =>
-      if Float32.eq_dec f1 f2 then v else Vtop
+      if Float32.eq_dec f1 f2 then v else ntop
   | L i1, L i2 =>
-      if Int64.eq i1 i2 then v else Vtop
+      if Int64.eq i1 i2 then v else ntop
+  | Ptr p1, Ptr p2 => Ptr(plub p1 p2)
+  | Ptr p1, Ifptr p2 => Ifptr(plub p1 p2)
+  | Ifptr p1, Ptr p2 => Ifptr(plub p1 p2)
+  | Ifptr p1, Ifptr p2 => Ifptr(plub p1 p2)
+  | (Ptr p1 | Ifptr p1), (Uns p2 _ | Sgn p2 _) => Ifptr(plub p1 p2)
+  | (Uns p1 _ | Sgn p1 _), (Ptr p2 | Ifptr p2) => Ifptr(plub p1 p2)
+  | _, (Ptr p | Ifptr p) | (Ptr p | Ifptr p), _ => if va_strict tt then Ifptr p else Vtop
   | _, _ => Vtop
   end.
 
@@ -336,16 +906,28 @@ Proof.
   congruence.
   rewrite orb_comm.
   destruct (Int.lt n0 Int.zero || Int.lt n Int.zero); f_equal; apply Z.max_comm.
-- f_equal.  apply Z.max_comm.
-- f_equal.  apply Z.max_comm.
-- f_equal.  apply Z.max_comm.
-- f_equal.  apply Z.max_comm.
+- f_equal. apply plub_comm. apply Z.max_comm.
+- f_equal. apply plub_comm. apply Z.max_comm.
+- f_equal; apply plub_comm.
+- f_equal; apply plub_comm.
+- f_equal. apply plub_comm. apply Z.max_comm.
+- f_equal. apply plub_comm. apply Z.max_comm.
+- f_equal; apply plub_comm.
+- f_equal; apply plub_comm.
 - rewrite Int64.eq_sym. predSpec Int64.eq Int64.eq_spec n0 n; congruence.
 - rewrite dec_eq_sym. destruct (Float.eq_dec f0 f). congruence. auto.
 - rewrite dec_eq_sym. destruct (Float32.eq_dec f0 f). congruence. auto.
+- f_equal; apply plub_comm.
+- f_equal; apply plub_comm.
+- f_equal; apply plub_comm.
+- f_equal; apply plub_comm.
+- f_equal; apply plub_comm.
+- f_equal; apply plub_comm.
+- f_equal; apply plub_comm.
+- f_equal; apply plub_comm.
 Qed.
 
-Lemma vge_uns_uns': forall n, vge (uns n) (Uns n).
+Lemma vge_uns_uns': forall p n, vge (uns p n) (Uns p n).
 Proof.
   unfold uns; intros.
   destruct (zle n 1). auto with va.
@@ -355,21 +937,21 @@ Proof.
   destruct (zle n 16); auto with va.
 Qed.
 
-Lemma vge_uns_i': forall n i, 0 <= n -> is_uns n i -> vge (uns n) (I i).
+Lemma vge_uns_i': forall p n i, 0 <= n -> is_uns n i -> vge (uns p n) (I i).
 Proof.
-  intros. apply vge_trans with (Uns n). apply vge_uns_uns'. auto with va.
+  intros. apply vge_trans with (Uns p n). apply vge_uns_uns'. auto with va.
 Qed.
 
-Lemma vge_sgn_sgn': forall n, vge (sgn n) (Sgn n).
+Lemma vge_sgn_sgn': forall p n, vge (sgn p n) (Sgn p n).
 Proof.
   unfold sgn; intros.
   destruct (zle n 8). auto with va.
   destruct (zle n 16); auto with va.
 Qed.
 
-Lemma vge_sgn_i': forall n i, 0 < n -> is_sgn n i -> vge (sgn n) (I i).
+Lemma vge_sgn_i': forall p n i, 0 < n -> is_sgn n i -> vge (sgn p n) (I i).
 Proof.
-  intros. apply vge_trans with (Sgn n). apply vge_sgn_sgn'. auto with va.
+  intros. apply vge_trans with (Sgn p n). apply vge_sgn_sgn'. auto with va.
 Qed.
 
 Hint Resolve vge_uns_uns' vge_uns_i' vge_sgn_sgn' vge_sgn_i' : va.
@@ -390,7 +972,7 @@ Lemma vge_lub_l:
 Proof.
   assert (IFSTRICT: forall (cond: bool) x1 x2 y, vge x1 y -> vge x2 y -> vge (if cond then x1 else x2) y).
   { destruct cond; auto with va. }
-  unfold vlub; destruct x, y; eauto with va.
+  unfold vlub; destruct x, y; eauto using pge_lub_l with va.
 - predSpec Int.eq Int.eq_spec n n0. auto with va.
   destruct (Int.lt n Int.zero || Int.lt n0 Int.zero).
   apply vge_sgn_i'. generalize (ssize_pos n); xomega. eauto with va.
@@ -401,13 +983,14 @@ Proof.
 - apply vge_sgn_i'. generalize (ssize_pos n); xomega. eauto with va.
 - destruct (Int.lt n0 Int.zero).
   eapply vge_trans. apply vge_sgn_sgn'.
-  apply vge_trans with (Sgn (n + 1)); eauto with va.
+  apply vge_trans with (Sgn p (n + 1)); eauto with va.
   eapply vge_trans. apply vge_uns_uns'. eauto with va.
 - eapply vge_trans. apply vge_sgn_sgn'.
-  apply vge_trans with (Sgn (n + 1)); eauto  with va.
+  apply vge_trans with (Sgn p (n + 1)); eauto using pge_lub_l with va.
 - eapply vge_trans. apply vge_sgn_sgn'. eauto with va.
-- eapply vge_trans. apply vge_sgn_sgn'. eauto with va.
-- eapply vge_trans. apply vge_sgn_sgn'. eauto with va.
+- eapply vge_trans. apply vge_sgn_sgn'. eauto using pge_lub_l with va.
+- eapply vge_trans. apply vge_sgn_sgn'. eauto using pge_lub_l with va.
+- destruct (Int64.eq n n0); constructor.
 - destruct (Float.eq_dec f f0); constructor.
 - destruct (Float32.eq_dec f f0); constructor.
 Qed.
@@ -430,35 +1013,147 @@ Proof.
   intros. rewrite vlub_comm. apply vmatch_lub_l; auto.
 Qed.
 
+(** In the CompCert semantics, a memory load or store succeeds only
+  if the address is a pointer value.  Hence, in strict mode,
+  [aptr_of_aval x] returns [Pbot] (no pointer value) if [x]
+  denotes a number or [Vundef].  However, in real code, memory
+  addresses are sometimes synthesized from integers, e.g. an absolute
+  address for a hardware device.  It is a reasonable assumption
+  that these absolute addresses do not point within the stack block,
+  however.  Therefore, in relaxed mode, [aptr_of_aval x] returns
+  [Nonstack] (any pointer outside the stack) when [x] denotes a number. *)
+
+Definition aptr_of_aval (v: aval) : aptr :=
+  match v with
+  | Ptr p => p
+  | Ifptr p => p
+  | _ => if va_strict tt then Pbot else Nonstack
+  end.
+
+Lemma match_aptr_of_aval:
+  forall b ofs av,
+  vmatch (Vptr b ofs) av -> pmatch b ofs (aptr_of_aval av).
+Proof.
+  unfold aptr_of_aval; intros. inv H; auto.
+Qed.
+
+Definition vplub (v: aval) (p: aptr) : aptr :=
+  match v with
+  | Ptr q => plub q p
+  | Ifptr q => plub q p
+  | _ => p
+  end.
+
+Lemma vmatch_vplub_l:
+  forall v x p, vmatch v x -> vmatch v (Ifptr (vplub x p)).
+Proof.
+  intros. unfold vplub; inv H; auto with va; constructor; eapply pmatch_lub_l; eauto.
+Qed.
+
+Lemma pmatch_vplub:
+  forall b ofs x p, pmatch b ofs p -> pmatch b ofs (vplub x p).
+Proof.
+  intros.
+  assert (DFL: pmatch b ofs (if va_strict tt then p else Ptop)).
+  { destruct (va_strict tt); auto. eapply pmatch_top'; eauto. }
+  unfold vplub; destruct x; auto; apply pmatch_lub_r; auto.
+Qed.
+
+Lemma vmatch_vplub_r:
+  forall v x p, vmatch v (Ifptr p) -> vmatch v (Ifptr (vplub x p)).
+Proof.
+  intros. apply vmatch_ifptr; intros; subst v. inv H. apply pmatch_vplub; auto.
+Qed.
+
+(** Inclusion *)
+
+Definition vpincl (v: aval) (p: aptr) : bool :=
+  match v with
+  | Ptr q | Ifptr q | Uns q _ | Sgn q _ => pincl q p
+  | _ => true
+  end.
+
+Lemma vpincl_ge:
+  forall x p, vpincl x p = true -> vge (Ifptr p) x.
+Proof.
+  unfold vpincl; intros. destruct x; constructor; apply pincl_ge; auto.
+Qed.
+
+Lemma vpincl_sound:
+  forall v x p, vpincl x p = true -> vmatch v x -> vmatch v (Ifptr p).
+Proof.
+  intros. apply vmatch_ge with x; auto. apply vpincl_ge; auto.
+Qed.
 
 Definition vincl (v w: aval) : bool :=
   match v, w with
   | Vbot, _ => true
   | I i, I j => Int.eq_dec i j
-  | I i, Uns n => Int.eq_dec (Int.zero_ext n i) i && zle 0 n
-  | I i, Sgn n => Int.eq_dec (Int.sign_ext n i) i && zlt 0 n
-  | Uns n, Uns m => zle n m 
-  | Uns n, Sgn m => zlt n m 
-  | Sgn n, Sgn m => zle n m 
+  | I i, Uns p n => Int.eq_dec (Int.zero_ext n i) i && zle 0 n
+  | I i, Sgn p n => Int.eq_dec (Int.sign_ext n i) i && zlt 0 n
+  | Uns p n, Uns q m => zle n m && pincl p q
+  | Uns p n, Sgn q m => zlt n m && pincl p q
+  | Sgn p n, Sgn q m => zle n m && pincl p q
   | L i, L j => Int64.eq_dec i j
   | F i, F j => Float.eq_dec i j
   | FS i, FS j => Float32.eq_dec i j
-  | _, Vtop => true
+  | Ptr p, Ptr q => pincl p q
+  | (Ptr p | Ifptr p | Uns p _ | Sgn p _), Ifptr q => pincl p q
+  | _, Ifptr _ => true
   | _, _ => false
   end.
 
 Lemma vincl_ge: forall v w, vincl v w = true -> vge w v.
 Proof.
   unfold vincl; destruct v; destruct w;
-  intros; try discriminate; try InvBooleans; try subst; auto  with va.
+  intros; try discriminate; try InvBooleans; try subst; auto using pincl_ge with va.
 - constructor; auto. rewrite is_uns_zero_ext; auto.
 - constructor; auto. rewrite is_sgn_sign_ext; auto.
+Qed.
+
+(** Loading constants *)
+
+Definition genv_match (ge: genv) : Prop :=
+  (forall id b, Genv.find_symbol ge id = Some b <-> bc b = BCglob id)
+/\(forall b, Plt b (Genv.genv_next ge) -> bc b <> BCinvalid /\ bc b <> BCstack).
+
+Lemma symbol_address_sound:
+  forall ge id ofs,
+  genv_match ge ->
+  vmatch (Genv.symbol_address ge id ofs) (Ptr (Gl id ofs)).
+Proof.
+  intros. unfold Genv.symbol_address. destruct (Genv.find_symbol ge id) as [b|] eqn:F.
+  constructor. constructor. apply H; auto.
+  constructor.
+Qed.
+
+Lemma vmatch_ptr_gl:
+  forall ge v id ofs,
+  genv_match ge ->
+  vmatch v (Ptr (Gl id ofs)) ->
+  Val.lessdef v (Genv.symbol_address ge id ofs).
+Proof.
+  intros. unfold Genv.symbol_address. inv H0.
+- inv H3. replace (Genv.find_symbol ge id) with (Some b). constructor.
+  symmetry. apply H; auto.
+- constructor.
+Qed.
+
+Lemma vmatch_ptr_stk:
+  forall v ofs sp,
+  vmatch v (Ptr(Stk ofs)) ->
+  bc sp = BCstack ->
+  Val.lessdef v (Vptr sp ofs).
+Proof.
+  intros. inv H.
+- inv H3. replace b with sp by (eapply bc_stack; eauto). constructor.
+- constructor.
 Qed.
 
 (** Generic operations that just do constant propagation. *)
 
 Definition unop_int (sem: int -> int) (x: aval) :=
-  match x with I n => I (sem n) | _ => Vtop end.
+  match x with I n => I (sem n) | _ => ntop1 x end.
 
 Lemma unop_int_sound:
   forall sem v x,
@@ -469,7 +1164,7 @@ Proof.
 Qed.
 
 Definition binop_int (sem: int -> int -> int) (x y: aval) :=
-  match x, y with I n, I m => I (sem n m) | _, _ => Vtop end.
+  match x, y with I n, I m => I (sem n m) | _, _ => ntop2 x y end.
 
 Lemma binop_int_sound:
   forall sem v x w y,
@@ -480,7 +1175,7 @@ Proof.
 Qed.
 
 Definition unop_long (sem: int64 -> int64) (x: aval) :=
-  match x with L n => L (sem n) | _ => Vtop end.
+  match x with L n => L (sem n) | _ => ntop1 x end.
 
 Lemma unop_long_sound:
   forall sem v x,
@@ -491,7 +1186,7 @@ Proof.
 Qed.
 
 Definition binop_long (sem: int64 -> int64 -> int64) (x y: aval) :=
-  match x, y with L n, L m => L (sem n m) | _, _ => Vtop end.
+  match x, y with L n, L m => L (sem n m) | _, _ => ntop2 x y end.
 
 Lemma binop_long_sound:
   forall sem v x w y,
@@ -502,7 +1197,7 @@ Proof.
 Qed.
 
 Definition unop_float (sem: float -> float) (x: aval) :=
-  match x with F n => F (sem n) | _ => Vtop end.
+  match x with F n => F (sem n) | _ => ntop1 x end.
 
 Lemma unop_float_sound:
   forall sem v x,
@@ -513,7 +1208,7 @@ Proof.
 Qed.
 
 Definition binop_float (sem: float -> float -> float) (x y: aval) :=
-  match x, y with F n, F m => F (sem n m) | _, _ => Vtop end.
+  match x, y with F n, F m => F (sem n m) | _, _ => ntop2 x y end.
 
 Lemma binop_float_sound:
   forall sem v x w y,
@@ -524,7 +1219,7 @@ Proof.
 Qed.
 
 Definition unop_single (sem: float32 -> float32) (x: aval) :=
-  match x with FS n => FS (sem n) | _ => Vtop end.
+  match x with FS n => FS (sem n) | _ => ntop1 x end.
 
 Lemma unop_single_sound:
   forall sem v x,
@@ -535,7 +1230,7 @@ Proof.
 Qed.
 
 Definition binop_single (sem: float32 -> float32 -> float32) (x y: aval) :=
-  match x, y with FS n, FS m => FS (sem n m) | _, _ => Vtop end.
+  match x, y with FS n, FS m => FS (sem n m) | _, _ => ntop2 x y end.
 
 Lemma binop_single_sound:
   forall sem v x w y,
@@ -553,21 +1248,22 @@ Definition shl (v w: aval) :=
       if Int.ltu amount Int.iwordsize then
         match v with
         | I i => I (Int.shl i amount)
-        | Uns n => uns (n + Int.unsigned amount)
-        | Sgn n => sgn (n + Int.unsigned amount)
-        | _ => Vtop
+        | Uns p n => uns p (n + Int.unsigned amount)
+        | Sgn p n => sgn p (n + Int.unsigned amount)
+        | _ => ntop1 v
         end
-      else Vtop
-  | _ => Vtop
+      else ntop1 v
+  | _ => ntop1 v
   end.
 
 Lemma shl_sound:
   forall v w x y, vmatch v x -> vmatch w y -> vmatch (Val.shl v w) (shl x y).
 Proof.
   intros.
-  assert (DEFAULT: vmatch (Val.shl v w) Vtop).
+  assert (DEFAULT: vmatch (Val.shl v w) (ntop1 x)).
   {
     destruct v; destruct w; simpl; try constructor.
+    destruct (Int.ltu i0 Int.iwordsize); constructor.
   }
   destruct y; auto. simpl. inv H0. unfold Val.shl.
   destruct (Int.ltu n Int.iwordsize) eqn:LTU; auto.
@@ -588,35 +1284,36 @@ Definition shru (v w: aval) :=
       if Int.ltu amount Int.iwordsize then
         match v with
         | I i => I (Int.shru i amount)
-        | Uns n => uns (n - Int.unsigned amount)
-        | _ => uns (Int.zwordsize - Int.unsigned amount)
+        | Uns p n => uns p (n - Int.unsigned amount)
+        | _ => uns (provenance v) (Int.zwordsize - Int.unsigned amount)
         end
-      else Vtop
-  | _ => Vtop
+      else ntop1 v
+  | _ => ntop1 v
   end.
 
 Lemma shru_sound:
   forall v w x y, vmatch v x -> vmatch w y -> vmatch (Val.shru v w) (shru x y).
 Proof.
   intros.
-  assert (DEFAULT: vmatch (Val.shru v w) Vtop)
-    by (destruct v; destruct w; simpl; try constructor).
+  assert (DEFAULT: vmatch (Val.shru v w) (ntop1 x)).
+  {
+    destruct v; destruct w; simpl; try constructor.
+    destruct (Int.ltu i0 Int.iwordsize); constructor.
+  }
   destruct y; auto. inv H0. unfold shru, Val.shru.
   destruct (Int.ltu n Int.iwordsize) eqn:LTU; auto.
-  - exploit Int.ltu_inv; eauto.
-    intros RANGE. change (Int.unsigned Int.iwordsize) with Int.zwordsize in RANGE.
-    assert (DEFAULT2: forall i, vmatch (Vint (Int.shru i n)) (uns (Int.zwordsize - Int.unsigned n))).
-    {
-      intros. apply vmatch_uns. red; intros.
-      rewrite Int.bits_shru by omega. apply zlt_false. omega.
-    }
-    inv H; auto with va.
-    + apply vmatch_uns'. red; intros. zify.
-      rewrite Int.bits_shru by omega.
-      destruct (zlt (m + Int.unsigned n) Int.zwordsize); auto.
-      apply H1; omega.
-    + destruct v ; eauto with va. 
-  - destruct v; constructor.
+  exploit Int.ltu_inv; eauto. intros RANGE. change (Int.unsigned Int.iwordsize) with Int.zwordsize in RANGE.
+  assert (DEFAULT2: forall i, vmatch (Vint (Int.shru i n)) (uns (provenance x) (Int.zwordsize - Int.unsigned n))).
+  {
+    intros. apply vmatch_uns. red; intros.
+    rewrite Int.bits_shru by omega. apply zlt_false. omega.
+  }
+  inv H; auto with va.
+- apply vmatch_uns'. red; intros. zify.
+  rewrite Int.bits_shru by omega.
+  destruct (zlt (m + Int.unsigned n) Int.zwordsize); auto.
+  apply H1; omega.
+- destruct v; constructor.
 Qed.
 
 Definition shr (v w: aval) :=
@@ -625,34 +1322,35 @@ Definition shr (v w: aval) :=
       if Int.ltu amount Int.iwordsize then
         match v with
         | I i => I (Int.shr i amount)
-        | Uns n => sgn (n + 1 - Int.unsigned amount)
-        | Sgn n => sgn (n - Int.unsigned amount)
-        | _ => sgn (Int.zwordsize - Int.unsigned amount)
+        | Uns p n => sgn p (n + 1 - Int.unsigned amount)
+        | Sgn p n => sgn p (n - Int.unsigned amount)
+        | _ => sgn (provenance v) (Int.zwordsize - Int.unsigned amount)
         end
-      else Vtop
-  | _ => Vtop
+      else ntop1 v
+  | _ => ntop1 v
   end.
 
 Lemma shr_sound:
   forall v w x y, vmatch v x -> vmatch w y -> vmatch (Val.shr v w) (shr x y).
 Proof.
   intros.
-  assert (DEFAULT: vmatch (Val.shr v w) Vtop).
+  assert (DEFAULT: vmatch (Val.shr v w) (ntop1 x)).
   {
     destruct v; destruct w; simpl; try constructor.
+    destruct (Int.ltu i0 Int.iwordsize); constructor.
   }
   destruct y; auto. inv H0. unfold shr, Val.shr.
   destruct (Int.ltu n Int.iwordsize) eqn:LTU; auto.
   exploit Int.ltu_inv; eauto. intros RANGE. change (Int.unsigned Int.iwordsize) with Int.zwordsize in RANGE.
-  assert (DEFAULT2: forall i, vmatch (Vint (Int.shr i n)) (sgn (Int.zwordsize - Int.unsigned n))).
+  assert (DEFAULT2: forall i, vmatch (Vint (Int.shr i n)) (sgn (provenance x) (Int.zwordsize - Int.unsigned n))).
   {
     intros. apply vmatch_sgn. red; intros.
     rewrite ! Int.bits_shr by omega. f_equal.
     destruct (zlt (m + Int.unsigned n) Int.zwordsize);
     destruct (zlt (Int.zwordsize - 1 + Int.unsigned n) Int.zwordsize);
     omega.
-  } 
-  assert (SGN: forall i p, is_sgn p i -> 0 < p -> vmatch (Vint (Int.shr i n)) (sgn (p - Int.unsigned n))).
+  }
+  assert (SGN: forall q i p, is_sgn p i -> 0 < p -> vmatch (Vint (Int.shr i n)) (sgn q (p - Int.unsigned n))).
   {
     intros. apply vmatch_sgn'. red; intros. zify.
     rewrite ! Int.bits_shr by omega.
@@ -666,20 +1364,19 @@ Proof.
     auto.
   }
   inv H; eauto with va.
-  - destruct v ; auto with va.
-  - destruct v; constructor.
+- destruct v; constructor.
 Qed.
 
 Definition and (v w: aval) :=
   match v, w with
   | I i1, I i2 => I (Int.and i1 i2)
-  | I i, Uns n | Uns n, I i => uns (Z.min n (usize i))
-  | I i, x | x, I i => uns (usize i)
-  | Uns n1, Uns n2 => uns (Z.min n1 n2)
-  | Uns n, _ => uns n
-  | _, Uns n => uns n
-  | Sgn n1, Sgn n2 => sgn (Z.max n1 n2)
-  | _, _ => Vtop
+  | I i, Uns p n | Uns p n, I i => uns p (Z.min n (usize i))
+  | I i, x | x, I i => uns (provenance x) (usize i)
+  | Uns p1 n1, Uns p2 n2 => uns (plub p1 p2) (Z.min n1 n2)
+  | Uns p n, _ => uns (plub p (provenance w)) n
+  | _, Uns p n => uns (plub (provenance v) p) n
+  | Sgn p1 n1, Sgn p2 n2 => sgn (plub p1 p2) (Z.max n1 n2)
+  | _, _ => ntop2 v w
   end.
 
 Lemma and_sound:
@@ -703,19 +1400,16 @@ Proof.
     intros; red; intros. rewrite ! Int.bits_and by auto with va.
     rewrite H by auto with va. rewrite H0 by auto with va. auto.
   }
-  intros.
-  unfold and, Val.and; inv H; eauto with va; inv H0;
-    try (destruct w) ;
-    try (destruct v) ; eauto with va.
+  intros. unfold and, Val.and; inv H; eauto with va; inv H0; eauto with va.
 Qed.
 
 Definition or (v w: aval) :=
   match v, w with
   | I i1, I i2 => I (Int.or i1 i2)
-  | I i, Uns n | Uns n, I i => uns (Z.max n (usize i))
-  | Uns n1, Uns n2 => uns  (Z.max n1 n2)
-  | Sgn n1, Sgn n2 => sgn  (Z.max n1 n2)
-  | _, _ => Vtop
+  | I i, Uns p n | Uns p n, I i => uns p (Z.max n (usize i))
+  | Uns p1 n1, Uns p2 n2 => uns (plub p1 p2) (Z.max n1 n2)
+  | Sgn p1 n1, Sgn p2 n2 => sgn (plub p1 p2) (Z.max n1 n2)
+  | _, _ => ntop2 v w
   end.
 
 Lemma or_sound:
@@ -737,10 +1431,10 @@ Qed.
 Definition xor (v w: aval) :=
   match v, w with
   | I i1, I i2 => I (Int.xor i1 i2)
-  | I i, Uns n | Uns n, I i => uns (Z.max n (usize i))
-  | Uns n1, Uns n2 => uns  (Z.max n1 n2)
-  | Sgn n1, Sgn n2 => sgn  (Z.max n1 n2)
-  | _, _ => Vtop
+  | I i, Uns p n | Uns p n, I i => uns p (Z.max n (usize i))
+  | Uns p1 n1, Uns p2 n2 => uns (plub p1 p2) (Z.max n1 n2)
+  | Sgn p1 n1, Sgn p2 n2 => sgn (plub p1 p2) (Z.max n1 n2)
+  | _, _ => ntop2 v w
   end.
 
 Lemma xor_sound:
@@ -762,9 +1456,9 @@ Qed.
 Definition notint (v: aval) :=
   match v with
   | I i => I (Int.not i)
-  | Uns n => sgn (n + 1)
-  | Sgn n => Sgn n
-  | _ => Vtop
+  | Uns p n => sgn p (n + 1)
+  | Sgn p n => Sgn p n
+  | _ => ntop1 v
   end.
 
 Lemma notint_sound:
@@ -781,26 +1475,29 @@ Qed.
 Definition rol (x y: aval) :=
   match y, x with
   | I j, I i => I(Int.rol i j)
-  | I j, Uns n => uns (n + Int.unsigned j)
-  | I j, Sgn n => if zlt n Int.zwordsize then sgn (n + Int.unsigned j) else Vtop
-  | _, _ => Vtop
+  | I j, Uns p n => uns p (n + Int.unsigned j)
+  | I j, Sgn p n => if zlt n Int.zwordsize then sgn p (n + Int.unsigned j) else ntop1 x
+  | _, _ => ntop1 x
   end.
 
 Lemma rol_sound:
   forall v w x y, vmatch v x -> vmatch w y -> vmatch (Val.rol v w) (rol x y).
 Proof.
   intros.
-  assert (DEFAULT: vmatch (Val.rol v w) Vtop) by constructor.
+  assert (DEFAULT: forall p, vmatch (Val.rol v w) (Ifptr p)).
+  {
+    destruct v; destruct w; simpl; constructor.
+  }
   unfold rol; destruct y; try apply DEFAULT; auto. inv H0. unfold Val.rol.
   inv H; auto with va.
 - apply vmatch_uns. red; intros. rewrite Int.bits_rol by auto.
   generalize (Int.unsigned_range n); intros.
-  rewrite Zmod_small by omega.
+  rewrite Z.mod_small by omega.
   apply H1. omega. omega.
 - destruct (zlt n0 Int.zwordsize); auto with va.
   apply vmatch_sgn. red; intros. rewrite ! Int.bits_rol by omega.
   generalize (Int.unsigned_range n); intros.
-  rewrite ! Zmod_small by omega.
+  rewrite ! Z.mod_small by omega.
   rewrite H1 by omega. symmetry. rewrite H1 by omega. auto.
 - destruct (zlt n0 Int.zwordsize); auto with va.
 Qed.
@@ -808,14 +1505,17 @@ Qed.
 Definition ror (x y: aval) :=
   match y, x with
   | I j, I i => I(Int.ror i j)
-  | _, _ => Vtop
+  | _, _ => ntop1 x
   end.
 
 Lemma ror_sound:
   forall v w x y, vmatch v x -> vmatch w y -> vmatch (Val.ror v w) (ror x y).
 Proof.
   intros.
-  assert (DEFAULT: vmatch (Val.ror v w) Vtop) by constructor.
+  assert (DEFAULT: forall p, vmatch (Val.ror v w) (Ifptr p)).
+  {
+    destruct v; destruct w; simpl; constructor.
+  }
   unfold ror; destruct y; try apply DEFAULT; auto. inv H0. unfold Val.ror.
   inv H; auto with va.
 Qed.
@@ -844,7 +1544,12 @@ Proof (unop_int_sound Int.neg).
 Definition add (x y: aval) :=
   match x, y with
   | I i, I j => I (Int.add i j)
-  | _, _ => Vtop
+  | Ptr p, I i | I i, Ptr p => Ptr (if Archi.ptr64 then poffset p else padd p (Ptrofs.of_int i))
+  | Ptr p, _   | _, Ptr p   => Ptr (poffset p)
+  | Ifptr p, I i | I i, Ifptr p => Ifptr (if Archi.ptr64 then poffset p else padd p (Ptrofs.of_int i))
+  | Ifptr p, Ifptr q => Ifptr (plub (poffset p) (poffset q))
+  | Ifptr p, _ | _, Ifptr p => Ifptr (poffset p)
+  | _, _ => ntop2 x y
   end.
 
 Lemma add_sound:
@@ -854,12 +1559,18 @@ Proof.
 - inv H; inv H0; constructor.
 - inv H; inv H0; constructor;
   ((apply padd_sound; assumption) || (eapply poffset_sound; eassumption) || idtac).
+  apply pmatch_lub_r. eapply poffset_sound; eauto.
+  apply pmatch_lub_l. eapply poffset_sound; eauto.
 Qed.
 
 Definition sub (v w: aval) :=
   match v, w with
   | I i1, I i2 => I (Int.sub i1 i2)
-  | _, _ => Vtop
+  | Ptr p, I i => if Archi.ptr64 then Ifptr (poffset p) else Ptr (psub p (Ptrofs.of_int i))
+  | Ptr p, _   => Ifptr (poffset p)
+  | Ifptr p, I i => if Archi.ptr64 then Ifptr (plub (poffset p) (provenance w)) else Ifptr (psub p (Ptrofs.of_int i))
+  | Ifptr p, _ => Ifptr (plub (poffset p) (provenance w))
+  | _, _ => ntop2 v w
   end.
 
 Lemma sub_sound:
@@ -867,7 +1578,7 @@ Lemma sub_sound:
 Proof.
   intros. unfold Val.sub, sub. destruct Archi.ptr64.
 - inv H; inv H0; eauto with va.
-- inv H; inv H0; try (destruct (eq_block b b0)); eauto  with va.
+- inv H; inv H0; try (destruct (eq_block b b0)); eauto using psub_sound, poffset_sound, pmatch_lub_l with va.
 Qed.
 
 Definition mul := binop_int Int.mul.
@@ -893,9 +1604,9 @@ Definition divs (v w: aval) :=
   | I i2, I i1 =>
       if Int.eq i2 Int.zero
       || Int.eq i1 (Int.repr Int.min_signed) && Int.eq i2 Int.mone
-      then if va_strict tt then Vbot else Vtop
+      then if va_strict tt then Vbot else ntop
       else I (Int.divs i1 i2)
-  | _, _ => Vtop
+  | _, _ => ntop2 v w
   end.
 
 Lemma divs_sound:
@@ -911,9 +1622,9 @@ Definition divu (v w: aval) :=
   match w, v with
   | I i2, I i1 =>
       if Int.eq i2 Int.zero
-       then if va_strict tt then Vbot else Vtop
+       then if va_strict tt then Vbot else ntop
       else I (Int.divu i1 i2)
-  | _, _ => Vtop
+  | _, _ => ntop2 v w
   end.
 
 Lemma divu_sound:
@@ -929,9 +1640,9 @@ Definition mods (v w: aval) :=
   | I i2, I i1 =>
       if Int.eq i2 Int.zero
       || Int.eq i1 (Int.repr Int.min_signed) && Int.eq i2 Int.mone
-      then if va_strict tt then Vbot else Vtop
+      then if va_strict tt then Vbot else ntop
       else I (Int.mods i1 i2)
-  | _, _ => Vtop
+  | _, _ => ntop2 v w
   end.
 
 Lemma mods_sound:
@@ -947,10 +1658,10 @@ Definition modu (v w: aval) :=
   match w, v with
   | I i2, I i1 =>
       if Int.eq i2 Int.zero
-      then if va_strict tt then Vbot else Vtop
+      then if va_strict tt then Vbot else ntop
       else I (Int.modu i1 i2)
-  | I i2, _ => uns (usize i2)
-  | _, _ => Vtop
+  | I i2, _ => uns (provenance v) (usize i2)
+  | _, _ => ntop2 v w
   end.
 
 Lemma modu_sound:
@@ -974,8 +1685,8 @@ Qed.
 
 Definition shrx (v w: aval) :=
   match v, w with
-  | I i, I j => if Int.ltu j (Int.repr 31) then I(Int.shrx i j) else Vtop
-  | _, _ => Vtop
+  | I i, I j => if Int.ltu j (Int.repr 31) then I(Int.shrx i j) else ntop
+  | _, _ => ntop1 v
   end.
 
 Lemma shrx_sound:
@@ -996,10 +1707,10 @@ Definition shift_long (sem: int64 -> int -> int64) (v w: aval) :=
       if Int.ltu amount Int64.iwordsize' then
         match v with
         | L i => L (sem i amount)
-        | _ => Vtop
+        | _ => ntop1 v
         end
-      else Vtop
-  | _ => Vtop
+      else ntop1 v
+  | _ => ntop1 v
   end.
 
 Lemma shift_long_sound:
@@ -1017,9 +1728,9 @@ Proof.
             | Vlong i, Vint j => if Int.ltu j Int64.iwordsize'
                                  then Vlong (sem i j) else Vundef
             | _, _ => Vundef end)
-           Vtop).
+           (ntop1 x)).
   { destruct v; try constructor; destruct w; try constructor.
-  }    
+    destruct (Int.ltu i0 Int64.iwordsize'); constructor. }
   unfold shift_long. destruct y; auto.
   destruct (Int.ltu n Int64.iwordsize') eqn:LT; auto.
   destruct x; auto.
@@ -1071,7 +1782,7 @@ Proof (unop_long_sound Int64.not).
 Definition rotate_long (sem: int64 -> int64 -> int64) (v w: aval) :=
   match v, w with
   | L i, I amount => L (sem i (Int64.repr (Int.unsigned amount)))
-  | _, _ => Vtop
+  | _, _ => ntop1 v
   end.
 
 Lemma rotate_long_sound:
@@ -1087,8 +1798,8 @@ Proof.
     vmatch (match v, w with
             | Vlong i, Vint j => Vlong (sem i (Int64.repr (Int.unsigned j)))
             | _, _ => Vundef end)
-           Vtop).
-  { destruct v; try constructor. }
+           (ntop1 x)).
+  { destruct v; try constructor. destruct w; constructor. }
   unfold rotate_long. destruct x; auto. destruct y; auto. inv H; inv H0. constructor.
 Qed.
 
@@ -1113,7 +1824,12 @@ Proof (unop_long_sound Int64.neg).
 Definition addl (x y: aval) :=
   match x, y with
   | L i, L j => L (Int64.add i j)
-  | _, _ => Vtop
+  | Ptr p, L i | L i, Ptr p => Ptr (if Archi.ptr64 then padd p (Ptrofs.of_int64 i) else poffset p)
+  | Ptr p, _   | _, Ptr p   => Ptr (poffset p)
+  | Ifptr p, L i | L i, Ifptr p => Ifptr (if Archi.ptr64 then padd p (Ptrofs.of_int64 i) else poffset p)
+  | Ifptr p, Ifptr q => Ifptr (plub (poffset p) (poffset q))
+  | Ifptr p, _ | _, Ifptr p => Ifptr (poffset p)
+  | _, _ => ntop2 x y
   end.
 
 Lemma addl_sound:
@@ -1122,20 +1838,26 @@ Proof.
   intros. unfold Val.addl, addl. destruct Archi.ptr64.
 - inv H; inv H0; constructor;
   ((apply padd_sound; assumption) || (eapply poffset_sound; eassumption) || idtac).
+  apply pmatch_lub_r. eapply poffset_sound; eauto.
+  apply pmatch_lub_l. eapply poffset_sound; eauto.
 - inv H; inv H0; constructor.
 Qed.
 
 Definition subl (v w: aval) :=
   match v, w with
   | L i1, L i2 => L (Int64.sub i1 i2)
-  | _, _ => Vtop
+  | Ptr p, L i => if Archi.ptr64 then Ptr (psub p (Ptrofs.of_int64 i)) else Ifptr (poffset p)
+  | Ptr p, _   => Ifptr (poffset p)
+  | Ifptr p, L i => if Archi.ptr64 then Ifptr (psub p (Ptrofs.of_int64 i)) else Ifptr (plub (poffset p) (provenance w))
+  | Ifptr p, _ => Ifptr (plub (poffset p) (provenance w))
+  | _, _ => ntop2 v w
   end.
 
 Lemma subl_sound:
   forall v w x y, vmatch v x -> vmatch w y -> vmatch (Val.subl v w) (subl x y).
 Proof.
   intros. unfold Val.subl, subl. destruct Archi.ptr64.
-- inv H; inv H0; try (destruct (eq_block b b0)); eauto with va.
+- inv H; inv H0; try (destruct (eq_block b b0)); eauto using psub_sound, poffset_sound, pmatch_lub_l with va.
 - inv H; inv H0; eauto with va.
 Qed.
 
@@ -1162,9 +1884,9 @@ Definition divls (v w: aval) :=
   | L i2, L i1 =>
       if Int64.eq i2 Int64.zero
       || Int64.eq i1 (Int64.repr Int64.min_signed) && Int64.eq i2 Int64.mone
-      then if va_strict tt then Vbot else Vtop
+      then if va_strict tt then Vbot else ntop
       else L (Int64.divs i1 i2)
-  | _, _ => Vtop
+  | _, _ => ntop2 v w
   end.
 
 Lemma divls_sound:
@@ -1180,9 +1902,9 @@ Definition divlu (v w: aval) :=
   match w, v with
   | L i2, L i1 =>
       if Int64.eq i2 Int64.zero
-       then if va_strict tt then Vbot else Vtop
+       then if va_strict tt then Vbot else ntop
       else L (Int64.divu i1 i2)
-  | _, _ => Vtop
+  | _, _ => ntop2 v w
   end.
 
 Lemma divlu_sound:
@@ -1198,9 +1920,9 @@ Definition modls (v w: aval) :=
   | L i2, L i1 =>
       if Int64.eq i2 Int64.zero
       || Int64.eq i1 (Int64.repr Int64.min_signed) && Int64.eq i2 Int64.mone
-      then if va_strict tt then Vbot else Vtop
+      then if va_strict tt then Vbot else ntop
       else L (Int64.mods i1 i2)
-  | _, _ => Vtop
+  | _, _ => ntop2 v w
   end.
 
 Lemma modls_sound:
@@ -1216,9 +1938,9 @@ Definition modlu (v w: aval) :=
   match w, v with
   | L i2, L i1 =>
       if Int64.eq i2 Int64.zero
-      then if va_strict tt then Vbot else Vtop
+      then if va_strict tt then Vbot else ntop
       else L (Int64.modu i1 i2)
-  | _, _ => Vtop
+  | _, _ => ntop2 v w
   end.
 
 Lemma modlu_sound:
@@ -1231,8 +1953,8 @@ Qed.
 
 Definition shrxl (v w: aval) :=
   match v, w with
-  | L i, I j => if Int.ltu j (Int.repr 63) then L(Int64.shrx' i j) else Vtop
-  | _, _ => Vtop
+  | L i, I j => if Int.ltu j (Int.repr 63) then L(Int64.shrx' i j) else ntop
+  | _, _ => ntop1 v
   end.
 
 Lemma shrxl_sound:
@@ -1256,6 +1978,22 @@ Proof.
   replace (Val.rolml v amount mask) with (Val.andl (Val.roll v (Vint amount)) (Vlong mask)).
   apply andl_sound. apply roll_sound. auto. constructor. constructor.
   destruct v; auto.
+Qed.
+
+(** Pointer operations *)
+
+Definition offset_ptr (v: aval) (n: ptrofs) :=
+  match v with
+  | Ptr p => Ptr (padd p n)
+  | Ifptr p => Ifptr (padd p n)
+  | _ => ntop1 v
+  end.
+
+Lemma offset_ptr_sound:
+  forall v x n, vmatch v x -> vmatch (Val.offset_ptr v n) (offset_ptr x n).
+Proof.
+  intros. unfold Val.offset_ptr, offset_ptr.
+  inv H; constructor; apply padd_sound; assumption.
 Qed.
 
 (** Floating-point arithmetic operations *)
@@ -1337,8 +2075,8 @@ Proof (binop_single_sound Float32.div).
 Definition zero_ext (nbits: Z) (v: aval) :=
   match v with
   | I i => I (Int.zero_ext nbits i)
-  | Uns n => uns (Z.min n nbits)
-  | _ => uns nbits
+  | Uns p n => uns p (Z.min n nbits)
+  | _ => uns (provenance v) nbits
   end.
 
 Lemma zero_ext_sound:
@@ -1351,40 +2089,56 @@ Proof.
   intros. inv H; simpl; auto with va. apply vmatch_uns.
   red; intros. zify.
   rewrite Int.bits_zero_ext by omega.
-  destruct (zlt m nbits); auto with va.
-  destruct v ; auto with va.
-  simpl. auto with va.
+  destruct (zlt m nbits); auto. apply H1; omega.
 Qed.
 
 Definition sign_ext (nbits: Z) (v: aval) :=
+  if zle nbits 0 then Uns (provenance v) 0 else
   match v with
   | I i => I (Int.sign_ext nbits i)
-  | Uns n => if zlt n nbits then Uns n else sgn nbits
-  | Sgn n => sgn (Z.min n nbits)
-  | _ => sgn nbits
+  | Uns p n => if zlt n nbits then Uns p n else sgn p nbits
+  | Sgn p n => sgn p (Z.min n nbits)
+  | _ => sgn (provenance v) nbits
   end.
 
 Lemma sign_ext_sound:
-  forall nbits v x, 0 < nbits -> vmatch v x -> vmatch (Val.sign_ext nbits v) (sign_ext nbits x).
+  forall nbits v x, vmatch v x -> vmatch (Val.sign_ext nbits v) (sign_ext nbits x).
 Proof.
-  assert (DFL: forall nbits i, 0 < nbits -> vmatch (Vint (Int.sign_ext nbits i)) (sgn nbits)).
+  assert (DFL: forall p nbits i, 0 < nbits -> vmatch (Vint (Int.sign_ext nbits i)) (sgn p nbits)).
   {
     intros. apply vmatch_sgn. apply is_sign_ext_sgn; auto with va.
   }
-  intros. inv H0; simpl; auto with va.
-- destruct (zlt n nbits); eauto with va.
+  intros. unfold sign_ext. destruct (zle nbits 0).
+- destruct v; simpl; auto with va. constructor. omega. 
+  rewrite Int.sign_ext_below by auto. red; intros; apply Int.bits_zero.
+- inv H; simpl; auto with va.
++ destruct (zlt n nbits); eauto with va.
   constructor; auto. eapply is_sign_ext_uns; eauto with va.
-- destruct (zlt n nbits); auto with va.
-- apply vmatch_sgn. apply is_sign_ext_sgn; auto with va.
++ destruct (zlt n nbits); auto with va.
++ apply vmatch_sgn. apply is_sign_ext_sgn; auto with va.
   apply Z.min_case; auto with va.
-- destruct v ; auto with va.
-  simpl. auto with va.
+Qed.
+
+Definition zero_ext_l (s: Z) := unop_long (Int64.zero_ext s).
+
+Lemma zero_ext_l_sound:
+  forall s v x, vmatch v x -> vmatch (Val.zero_ext_l s v) (zero_ext_l s x).
+Proof.
+  intros s. exact (unop_long_sound (Int64.zero_ext s)).
+Qed.
+
+Definition sign_ext_l (s: Z) := unop_long (Int64.sign_ext s).
+
+Lemma sign_ext_l_sound:
+  forall s v x, vmatch v x -> vmatch (Val.sign_ext_l s v) (sign_ext_l s x).
+Proof.
+  intros s. exact (unop_long_sound (Int64.sign_ext s)).
 Qed.
 
 Definition longofint (v: aval) :=
   match v with
   | I i => L (Int64.repr (Int.signed i))
-  | _ => Vtop
+  | _ => ntop1 v
   end.
 
 Lemma longofint_sound:
@@ -1396,7 +2150,7 @@ Qed.
 Definition longofintu (v: aval) :=
   match v with
   | I i => L (Int64.repr (Int.unsigned i))
-  | _ => Vtop
+  | _ => ntop1 v
   end.
 
 Lemma longofintu_sound:
@@ -1408,30 +2162,30 @@ Qed.
 Definition singleoffloat (v: aval) :=
   match v with
   | F f => FS (Float.to_single f)
-  | _   => Vtop
+  | _   => ntop1 v
   end.
 
 Lemma singleoffloat_sound:
   forall v x, vmatch v x -> vmatch (Val.singleoffloat v) (singleoffloat x).
 Proof.
   intros.
-  assert (DEFAULT: vmatch (Val.singleoffloat v) Vtop).
-  { constructor. }
+  assert (DEFAULT: vmatch (Val.singleoffloat v) (ntop1 x)).
+  { destruct v; constructor. }
   destruct x; auto. inv H. constructor.
 Qed.
 
 Definition floatofsingle (v: aval) :=
   match v with
   | FS f => F (Float.of_single f)
-  | _   => Vtop
+  | _   => ntop1 v
   end.
 
 Lemma floatofsingle_sound:
   forall v x, vmatch v x -> vmatch (Val.floatofsingle v) (floatofsingle x).
 Proof.
   intros.
-  assert (DEFAULT: vmatch (Val.floatofsingle v) Vtop).
-  { constructor. }
+  assert (DEFAULT: vmatch (Val.floatofsingle v) (ntop1 x)).
+  { destruct v; constructor. }
   destruct x; auto. inv H. constructor.
 Qed.
 
@@ -1440,9 +2194,9 @@ Definition intoffloat (x: aval) :=
   | F f =>
       match Float.to_int f with
       | Some i => I i
-      | None => if va_strict tt then Vbot else Vtop
+      | None => if va_strict tt then Vbot else ntop
       end
-  | _ => Vtop
+  | _ => ntop1 x
   end.
 
 Lemma intoffloat_sound:
@@ -1458,9 +2212,9 @@ Definition intuoffloat (x: aval) :=
   | F f =>
       match Float.to_intu f with
       | Some i => I i
-      | None => if va_strict tt then Vbot else Vtop
+      | None => if va_strict tt then Vbot else ntop
       end
-  | _ => Vtop
+  | _ => ntop1 x
   end.
 
 Lemma intuoffloat_sound:
@@ -1474,7 +2228,7 @@ Qed.
 Definition floatofint (x: aval) :=
   match x with
   | I i => F(Float.of_int i)
-  | _   => Vtop
+  | _   => ntop1 x
   end.
 
 Lemma floatofint_sound:
@@ -1487,7 +2241,7 @@ Qed.
 Definition floatofintu (x: aval) :=
   match x with
   | I i => F(Float.of_intu i)
-  | _   => Vtop
+  | _   => ntop1 x
   end.
 
 Lemma floatofintu_sound:
@@ -1502,9 +2256,9 @@ Definition intofsingle (x: aval) :=
   | FS f =>
       match Float32.to_int f with
       | Some i => I i
-      | None => if va_strict tt then Vbot else Vtop
+      | None => if va_strict tt then Vbot else ntop
       end
-  | _ => Vtop
+  | _ => ntop1 x
   end.
 
 Lemma intofsingle_sound:
@@ -1520,9 +2274,9 @@ Definition intuofsingle (x: aval) :=
   | FS f =>
       match Float32.to_intu f with
       | Some i => I i
-      | None => if va_strict tt then Vbot else Vtop
+      | None => if va_strict tt then Vbot else ntop
       end
-  | _ => Vtop
+  | _ => ntop1 x
   end.
 
 Lemma intuofsingle_sound:
@@ -1536,7 +2290,7 @@ Qed.
 Definition singleofint (x: aval) :=
   match x with
   | I i => FS(Float32.of_int i)
-  | _   => Vtop
+  | _   => ntop1 x
   end.
 
 Lemma singleofint_sound:
@@ -1549,7 +2303,7 @@ Qed.
 Definition singleofintu (x: aval) :=
   match x with
   | I i => FS(Float32.of_intu i)
-  | _   => Vtop
+  | _   => ntop1 x
   end.
 
 Lemma singleofintu_sound:
@@ -1564,9 +2318,9 @@ Definition longoffloat (x: aval) :=
   | F f =>
       match Float.to_long f with
       | Some i => L i
-      | None => if va_strict tt then Vbot else Vtop
+      | None => if va_strict tt then Vbot else ntop
       end
-  | _ => Vtop
+  | _ => ntop1 x
   end.
 
 Lemma longoffloat_sound:
@@ -1582,9 +2336,9 @@ Definition longuoffloat (x: aval) :=
   | F f =>
       match Float.to_longu f with
       | Some i => L i
-      | None => if va_strict tt then Vbot else Vtop
+      | None => if va_strict tt then Vbot else ntop
       end
-  | _ => Vtop
+  | _ => ntop1 x
   end.
 
 Lemma longuoffloat_sound:
@@ -1598,7 +2352,7 @@ Qed.
 Definition floatoflong (x: aval) :=
   match x with
   | L i => F(Float.of_long i)
-  | _   => Vtop
+  | _   => ntop1 x
   end.
 
 Lemma floatoflong_sound:
@@ -1611,7 +2365,7 @@ Qed.
 Definition floatoflongu (x: aval) :=
   match x with
   | L i => F(Float.of_longu i)
-  | _   => Vtop
+  | _   => ntop1 x
   end.
 
 Lemma floatoflongu_sound:
@@ -1626,9 +2380,9 @@ Definition longofsingle (x: aval) :=
   | FS f =>
       match Float32.to_long f with
       | Some i => L i
-      | None => if va_strict tt then Vbot else Vtop
+      | None => if va_strict tt then Vbot else ntop
       end
-  | _ => Vtop
+  | _ => ntop1 x
   end.
 
 Lemma longofsingle_sound:
@@ -1644,9 +2398,9 @@ Definition longuofsingle (x: aval) :=
   | FS f =>
       match Float32.to_longu f with
       | Some i => L i
-      | None => if va_strict tt then Vbot else Vtop
+      | None => if va_strict tt then Vbot else ntop
       end
-  | _ => Vtop
+  | _ => ntop1 x
   end.
 
 Lemma longuofsingle_sound:
@@ -1660,7 +2414,7 @@ Qed.
 Definition singleoflong (x: aval) :=
   match x with
   | L i => FS(Float32.of_long i)
-  | _   => Vtop
+  | _   => ntop1 x
   end.
 
 Lemma singleoflong_sound:
@@ -1673,7 +2427,7 @@ Qed.
 Definition singleoflongu (x: aval) :=
   match x with
   | L i => FS(Float32.of_longu i)
-  | _   => Vtop
+  | _   => ntop1 x
   end.
 
 Lemma singleoflongu_sound:
@@ -1686,7 +2440,7 @@ Qed.
 Definition floatofwords (x y: aval) :=
   match x, y with
   | I i, I j => F(Float.from_words i j)
-  | _, _     => Vtop
+  | _, _     => ntop2 x y
   end.
 
 Lemma floatofwords_sound:
@@ -1698,7 +2452,7 @@ Qed.
 Definition longofwords (x y: aval) :=
   match y, x with
   | I j, I i => L(Int64.ofwords i j)
-  | _, _     => Vtop
+  | _, _     => ntop2 x y
   end.
 
 Lemma longofwords_sound:
@@ -1710,7 +2464,7 @@ Qed.
 Definition loword (x: aval) :=
   match x with
   | L i => I(Int64.loword i)
-  | _   => Vtop
+  | _   => ntop1 x
   end.
 
 Lemma loword_sound: forall v x, vmatch v x -> vmatch (Val.loword v) (loword x).
@@ -1721,7 +2475,7 @@ Qed.
 Definition hiword (x: aval) :=
   match x with
   | L i => I(Int64.hiword i)
-  | _   => Vtop
+  | _   => ntop1 x
   end.
 
 Lemma hiword_sound: forall v x, vmatch v x -> vmatch (Val.hiword v) (hiword x).
@@ -1731,15 +2485,15 @@ Qed.
 
 (** Comparisons and variation intervals *)
 
-Definition cmp_intv (c: comparison) (i: Z * Z) (n: Z) : ValueDomain.abool :=
+Definition cmp_intv (c: comparison) (i: Z * Z) (n: Z) : abool :=
   let (lo, hi) := i in
   match c with
-  | Ceq => if zlt n lo || zlt hi n then ValueDomain.Maybe false else ValueDomain.Btop
-  | Cne => ValueDomain.Btop
-  | Clt => if zlt hi n then ValueDomain.Maybe true else if zle n lo then ValueDomain.Maybe false else ValueDomain.Btop
-  | Cle => if zle hi n then ValueDomain.Maybe true else if zlt n lo then ValueDomain.Maybe false else ValueDomain.Btop
-  | Cgt => if zlt n lo then ValueDomain.Maybe true else if zle hi n then ValueDomain.Maybe false else ValueDomain.Btop
-  | Cge => if zle n lo then ValueDomain.Maybe true else if zlt hi n then ValueDomain.Maybe false else ValueDomain.Btop
+  | Ceq => if zlt n lo || zlt hi n then Maybe false else Btop
+  | Cne => Btop
+  | Clt => if zlt hi n then Maybe true else if zle n lo then Maybe false else Btop
+  | Cle => if zle hi n then Maybe true else if zlt n lo then Maybe false else Btop
+  | Cgt => if zlt n lo then Maybe true else if zle hi n then Maybe false else Btop
+  | Cge => if zle n lo then Maybe true else if zlt hi n then Maybe false else Btop
   end.
 
 Definition zcmp (c: comparison) (n1 n2: Z) : bool :=
@@ -1755,7 +2509,7 @@ Definition zcmp (c: comparison) (n1 n2: Z) : bool :=
 Lemma zcmp_intv_sound:
   forall c i x n,
   fst i <= x <= snd i ->
-  ValueDomain.cmatch (Some (zcmp c x n)) (cmp_intv c i n).
+  cmatch (Some (zcmp c x n)) (cmp_intv c i n).
 Proof.
   intros c [lo hi] x n; simpl; intros R.
   destruct c; unfold zcmp, proj_sumbool.
@@ -1784,7 +2538,7 @@ Proof.
 Qed.
 
 Lemma cmp_intv_None:
-  forall c i n, ValueDomain.cmatch None (cmp_intv c i n).
+  forall c i n, cmatch None (cmp_intv c i n).
 Proof.
   unfold cmp_intv; intros. destruct i as [lo hi].
   destruct c.
@@ -1805,7 +2559,7 @@ Qed.
 Definition uintv (v: aval) : Z * Z :=
   match v with
   | I n => (Int.unsigned n, Int.unsigned n)
-  | Uns n => if zlt n Int.zwordsize then (0, two_p n - 1) else (0, Int.max_unsigned)
+  | Uns _ n => if zlt n Int.zwordsize then (0, two_p n - 1) else (0, Int.max_unsigned)
   | _ => (0, Int.max_unsigned)
   end.
 
@@ -1823,7 +2577,7 @@ Qed.
 Lemma cmpu_intv_sound:
   forall valid c n1 v1 n2,
   vmatch (Vint n1) v1 ->
-  ValueDomain.cmatch (Val.cmpu_bool valid c (Vint n1) (Vint n2)) (cmp_intv c (uintv v1) (Int.unsigned n2)).
+  cmatch (Val.cmpu_bool valid c (Vint n1) (Vint n2)) (cmp_intv c (uintv v1) (Int.unsigned n2)).
 Proof.
   intros. simpl. replace (Int.cmpu c n1 n2) with (zcmp c (Int.unsigned n1) (Int.unsigned n2)).
   apply zcmp_intv_sound; apply uintv_sound; auto.
@@ -1835,7 +2589,7 @@ Qed.
 Lemma cmpu_intv_sound_2:
   forall valid c n1 v1 n2,
   vmatch (Vint n1) v1 ->
-  ValueDomain.cmatch (Val.cmpu_bool valid c (Vint n2) (Vint n1)) (cmp_intv (swap_comparison c) (uintv v1) (Int.unsigned n2)).
+  cmatch (Val.cmpu_bool valid c (Vint n2) (Vint n1)) (cmp_intv (swap_comparison c) (uintv v1) (Int.unsigned n2)).
 Proof.
   intros. rewrite <- Val.swap_cmpu_bool. apply cmpu_intv_sound; auto.
 Qed.
@@ -1843,9 +2597,9 @@ Qed.
 Definition sintv (v: aval) : Z * Z :=
   match v with
   | I n => (Int.signed n, Int.signed n)
-  | Uns n =>
+  | Uns _ n =>
       if zlt n Int.zwordsize then (0, two_p n - 1) else (Int.min_signed, Int.max_signed)
-  | Sgn n =>
+  | Sgn _ n =>
       if zlt n Int.zwordsize
       then (let x := two_p (n-1) in (-x, x-1))
       else (Int.min_signed, Int.max_signed)
@@ -1878,7 +2632,7 @@ Qed.
 Lemma cmp_intv_sound:
   forall c n1 v1 n2,
   vmatch (Vint n1) v1 ->
-  ValueDomain.cmatch (Val.cmp_bool c (Vint n1) (Vint n2)) (cmp_intv c (sintv v1) (Int.signed n2)).
+  cmatch (Val.cmp_bool c (Vint n1) (Vint n2)) (cmp_intv c (sintv v1) (Int.signed n2)).
 Proof.
   intros. simpl. replace (Int.cmp c n1 n2) with (zcmp c (Int.signed n1) (Int.signed n2)).
   apply zcmp_intv_sound; apply sintv_sound; auto.
@@ -1890,124 +2644,161 @@ Qed.
 Lemma cmp_intv_sound_2:
   forall c n1 v1 n2,
   vmatch (Vint n1) v1 ->
-  ValueDomain.cmatch (Val.cmp_bool c (Vint n2) (Vint n1)) (cmp_intv (swap_comparison c) (sintv v1) (Int.signed n2)).
+  cmatch (Val.cmp_bool c (Vint n2) (Vint n1)) (cmp_intv (swap_comparison c) (sintv v1) (Int.signed n2)).
 Proof.
   intros. rewrite <- Val.swap_cmp_bool. apply cmp_intv_sound; auto.
 Qed.
 
 (** Comparisons *)
-Definition cmpu_bool (c: comparison) (v w: aval) : ValueDomain.abool :=
+
+Definition cmpu_bool (c: comparison) (v w: aval) : abool :=
   match v, w with
-  | I i1, I i2 => ValueDomain.Just (Int.cmpu c i1 i2)
-  | _, I i => ValueDomain.club (cmp_intv c (uintv v) (Int.unsigned i)) (ValueDomain.cmp_different_blocks c)
-  | I i, _ => ValueDomain.club (cmp_intv (swap_comparison c) (uintv w) (Int.unsigned i)) (ValueDomain.cmp_different_blocks c)
-  | _, _ => ValueDomain.Btop
+  | I i1, I i2 => Just (Int.cmpu c i1 i2)
+  | Ptr _, I i => if Int.eq i Int.zero then cmp_different_blocks c else Btop
+  | I i, Ptr _ => if Int.eq i Int.zero then cmp_different_blocks c else Btop
+  | Ptr p1, Ptr p2 => pcmp c p1 p2
+  | _, I i => club (cmp_intv c (uintv v) (Int.unsigned i)) (cmp_different_blocks c)
+  | I i, _ => club (cmp_intv (swap_comparison c) (uintv w) (Int.unsigned i)) (cmp_different_blocks c)
+  | _, _ => Btop
   end.
 
 Lemma cmpu_bool_sound:
-  forall valid c v w x y,
-    vmatch v x ->
-    vmatch w y ->
-    ValueDomain.cmatch (Val.cmpu_bool valid c v w) (cmpu_bool c x y).
+  forall valid c v w x y, vmatch v x -> vmatch w y -> cmatch (Val.cmpu_bool valid c v w) (cmpu_bool c x y).
 Proof.
   intros.
+  assert (IP: forall i b ofs,
+    cmatch (Val.cmpu_bool valid c (Vint i) (Vptr b ofs)) (cmp_different_blocks c)).
+  {
+    intros. simpl. destruct Archi.ptr64.
+    apply cmp_different_blocks_none.
+    destruct (Int.eq i Int.zero && (valid b (Ptrofs.unsigned ofs) || valid b (Ptrofs.unsigned ofs - 1))).
+    apply cmp_different_blocks_sound. apply cmp_different_blocks_none.
+  }
+  assert (PI: forall i b ofs,
+    cmatch (Val.cmpu_bool valid c (Vptr b ofs) (Vint i)) (cmp_different_blocks c)).
+  {
+    intros. simpl. destruct Archi.ptr64.
+    apply cmp_different_blocks_none.
+    destruct (Int.eq i Int.zero && (valid b (Ptrofs.unsigned ofs) || valid b (Ptrofs.unsigned ofs - 1))).
+    apply cmp_different_blocks_sound. apply cmp_different_blocks_none.
+  }
   unfold cmpu_bool; inversion H; subst; inversion H0; subst;
-    try (destruct w ) ;
-    try (destruct v ) ;
-    eauto using ValueDomain.cmatch_top, ValueDomain.cmp_different_blocks_none,
-    ValueDomain.pcmp_none,
-    ValueDomain.cmatch_lub_l, ValueDomain.cmatch_lub_r,
-    MATCH.cmpu_intv_sound, MATCH.cmpu_intv_sound_2, MATCH.cmp_intv_None with va.
-  - constructor.
+  auto using cmatch_top, cmp_different_blocks_none, pcmp_none,
+             cmatch_lub_l, cmatch_lub_r, pcmp_sound,
+             cmpu_intv_sound, cmpu_intv_sound_2, cmp_intv_None.
+- constructor.
+- destruct (Int.eq i Int.zero); auto using cmatch_top.
+- simpl; destruct (Int.eq i Int.zero); auto using cmatch_top, cmp_different_blocks_none.
+- destruct (Int.eq i Int.zero); auto using cmatch_top.
+- simpl; destruct (Int.eq i Int.zero); auto using cmatch_top, cmp_different_blocks_none.
 Qed.
 
-Definition cmp_bool (c: comparison) (v w: aval) : ValueDomain.abool :=
+Definition cmp_bool (c: comparison) (v w: aval) : abool :=
   match v, w with
-  | I i1, I i2 => ValueDomain.Just (Int.cmp c i1 i2)
+  | I i1, I i2 => Just (Int.cmp c i1 i2)
   | _, I i => cmp_intv c (sintv v) (Int.signed i)
   | I i, _ => cmp_intv (swap_comparison c) (sintv w) (Int.signed i)
-  | _, _ => ValueDomain.Btop
+  | _, _ => Btop
   end.
 
 Lemma cmp_bool_sound:
-  forall c v w x y, vmatch v x -> vmatch w y -> ValueDomain.cmatch (Val.cmp_bool c v w) (cmp_bool c x y).
+  forall c v w x y, vmatch v x -> vmatch w y -> cmatch (Val.cmp_bool c v w) (cmp_bool c x y).
 Proof.
   intros.
   unfold cmp_bool; inversion H; subst; inversion H0; subst;
-   try (destruct w ) ;
-   try (destruct v ) ;  
-  auto using ValueDomain.cmatch_top, cmp_intv_sound, cmp_intv_sound_2, cmp_intv_None.
+  auto using cmatch_top, cmp_intv_sound, cmp_intv_sound_2, cmp_intv_None.
 - constructor.
 Qed.
 
-Definition cmplu_bool (c: comparison) (v w: aval) : ValueDomain.abool :=
+Definition cmplu_bool (c: comparison) (v w: aval) : abool :=
   match v, w with
-  | L i1, L i2 => ValueDomain.Just (Int64.cmpu c i1 i2)
-  | _, _ => ValueDomain.Btop
+  | L i1, L i2 => Just (Int64.cmpu c i1 i2)
+  | Ptr _, L i => if Int64.eq i Int64.zero then cmp_different_blocks c else Btop
+  | L i, Ptr _ => if Int64.eq i Int64.zero then cmp_different_blocks c else Btop
+  | Ptr p1, Ptr p2 => pcmp c p1 p2
+  | _, _ => Btop
   end.
 
 Lemma cmplu_bool_sound:
-  forall valid c v w x y, vmatch v x -> vmatch w y -> ValueDomain.cmatch (Val.cmplu_bool valid c v w) (cmplu_bool c x y).
+  forall valid c v w x y, vmatch v x -> vmatch w y -> cmatch (Val.cmplu_bool valid c v w) (cmplu_bool c x y).
 Proof.
   intros.
+  assert (IP: forall i b ofs,
+    cmatch (Val.cmplu_bool valid c (Vlong i) (Vptr b ofs)) (cmp_different_blocks c)).
+  {
+    intros. simpl. destruct Archi.ptr64; simpl.
+    destruct (Int64.eq i Int64.zero && (valid b (Ptrofs.unsigned ofs) || valid b (Ptrofs.unsigned ofs - 1))).
+    apply cmp_different_blocks_sound. apply cmp_different_blocks_none.
+    apply cmp_different_blocks_none.
+  }
+  assert (PI: forall i b ofs,
+    cmatch (Val.cmplu_bool valid c (Vptr b ofs) (Vlong i)) (cmp_different_blocks c)).
+  {
+    intros. simpl. destruct Archi.ptr64; simpl.
+    destruct (Int64.eq i Int64.zero && (valid b (Ptrofs.unsigned ofs) || valid b (Ptrofs.unsigned ofs - 1))).
+    apply cmp_different_blocks_sound. apply cmp_different_blocks_none.
+    apply cmp_different_blocks_none.
+  }
   unfold cmplu_bool; inversion H; subst; inversion H0; subst;
-    try (destruct w ) ;
-    try (destruct v ) ;
-    auto using ValueDomain.cmatch_top, 
-             ValueDomain.cmatch_lub_l, ValueDomain.cmatch_lub_r.
+  auto using cmatch_top, cmp_different_blocks_none, pcmp_none,
+             cmatch_lub_l, cmatch_lub_r, pcmp_sound_64.
 - constructor.
+- destruct (Int64.eq i Int64.zero); auto using cmatch_top.
+- simpl; destruct (Int64.eq i Int64.zero); auto using cmatch_top, cmp_different_blocks_none.
+- destruct (Int64.eq i Int64.zero); auto using cmatch_top.
+- simpl; destruct (Int64.eq i Int64.zero); auto using cmatch_top, cmp_different_blocks_none.
 Qed.
 
-Definition cmpl_bool (c: comparison) (v w: aval) : ValueDomain.abool :=
+Definition cmpl_bool (c: comparison) (v w: aval) : abool :=
   match v, w with
-  | L i1, L i2 => ValueDomain.Just (Int64.cmp c i1 i2)
-  | _, _ => ValueDomain.Btop
+  | L i1, L i2 => Just (Int64.cmp c i1 i2)
+  | _, _ => Btop
   end.
 
 Lemma cmpl_bool_sound:
-  forall c v w x y, vmatch v x -> vmatch w y -> ValueDomain.cmatch (Val.cmpl_bool c v w) (cmpl_bool c x y).
+  forall c v w x y, vmatch v x -> vmatch w y -> cmatch (Val.cmpl_bool c v w) (cmpl_bool c x y).
 Proof.
   intros.
   unfold cmpl_bool; inversion H; subst; inversion H0; subst;
-  auto using ValueDomain.cmatch_top.
+  auto using cmatch_top.
 - constructor.
 Qed.
 
-Definition cmpf_bool (c: comparison) (v w: aval) : ValueDomain.abool :=
+Definition cmpf_bool (c: comparison) (v w: aval) : abool :=
   match v, w with
-  | F f1, F f2 => ValueDomain.Just (Float.cmp c f1 f2)
-  | _, _ => ValueDomain.Btop
+  | F f1, F f2 => Just (Float.cmp c f1 f2)
+  | _, _ => Btop
   end.
 
 Lemma cmpf_bool_sound:
-  forall c v w x y, vmatch v x -> vmatch w y -> ValueDomain.cmatch (Val.cmpf_bool c v w) (cmpf_bool c x y).
+  forall c v w x y, vmatch v x -> vmatch w y -> cmatch (Val.cmpf_bool c v w) (cmpf_bool c x y).
 Proof.
   intros. inv H; try constructor; inv H0; constructor.
 Qed.
 
-Definition cmpfs_bool (c: comparison) (v w: aval) : ValueDomain.abool :=
+Definition cmpfs_bool (c: comparison) (v w: aval) : abool :=
   match v, w with
-  | FS f1, FS f2 => ValueDomain.Just (Float32.cmp c f1 f2)
-  | _, _ => ValueDomain.Btop
+  | FS f1, FS f2 => Just (Float32.cmp c f1 f2)
+  | _, _ => Btop
   end.
 
 Lemma cmpfs_bool_sound:
-  forall c v w x y, vmatch v x -> vmatch w y -> ValueDomain.cmatch (Val.cmpfs_bool c v w) (cmpfs_bool c x y).
+  forall c v w x y, vmatch v x -> vmatch w y -> cmatch (Val.cmpfs_bool c v w) (cmpfs_bool c x y).
 Proof.
   intros. inv H; try constructor; inv H0; constructor.
 Qed.
 
-Definition maskzero (x: aval) (mask: int) : ValueDomain.abool :=
+Definition maskzero (x: aval) (mask: int) : abool :=
   match x with
-  | I i => ValueDomain.Just (Int.eq (Int.and i mask) Int.zero)
-  | Uns n => if Int.eq (Int.zero_ext n mask) Int.zero then ValueDomain.Maybe true else ValueDomain.Btop
-  | _ => ValueDomain.Btop
+  | I i => Just (Int.eq (Int.and i mask) Int.zero)
+  | Uns p n => if Int.eq (Int.zero_ext n mask) Int.zero then Maybe true else Btop
+  | _ => Btop
   end.
 
 Lemma maskzero_sound:
   forall mask v x,
   vmatch v x ->
-  ValueDomain.cmatch (Val.maskzero_bool v mask) (maskzero x mask).
+  cmatch (Val.maskzero_bool v mask) (maskzero x mask).
 Proof.
   intros. inv H; simpl; auto with va.
   predSpec Int.eq Int.eq_spec (Int.zero_ext n mask) Int.zero; auto with va.
@@ -2019,17 +2810,17 @@ Proof.
   destruct (Int.eq (Int.zero_ext n mask) Int.zero); constructor.
 Qed.
 
-Definition of_optbool (ab: ValueDomain.abool) : aval :=
+Definition of_optbool (ab: abool) : aval :=
   match ab with
-  | ValueDomain.Just b => I (if b then Int.one else Int.zero)
-  | _ => Uns 1
+  | Just b => I (if b then Int.one else Int.zero)
+  | _ => Uns Pbot 1
   end.
 
 Lemma of_optbool_sound:
-  forall ob ab, ValueDomain.cmatch ob ab -> vmatch (Val.of_optbool ob) (of_optbool ab).
+  forall ob ab, cmatch ob ab -> vmatch (Val.of_optbool ob) (of_optbool ab).
 Proof.
   intros.
-  assert (DEFAULT: vmatch (Val.of_optbool ob) (Uns 1)).
+  assert (DEFAULT: vmatch (Val.of_optbool ob) (Uns Pbot 1)).
   {
     destruct ob; simpl; auto with va.
     destruct b; constructor; try omega.
@@ -2039,29 +2830,30 @@ Proof.
   inv H; auto. simpl. destruct b; constructor.
 Qed.
 
-Definition resolve_branch (ab: ValueDomain.abool) : option bool :=
+Definition resolve_branch (ab: abool) : option bool :=
   match ab with
-  | ValueDomain.Just b => Some b
-  | ValueDomain.Maybe b => Some b
+  | Just b => Some b
+  | Maybe b => Some b
   | _ => None
   end.
 
 Lemma resolve_branch_sound:
   forall b ab b',
-  ValueDomain.cmatch (Some b) ab -> resolve_branch ab = Some b' -> b' = b.
+  cmatch (Some b) ab -> resolve_branch ab = Some b' -> b' = b.
 Proof.
   intros. inv H; simpl in H0; congruence.
 Qed.
 
 (** Select either returns one of its arguments, or Vundef. *)
+
 Definition add_undef (x: aval) :=
   match x with
-  | Vbot => Vtop
+  | Vbot => ntop
   | I i =>
       if Int.lt i Int.zero
-      then sgn (ssize i)
-      else uns (usize i)
-  | L _ | F _ | FS _ => Vtop
+      then sgn Pbot (ssize i)
+      else uns Pbot (usize i)
+  | L _ | F _ | FS _ => ntop
   | _ => x
   end.
 
@@ -2090,7 +2882,7 @@ Qed.
 
 Definition select (ab: abool) (x y: aval) :=
   match ab with
-  | Bnone => Vtop
+  | Bnone => ntop
   | Just b | Maybe b => add_undef (if b then x else y)
   | Btop => add_undef (vlub x y)
   end.
@@ -2116,27 +2908,30 @@ Definition vnormalize (chunk: memory_chunk) (v: aval) :=
   match chunk, v with
   | _, Vbot => Vbot
   | Mint8signed, I i => I (Int.sign_ext 8 i)
-  | Mint8signed, Uns n => if zlt n 8 then Uns n else Sgn 8
-  | Mint8signed, Sgn n => Sgn (Z.min n 8)
-  | Mint8signed, _ => Sgn 8
+  | Mint8signed, Uns p n => if zlt n 8 then Uns (provenance v) n else Sgn (provenance v) 8
+  | Mint8signed, Sgn p n => Sgn (provenance v) (Z.min n 8)
+  | Mint8signed, _ => Sgn (provenance v) 8
   | Mint8unsigned, I i => I (Int.zero_ext 8 i)
-  | Mint8unsigned, Uns n => Uns  (Z.min n 8)
-  | Mint8unsigned, _ => Uns  8
+  | Mint8unsigned, Uns p n => Uns (provenance v) (Z.min n 8)
+  | Mint8unsigned, _ => Uns (provenance v) 8
   | Mint16signed, I i => I (Int.sign_ext 16 i)
-  | Mint16signed, Uns n => if zlt n 16 then Uns  n else Sgn  16
-  | Mint16signed, Sgn n => Sgn  (Z.min n 16)
-  | Mint16signed, _ => Sgn 16
+  | Mint16signed, Uns p n => if zlt n 16 then Uns (provenance v) n else Sgn (provenance v) 16
+  | Mint16signed, Sgn p n => Sgn (provenance v) (Z.min n 16)
+  | Mint16signed, _ => Sgn (provenance v) 16
   | Mint16unsigned, I i => I (Int.zero_ext 16 i)
-  | Mint16unsigned, Uns n => Uns  (Z.min n 16)
-  | Mint16unsigned, _ => Uns  16
-  | Mint32, (I _ | Uns _ | Sgn _ ) => v
-  | Mint64, (L _ ) => v
-  | Mint64, (Uns _ | Sgn _) => Vtop
+  | Mint16unsigned, Uns p n => Uns (provenance v) (Z.min n 16)
+  | Mint16unsigned, _ => Uns (provenance v) 16
+  | Mint32, (I _ | Uns _ _ | Sgn _ _ | Ifptr _) => v
+  | Mint32, Ptr p => if Archi.ptr64 then Ifptr p else v
+  | Mint64, (L _ | Ifptr _) => v
+  | Mint64, (Uns p _ | Sgn p _) => Ifptr p
+  | Mint64, Ptr p => if Archi.ptr64 then v else Ifptr p
   | Mfloat32, FS f => v
   | Mfloat64, F f => v
-  | Many32, (I _ | Uns _ | Sgn _ | FS _ ) => v
+  | Many32, (I _ | Uns _ _ | Sgn _ _ | FS _ | Ifptr _) => v
+  | Many32, Ptr p => if Archi.ptr64 then Ifptr p else v
   | Many64, _ => v
-  | _, _ => Vtop
+  | _, _ => Ifptr (provenance v)
   end.
 
 Lemma vnormalize_sound:
@@ -2158,18 +2953,1542 @@ Proof.
 - constructor. omega. apply is_zero_ext_uns; auto with va.
 - constructor. xomega. apply is_sign_ext_sgn; auto with va. apply Z.min_case; auto with va.
 - constructor. omega. apply is_zero_ext_uns; auto with va.
-- destruct v ; auto with va.
-  constructor.
-  omega. apply is_sign_ext_sgn; auto with va.
-- destruct v ; auto with va.
-  constructor. omega. apply is_zero_ext_uns; auto with va.
-- destruct v ; auto with va.
-  constructor. omega. apply is_sign_ext_sgn; auto with va.
-- destruct v ; auto with va.
-  constructor. omega. apply is_zero_ext_uns; auto with va.
+- destruct ptr64; auto with va.
+- destruct ptr64; auto with va.
+- destruct ptr64; auto with va.
+- destruct ptr64; auto with va.
+- destruct ptr64; auto with va.
+- destruct ptr64; auto with va.
+- constructor. omega. apply is_sign_ext_sgn; auto with va.
+- constructor. omega. apply is_zero_ext_uns; auto with va.
+- constructor. omega. apply is_sign_ext_sgn; auto with va.
+- constructor. omega. apply is_zero_ext_uns; auto with va.
+- destruct ptr64; auto with va.
+- destruct ptr64; auto with va.
+- destruct ptr64; auto with va.
+Qed.
+
+Lemma vnormalize_cast:
+  forall chunk m b ofs v p,
+  Mem.load chunk m b ofs = Some v ->
+  vmatch v (Ifptr p) ->
+  vmatch v (vnormalize chunk (Ifptr p)).
+Proof.
+  intros. exploit Mem.load_cast; eauto. exploit Mem.load_type; eauto.
+  destruct chunk; simpl; intros.
+- (* int8signed *)
+  rewrite H2. destruct v; simpl; constructor. omega. apply is_sign_ext_sgn; auto with va.
+- (* int8unsigned *)
+  rewrite H2. destruct v; simpl; constructor. omega. apply is_zero_ext_uns; auto with va.
+- (* int16signed *)
+  rewrite H2. destruct v; simpl; constructor. omega. apply is_sign_ext_sgn; auto with va.
+- (* int16unsigned *)
+  rewrite H2. destruct v; simpl; constructor. omega. apply is_zero_ext_uns; auto with va.
+- (* int32 *)
+  auto.
+- (* int64 *)
+  auto.
+- (* float32 *)
+  destruct v; try contradiction; constructor.
+- (* float64 *)
+  destruct v; try contradiction; constructor.
+- (* any32 *)
+  destruct Archi.ptr64; auto.
+- (* any64 *)
+  auto.
+Qed.
+
+Remark poffset_monotone:
+  forall p q, pge p q -> pge (poffset p) (poffset q).
+Proof.
+  destruct 1; simpl; auto with va.
+Qed.
+
+Remark provenance_monotone:
+  forall x y, vge x y -> pge (provenance x) (provenance y).
+Proof.
+  unfold provenance; intros. destruct (va_strict tt). constructor.
+  inv H; auto using poffset_monotone with va.
+Qed.
+
+Lemma vnormalize_monotone:
+  forall chunk x y,
+  vge x y -> vge (vnormalize chunk x) (vnormalize chunk y).
+Proof with (auto using provenance_monotone with va).
+  intros chunk x y V; unfold vnormalize; generalize Archi.ptr64; intro ptr64; inversion V; subst; destruct chunk eqn:C; simpl...
+- destruct (zlt n 8); constructor...
+  apply is_sign_ext_uns...
+  apply is_sign_ext_sgn...
+- constructor... apply is_zero_ext_uns... apply Z.min_case...
+- destruct (zlt n 16); constructor...
+  apply is_sign_ext_uns...
+  apply is_sign_ext_sgn...
+- constructor... apply is_zero_ext_uns... apply Z.min_case...
+- unfold provenance; destruct (va_strict tt)...
+- destruct (zlt n1 8). rewrite zlt_true by omega...
+  destruct (zlt n2 8)...
+- destruct (zlt n1 16). rewrite zlt_true by omega...
+  destruct (zlt n2 16)...
+- constructor... apply is_sign_ext_sgn... apply Z.min_case...
+- constructor... apply is_zero_ext_uns...
+- constructor... apply is_sign_ext_sgn... apply Z.min_case...
+- constructor... apply is_zero_ext_uns...
+- unfold provenance; destruct (va_strict tt)...
+- destruct (zlt n2 8); constructor...
+- destruct (zlt n2 16); constructor...
+- destruct ptr64...
+- destruct ptr64...
+- destruct ptr64...
+- destruct ptr64...
+- destruct ptr64...
+- destruct ptr64...
+- constructor... apply is_sign_ext_sgn...
+- constructor... apply is_zero_ext_uns...
+- constructor... apply is_sign_ext_sgn...
+- constructor... apply is_zero_ext_uns...
+- unfold provenance; destruct (va_strict tt)...
+- unfold provenance; destruct (va_strict tt)...
+- unfold provenance; destruct (va_strict tt)...
+- unfold provenance; destruct (va_strict tt)...
+- unfold provenance; destruct (va_strict tt)...
+- unfold provenance; destruct (va_strict tt)...
+- unfold provenance; destruct (va_strict tt)...
+- unfold provenance; destruct (va_strict tt)...
+- destruct (zlt n 8)...
+- destruct (zlt n 16)...
+Qed.
+
+(** Analysis of known builtin functions.  All we have is a dynamic semantics
+  as a function [list val -> option val], but we can still perform 
+  some constant propagation. *)
+
+Definition val_of_aval (a: aval) : val :=
+  match a with
+  | I n => Vint n
+  | L n => Vlong n
+  | F f => Vfloat f
+  | FS f => Vsingle f
+  | _ => Vundef
+  end.
+
+Definition aval_of_val (v: val) : option aval :=
+  match v with
+  | Vint n => Some (I n)
+  | Vlong n => Some (L n)
+  | Vfloat f => Some (F f)
+  | Vsingle f => Some (FS f)
+  | _ => None
+  end.
+
+Lemma val_of_aval_sound:
+  forall v a, vmatch v a -> Val.lessdef (val_of_aval a) v.
+Proof.
+  destruct 1; simpl; auto.
+Qed.
+
+Corollary list_val_of_aval_sound:
+  forall vl al, list_forall2 vmatch vl al -> Val.lessdef_list (map val_of_aval al) vl.
+Proof.
+  induction 1; simpl; constructor; auto using val_of_aval_sound.
+Qed.
+
+Lemma aval_of_val_sound:
+  forall v a, aval_of_val v = Some a -> vmatch v a. 
+Proof.
+  intros v a E; destruct v; simpl in E; inv E; constructor.
+Qed.
+
+(** * Abstracting memory blocks *)
+
+Inductive acontent : Type :=
+ | ACval (chunk: memory_chunk) (av: aval).
+
+Definition eq_acontent : forall (c1 c2: acontent), {c1=c2} + {c1<>c2}.
+Proof.
+  intros. generalize chunk_eq eq_aval. decide equality.
+Defined.
+
+Record ablock : Type := ABlock {
+  ab_contents: ZTree.t acontent;
+  ab_summary: aptr
+}.
+
+Local Notation "a ## b" := (ZTree.get b a) (at level 1).
+
+Definition ablock_init (p: aptr) : ablock :=
+  {| ab_contents := ZTree.empty _; ab_summary := p |}.
+
+Definition chunk_compat (chunk chunk': memory_chunk) : bool :=
+  match chunk, chunk' with
+  | (Mint8signed | Mint8unsigned), (Mint8signed | Mint8unsigned) => true
+  | (Mint16signed | Mint16unsigned), (Mint16signed | Mint16unsigned) => true
+  | Mint32, Mint32 => true
+  | Mfloat32, Mfloat32 => true
+  | Mint64, Mint64 => true
+  | Mfloat64, Mfloat64 => true
+  | Many32, Many32 => true
+  | Many64, Many64 => true
+  | _, _ => false
+  end.
+
+Definition ablock_load (chunk: memory_chunk) (ab: ablock) (i: Z) : aval :=
+  match ab.(ab_contents)##i with
+  | None => vnormalize chunk (Ifptr ab.(ab_summary))
+  | Some (ACval chunk' av) =>
+      if chunk_compat chunk chunk'
+      then vnormalize chunk av
+      else vnormalize chunk (Ifptr ab.(ab_summary))
+  end.
+
+Definition ablock_load_anywhere (chunk: memory_chunk) (ab: ablock) : aval :=
+  vnormalize chunk (Ifptr ab.(ab_summary)).
+
+Function inval_after (lo: Z) (hi: Z) (c: ZTree.t acontent) { wf (Zwf lo) hi } : ZTree.t acontent :=
+  if zle lo hi
+  then inval_after lo (hi - 1) (ZTree.remove hi c)
+  else c.
+Proof.
+  intros; red; omega.
+  apply Zwf_well_founded.
+Qed.
+
+Definition inval_if (hi: Z) (lo: Z) (c: ZTree.t acontent) :=
+  match c##lo with
+  | None => c
+  | Some (ACval chunk av) => if zle (lo + size_chunk chunk) hi then c else ZTree.remove lo c
+  end.
+
+Function inval_before (hi: Z) (lo: Z) (c: ZTree.t acontent) { wf (Zwf_up hi) lo } : ZTree.t acontent :=
+  if zlt lo hi
+  then inval_before hi (lo + 1) (inval_if hi lo c)
+  else c.
+Proof.
+  intros; red; omega.
+  apply Zwf_up_well_founded.
+Qed.
+
+Definition ablock_store (chunk: memory_chunk) (ab: ablock) (i: Z) (av: aval) : ablock :=
+  {| ab_contents :=
+       ZTree.set i (ACval chunk av)
+         (inval_before i (i - 7)
+            (inval_after (i + 1) (i + size_chunk chunk - 1) ab.(ab_contents)));
+     ab_summary :=
+       vplub av ab.(ab_summary) |}.
+
+Definition ablock_store_anywhere (chunk: memory_chunk) (ab: ablock) (av: aval) : ablock :=
+  ablock_init (vplub av ab.(ab_summary)).
+
+Definition ablock_loadbytes (ab: ablock) : aptr := ab.(ab_summary).
+
+Definition ablock_storebytes (ab: ablock) (p: aptr) (ofs: Z) (sz: Z) :=
+  {| ab_contents :=
+       inval_before ofs (ofs - 7)
+         (inval_after ofs (ofs + sz - 1) ab.(ab_contents));
+     ab_summary :=
+       plub p ab.(ab_summary) |}.
+
+Definition ablock_storebytes_anywhere (ab: ablock) (p: aptr) :=
+  ablock_init (plub p ab.(ab_summary)).
+
+Definition smatch (m: mem) (b: block) (p: aptr) : Prop :=
+  (forall chunk ofs v, Mem.load chunk m b ofs = Some v -> vmatch v (Ifptr p))
+/\(forall ofs b' ofs' q i, Mem.loadbytes m b ofs 1 = Some (Fragment (Vptr b' ofs') q i :: nil) -> pmatch b' ofs' p).
+
+Remark loadbytes_load_ext:
+  forall b m m',
+  (forall ofs n bytes, Mem.loadbytes m' b ofs n = Some bytes -> n >= 0 -> Mem.loadbytes m b ofs n = Some bytes) ->
+  forall chunk ofs v, Mem.load chunk m' b ofs = Some v -> Mem.load chunk m b ofs = Some v.
+Proof.
+  intros. exploit Mem.load_loadbytes; eauto. intros [bytes [A B]].
+  exploit Mem.load_valid_access; eauto. intros [C D].
+  subst v. apply Mem.loadbytes_load; auto. apply H; auto. generalize (size_chunk_pos chunk); omega.
+Qed.
+
+Lemma smatch_ext:
+  forall m b p m',
+  smatch m b p ->
+  (forall ofs n bytes, Mem.loadbytes m' b ofs n = Some bytes -> n >= 0 -> Mem.loadbytes m b ofs n = Some bytes) ->
+  smatch m' b p.
+Proof.
+  intros. destruct H. split; intros.
+  eapply H; eauto. eapply loadbytes_load_ext; eauto.
+  eapply H1; eauto. apply H0; eauto. omega.
+Qed.
+
+Lemma smatch_inv:
+  forall m b p m',
+  smatch m b p ->
+  (forall ofs n, n >= 0 -> Mem.loadbytes m' b ofs n = Mem.loadbytes m b ofs n) ->
+  smatch m' b p.
+Proof.
+  intros. eapply smatch_ext; eauto.
+  intros. rewrite <- H0; eauto.
+Qed.
+
+Lemma smatch_ge:
+  forall m b p q, smatch m b p -> pge q p -> smatch m b q.
+Proof.
+  intros. destruct H as [A B]. split; intros.
+  apply vmatch_ge with (Ifptr p); eauto with va.
+  apply pmatch_ge with p; eauto with va.
+Qed.
+
+Lemma In_loadbytes:
+  forall m b byte n ofs bytes,
+  Mem.loadbytes m b ofs n = Some bytes ->
+  In byte bytes ->
+  exists ofs', ofs <= ofs' < ofs + n /\ Mem.loadbytes m b ofs' 1 = Some(byte :: nil).
+Proof.
+  intros until n. pattern n.
+  apply well_founded_ind with (R := Zwf 0).
+- apply Zwf_well_founded.
+- intros sz REC ofs bytes LOAD IN.
+  destruct (zle sz 0).
+  + rewrite (Mem.loadbytes_empty m b ofs sz) in LOAD by auto.
+    inv LOAD. contradiction.
+  + exploit (Mem.loadbytes_split m b ofs 1 (sz - 1) bytes).
+    replace (1 + (sz - 1)) with sz by omega. auto.
+    omega.
+    omega.
+    intros (bytes1 & bytes2 & LOAD1 & LOAD2 & CONCAT).
+    subst bytes.
+    exploit Mem.loadbytes_length. eexact LOAD1. change (Z.to_nat 1) with 1%nat. intros LENGTH1.
+    rewrite in_app_iff in IN. destruct IN.
+  * destruct bytes1; try discriminate. destruct bytes1; try discriminate.
+    simpl in H. destruct H; try contradiction. subst m0.
+    exists ofs; split. omega. auto.
+  * exploit (REC (sz - 1)). red; omega. eexact LOAD2. auto.
+    intros (ofs' & A & B).
+    exists ofs'; split. omega. auto.
+Qed.
+
+Lemma smatch_loadbytes:
+  forall m b p b' ofs' q i n ofs bytes,
+  Mem.loadbytes m b ofs n = Some bytes ->
+  smatch m b p ->
+  In (Fragment (Vptr b' ofs') q i) bytes ->
+  pmatch b' ofs' p.
+Proof.
+  intros. exploit In_loadbytes; eauto. intros (ofs1 & A & B).
+  eapply H0; eauto.
+Qed.
+
+Lemma loadbytes_provenance:
+  forall m b ofs' byte n ofs bytes,
+  Mem.loadbytes m b ofs n = Some bytes ->
+  Mem.loadbytes m b ofs' 1 = Some (byte :: nil) ->
+  ofs <= ofs' < ofs + n ->
+  In byte bytes.
+Proof.
+  intros until n. pattern n.
+  apply well_founded_ind with (R := Zwf 0).
+- apply Zwf_well_founded.
+- intros sz REC ofs bytes LOAD LOAD1 IN.
+  exploit (Mem.loadbytes_split m b ofs 1 (sz - 1) bytes).
+  replace (1 + (sz - 1)) with sz by omega. auto.
+  omega.
+  omega.
+  intros (bytes1 & bytes2 & LOAD3 & LOAD4 & CONCAT). subst bytes. rewrite in_app_iff.
+  destruct (zeq ofs ofs').
++ subst ofs'. rewrite LOAD1 in LOAD3; inv LOAD3. left; simpl; auto.
++ right. eapply (REC (sz - 1)). red; omega. eexact LOAD4. auto. omega.
+Qed.
+
+Lemma storebytes_provenance:
+  forall m b ofs bytes m' b' ofs' b'' ofs'' q i,
+  Mem.storebytes m b ofs bytes = Some m' ->
+  Mem.loadbytes m' b' ofs' 1 = Some (Fragment (Vptr b'' ofs'') q i :: nil) ->
+  In (Fragment (Vptr b'' ofs'') q i) bytes
+  \/ Mem.loadbytes m b' ofs' 1 = Some (Fragment (Vptr b'' ofs'') q i :: nil).
+Proof.
+  intros.
+  assert (EITHER:
+            (b' <> b \/ ofs' + 1 <= ofs \/ ofs + Z.of_nat (length bytes) <= ofs')
+         \/ (b' = b /\ ofs <= ofs' < ofs + Z.of_nat (length bytes))).
+  {
+    destruct (eq_block b' b); auto.
+    destruct (zle (ofs' + 1) ofs); auto.
+    destruct (zle (ofs + Z.of_nat (length bytes)) ofs'); auto.
+    right. split. auto. omega.
+  }
+  destruct EITHER as [A | (A & B)].
+- right. rewrite <- H0. symmetry. eapply Mem.loadbytes_storebytes_other; eauto. omega.
+- subst b'. left.
+  eapply loadbytes_provenance; eauto.
+  eapply Mem.loadbytes_storebytes_same; eauto.
+Qed.
+
+Lemma store_provenance:
+  forall chunk m b ofs v m' b' ofs' b'' ofs'' q i,
+  Mem.store chunk m b ofs v = Some m' ->
+  Mem.loadbytes m' b' ofs' 1 = Some (Fragment (Vptr b'' ofs'') q i :: nil) ->
+  v = Vptr b'' ofs'' /\ (chunk = Mint32 \/ chunk = Many32 \/ chunk = Mint64 \/ chunk = Many64)
+  \/ Mem.loadbytes m b' ofs' 1 = Some (Fragment (Vptr b'' ofs'') q i :: nil).
+Proof.
+  intros. exploit storebytes_provenance; eauto. eapply Mem.store_storebytes; eauto.
+  intros [A|A]; auto. left.
+  generalize (encode_val_shape chunk v). intros ENC; inv ENC.
+- split; auto. rewrite <- H1 in A; destruct A.
+  + congruence.
+  + exploit H5; eauto. intros (j & P & Q); congruence.
+- rewrite <- H1 in A; destruct A.
+  + congruence.
+  + exploit H3; eauto. intros [byte P]; congruence.
+- rewrite <- H1 in A; destruct A.
+  + congruence.
+  + exploit H2; eauto. congruence.
+Qed.
+
+Lemma smatch_store:
+  forall chunk m b ofs v m' b' p av,
+  Mem.store chunk m b ofs v = Some m' ->
+  smatch m b' p ->
+  vmatch v av ->
+  smatch m' b' (vplub av p).
+Proof.
+  intros. destruct H0 as [A B]. split.
+- intros chunk' ofs' v' LOAD. destruct v'; auto with va.
+  exploit Mem.load_pointer_store; eauto.
+  intros [(P & Q & R & S) | DISJ].
++ subst. apply vmatch_vplub_l. auto.
++ apply vmatch_vplub_r. apply A with (chunk := chunk') (ofs := ofs').
+  rewrite <- LOAD. symmetry. eapply Mem.load_store_other; eauto.
+- intros. exploit store_provenance; eauto. intros [[P Q] | P].
++ subst.
+  assert (V: vmatch (Vptr b'0 ofs') (Ifptr (vplub av p))).
+  {
+    apply vmatch_vplub_l. auto.
+  }
+  inv V; auto.
++ apply pmatch_vplub. eapply B; eauto.
+Qed.
+
+Lemma smatch_storebytes:
+  forall m b ofs bytes m' b' p p',
+  Mem.storebytes m b ofs bytes = Some m' ->
+  smatch m b' p ->
+  (forall b' ofs' q i, In (Fragment (Vptr b' ofs') q i) bytes -> pmatch b' ofs' p') ->
+  smatch m' b' (plub p' p).
+Proof.
+  intros. destruct H0 as [A B]. split.
+- intros. apply vmatch_ifptr. intros bx ofsx EQ; subst v.
+  exploit Mem.load_loadbytes; eauto. intros (bytes' & P & Q).
+  destruct bytes' as [ | byte1' bytes'].
+  exploit Mem.loadbytes_length; eauto. intros. destruct chunk; discriminate.
+  generalize (decode_val_shape chunk byte1' bytes'). rewrite <- Q.
+  intros DEC; inv DEC; try contradiction.
+  assert (v = Vptr bx ofsx).
+  { destruct H5 as [E|[E|[E|E]]]; rewrite E in H4; destruct v; simpl in H4;
+    try congruence; destruct Archi.ptr64; congruence. }
+  exploit In_loadbytes; eauto. eauto with coqlib.
+  intros (ofs' & X & Y). subst v.
+  exploit storebytes_provenance; eauto. intros [Z | Z].
+  apply pmatch_lub_l. eauto.
+  apply pmatch_lub_r. eauto.
+- intros. exploit storebytes_provenance; eauto. intros [Z | Z].
+  apply pmatch_lub_l. eauto.
+  apply pmatch_lub_r. eauto.
+Qed.
+
+Definition bmatch (m: mem) (b: block) (ab: ablock) : Prop :=
+  smatch m b ab.(ab_summary) /\
+  forall chunk ofs v, Mem.load chunk m b ofs = Some v -> vmatch v (ablock_load chunk ab ofs).
+
+Lemma bmatch_ext:
+  forall m b ab m',
+  bmatch m b ab ->
+  (forall ofs n bytes, Mem.loadbytes m' b ofs n = Some bytes -> n >= 0 -> Mem.loadbytes m b ofs n = Some bytes) ->
+  bmatch m' b ab.
+Proof.
+  intros. destruct H as [A B]. split; intros.
+  apply smatch_ext with m; auto.
+  eapply B; eauto. eapply loadbytes_load_ext; eauto.
+Qed.
+
+Lemma bmatch_inv:
+  forall m b ab m',
+  bmatch m b ab ->
+  (forall ofs n, n >= 0 -> Mem.loadbytes m' b ofs n = Mem.loadbytes m b ofs n) ->
+  bmatch m' b ab.
+Proof.
+  intros. eapply bmatch_ext; eauto.
+  intros. rewrite <- H0; eauto.
+Qed.
+
+Lemma ablock_load_sound:
+  forall chunk m b ofs v ab,
+  Mem.load chunk m b ofs = Some v ->
+  bmatch m b ab ->
+  vmatch v (ablock_load chunk ab ofs).
+Proof.
+  intros. destruct H0. eauto.
+Qed.
+
+Lemma ablock_load_anywhere_sound:
+  forall chunk m b ofs v ab,
+  Mem.load chunk m b ofs = Some v ->
+  bmatch m b ab ->
+  vmatch v (ablock_load_anywhere chunk ab).
+Proof.
+  intros. destruct H0. destruct H0. unfold ablock_load_anywhere.
+  eapply vnormalize_cast; eauto.
+Qed.
+
+Lemma ablock_init_sound:
+  forall m b p, smatch m b p -> bmatch m b (ablock_init p).
+Proof.
+  intros; split; auto; intros.
+  unfold ablock_load, ablock_init; simpl. rewrite ZTree.gempty.
+  eapply vnormalize_cast; eauto. eapply H; eauto.
+Qed.
+
+Lemma ablock_store_anywhere_sound:
+  forall chunk m b ofs v m' b' ab av,
+  Mem.store chunk m b ofs v = Some m' ->
+  bmatch m b' ab ->
+  vmatch v av ->
+  bmatch m' b' (ablock_store_anywhere chunk ab av).
+Proof.
+  intros. destruct H0 as [A B]. unfold ablock_store_anywhere.
+  apply ablock_init_sound. eapply smatch_store; eauto.
+Qed.
+
+Remark inval_after_outside:
+  forall i lo hi c, i < lo \/ i > hi -> (inval_after lo hi c)##i = c##i.
+Proof.
+  intros until c. functional induction (inval_after lo hi c); intros.
+  rewrite IHt by omega. apply ZTree.gro. unfold ZTree.elt, ZIndexed.t; omega.
+  auto.
+Qed.
+
+Remark inval_after_contents:
+  forall chunk av i lo hi c,
+  (inval_after lo hi c)##i = Some (ACval chunk av) ->
+  c##i = Some (ACval chunk av) /\ (i < lo \/ i > hi).
+Proof.
+  intros until c. functional induction (inval_after lo hi c); intros.
+  destruct (zeq i hi).
+  subst i. rewrite inval_after_outside in H by omega. rewrite ZTree.grs in H. discriminate.
+  exploit IHt; eauto. intros [A B]. rewrite ZTree.gro in A by auto. split. auto. omega.
+  split. auto. omega.
+Qed.
+
+Remark inval_before_outside:
+  forall i hi lo c, i < lo \/ i >= hi -> (inval_before hi lo c)##i = c##i.
+Proof.
+  intros until c. functional induction (inval_before hi lo c); intros.
+  rewrite IHt by omega. unfold inval_if. destruct (c##lo) as [[chunk av]|]; auto.
+  destruct (zle (lo + size_chunk chunk) hi); auto.
+  apply ZTree.gro. unfold ZTree.elt, ZIndexed.t; omega.
+  auto.
+Qed.
+
+Remark inval_before_contents_1:
+  forall i chunk av lo hi c,
+  lo <= i < hi -> (inval_before hi lo c)##i = Some(ACval chunk av) ->
+  c##i = Some(ACval chunk av) /\ i + size_chunk chunk <= hi.
+Proof.
+  intros until c. functional induction (inval_before hi lo c); intros.
+- destruct (zeq lo i).
++ subst i. rewrite inval_before_outside in H0 by omega.
+  unfold inval_if in H0. destruct (c##lo) as [[chunk0 v0]|] eqn:C; try congruence.
+  destruct (zle (lo + size_chunk chunk0) hi).
+  rewrite C in H0; inv H0. auto.
+  rewrite ZTree.grs in H0. congruence.
++ exploit IHt. omega. auto. intros [A B]; split; auto.
+  unfold inval_if in A. destruct (c##lo) as [[chunk0 v0]|] eqn:C; auto.
+  destruct (zle (lo + size_chunk chunk0) hi); auto.
+  rewrite ZTree.gro in A; auto.
+- omegaContradiction.
+Qed.
+
+Lemma max_size_chunk: forall chunk, size_chunk chunk <= 8.
+Proof.
+  destruct chunk; simpl; omega.
+Qed.
+
+Remark inval_before_contents:
+  forall i c chunk' av' j,
+  (inval_before i (i - 7) c)##j = Some (ACval chunk' av') ->
+  c##j = Some (ACval chunk' av') /\ (j + size_chunk chunk' <= i \/ i <= j).
+Proof.
+  intros. destruct (zlt j (i - 7)).
+  rewrite inval_before_outside in H by omega.
+  split. auto. left. generalize (max_size_chunk chunk'); omega.
+  destruct (zlt j i).
+  exploit inval_before_contents_1; eauto. omega. tauto.
+  rewrite inval_before_outside in H by omega.
+  split. auto. omega.
+Qed.
+
+Lemma ablock_store_contents:
+  forall chunk ab i av j chunk' av',
+  (ablock_store chunk ab i av).(ab_contents)##j = Some(ACval chunk' av') ->
+     (i = j /\ chunk' = chunk /\ av' = av)
+  \/ (ab.(ab_contents)##j = Some(ACval chunk' av')
+      /\ (j + size_chunk chunk' <= i \/ i + size_chunk chunk <= j)).
+Proof.
+  unfold ablock_store; simpl; intros.
+  destruct (zeq i j).
+  subst j. rewrite ZTree.gss in H. inv H; auto.
+  right. rewrite ZTree.gso in H by auto.
+  exploit inval_before_contents; eauto. intros [A B].
+  exploit inval_after_contents; eauto. intros [C D].
+  split. auto. omega.
+Qed.
+
+Lemma chunk_compat_true:
+  forall c c',
+  chunk_compat c c' = true ->
+  size_chunk c = size_chunk c' /\ align_chunk c <= align_chunk c' /\ type_of_chunk c = type_of_chunk c'.
+Proof.
+  destruct c, c'; intros; try discriminate; simpl; auto with va.
+Qed.
+
+Lemma ablock_store_sound:
+  forall chunk m b ofs v m' ab av,
+  Mem.store chunk m b ofs v = Some m' ->
+  bmatch m b ab ->
+  vmatch v av ->
+  bmatch m' b (ablock_store chunk ab ofs av).
+Proof.
+  intros until av; intros STORE BIN VIN. destruct BIN as [BIN1 BIN2]. split.
+  eapply smatch_store; eauto.
+  intros chunk' ofs' v' LOAD.
+  assert (SUMMARY: vmatch v' (vnormalize chunk' (Ifptr (vplub av ab.(ab_summary))))).
+  { exploit smatch_store; eauto. intros [A B]. eapply vnormalize_cast; eauto. }
+  unfold ablock_load.
+  destruct ((ab_contents (ablock_store chunk ab ofs av)) ## ofs') as [[chunk1 av1]|] eqn:C; auto.
+  destruct (chunk_compat chunk' chunk1) eqn:COMPAT; auto.
+  exploit chunk_compat_true; eauto. intros (U & V & W).
+  exploit ablock_store_contents; eauto. intros [(P & Q & R) | (P & Q)].
+- (* same offset and compatible chunks *)
+  subst.
+  assert (v' = Val.load_result chunk' v).
+  { exploit Mem.load_store_similar_2; eauto. congruence. }
+  subst v'. apply vnormalize_sound; auto.
+- (* disjoint load/store *)
+  assert (Mem.load chunk' m b ofs' = Some v').
+  { rewrite <- LOAD. symmetry. eapply Mem.load_store_other; eauto.
+    rewrite U. auto. }
+  exploit BIN2; eauto. unfold ablock_load. rewrite P. rewrite COMPAT. auto.
+Qed.
+
+Lemma ablock_loadbytes_sound:
+  forall m b ab b' ofs' q i n ofs bytes,
+  Mem.loadbytes m b ofs n = Some bytes ->
+  bmatch m b ab ->
+  In (Fragment (Vptr b' ofs') q i) bytes ->
+  pmatch b' ofs' (ablock_loadbytes ab).
+Proof.
+  intros. destruct H0. eapply smatch_loadbytes; eauto.
+Qed.
+
+Lemma ablock_storebytes_anywhere_sound:
+  forall m b ofs bytes p m' b' ab,
+  Mem.storebytes m b ofs bytes = Some m' ->
+  (forall b' ofs' q i, In (Fragment (Vptr b' ofs') q i) bytes -> pmatch b' ofs' p) ->
+  bmatch m b' ab ->
+  bmatch m' b' (ablock_storebytes_anywhere ab p).
+Proof.
+  intros. destruct H1 as [A B]. apply ablock_init_sound.
+  eapply smatch_storebytes; eauto.
+Qed.
+
+Lemma ablock_storebytes_contents:
+  forall ab p i sz j chunk' av',
+  (ablock_storebytes ab p i sz).(ab_contents)##j = Some(ACval chunk' av') ->
+  ab.(ab_contents)##j = Some (ACval chunk' av')
+  /\ (j + size_chunk chunk' <= i \/ i + Z.max sz 0 <= j).
+Proof.
+  unfold ablock_storebytes; simpl; intros.
+  exploit inval_before_contents; eauto. clear H. intros [A B].
+  exploit inval_after_contents; eauto. clear A. intros [C D].
+  split. auto. xomega.
+Qed.
+
+Lemma ablock_storebytes_sound:
+  forall m b ofs bytes m' p ab sz,
+  Mem.storebytes m b ofs bytes = Some m' ->
+  length bytes = Z.to_nat sz ->
+  (forall b' ofs' q i, In (Fragment (Vptr b' ofs') q i) bytes -> pmatch b' ofs' p) ->
+  bmatch m b ab ->
+  bmatch m' b (ablock_storebytes ab p ofs sz).
+Proof.
+  intros until sz; intros STORE LENGTH CONTENTS BM. destruct BM as [BM1 BM2]. split.
+  eapply smatch_storebytes; eauto.
+  intros chunk' ofs' v' LOAD'.
+  assert (SUMMARY: vmatch v' (vnormalize chunk' (Ifptr (plub p ab.(ab_summary))))).
+  { exploit smatch_storebytes; eauto. intros [A B]. eapply vnormalize_cast; eauto. }
+  unfold ablock_load.
+  destruct (ab_contents (ablock_storebytes ab p ofs sz))##ofs' as [[chunk av]|] eqn:C; auto.
+  destruct (chunk_compat chunk' chunk) eqn:COMPAT; auto.
+  exploit chunk_compat_true; eauto. intros (U & V & W).
+  exploit ablock_storebytes_contents; eauto. intros [A B].
+  assert (Mem.load chunk' m b ofs' = Some v').
+  { rewrite <- LOAD'; symmetry. eapply Mem.load_storebytes_other; eauto.
+    rewrite U. rewrite LENGTH. rewrite Z_to_nat_max. right; omega. }
+  exploit BM2; eauto. unfold ablock_load. rewrite A. rewrite COMPAT. auto.
+Qed.
+
+(** Boolean equality *)
+
+Definition bbeq (ab1 ab2: ablock) : bool :=
+  eq_aptr ab1.(ab_summary) ab2.(ab_summary) &&
+  ZTree.beq (fun c1 c2 => proj_sumbool (eq_acontent c1 c2)) ab1.(ab_contents) ab2.(ab_contents).
+
+Lemma bbeq_load:
+  forall ab1 ab2,
+  bbeq ab1 ab2 = true ->
+  ab1.(ab_summary) = ab2.(ab_summary)
+  /\ (forall chunk i, ablock_load chunk ab1 i = ablock_load chunk ab2 i).
+Proof.
+  unfold bbeq; intros. InvBooleans. split.
+- unfold ablock_load_anywhere; intros; congruence.
+- assert (A: forall i, ZTree.get i (ab_contents ab1) = ZTree.get i (ab_contents ab2)).
+  {
+    intros. exploit ZTree.beq_sound; eauto. instantiate (1 := i).
+    destruct (ab_contents ab1)##i, (ab_contents ab2)##i; intros; try contradiction.
+    InvBooleans; subst; auto.
+    auto. }
+  intros. unfold ablock_load. rewrite A, H.
+  destruct (ab_contents ab2)##i; auto.
+Qed.
+
+Lemma bbeq_sound:
+  forall ab1 ab2,
+  bbeq ab1 ab2 = true ->
+  forall m b, bmatch m b ab1 <-> bmatch m b ab2.
+Proof.
+  intros. exploit bbeq_load; eauto. intros [A B].
+  unfold bmatch. rewrite A. intuition. rewrite <- B; eauto. rewrite B; eauto.
+Qed.
+
+(** Least upper bound *)
+
+Definition combine_acontents (c1 c2: option acontent) : option acontent :=
+  match c1, c2 with
+  | Some (ACval chunk1 v1), Some (ACval chunk2 v2) =>
+      if chunk_eq chunk1 chunk2 then Some(ACval chunk1 (vlub v1 v2)) else None
+  | _, _ =>
+      None
+  end.
+
+Definition blub (ab1 ab2: ablock) : ablock :=
+  {| ab_contents := ZTree.combine combine_acontents ab1.(ab_contents) ab2.(ab_contents);
+     ab_summary := plub ab1.(ab_summary) ab2.(ab_summary) |}.
+
+Lemma smatch_lub_l:
+  forall m b p q, smatch m b p -> smatch m b (plub p q).
+Proof.
+  intros. destruct H as [A B]. split; intros.
+  change (vmatch v (vlub (Ifptr p) (Ifptr q))). apply vmatch_lub_l. eapply A; eauto.
+  apply pmatch_lub_l. eapply B; eauto.
+Qed.
+
+Lemma smatch_lub_r:
+  forall m b p q, smatch m b q -> smatch m b (plub p q).
+Proof.
+  intros. destruct H as [A B]. split; intros.
+  change (vmatch v (vlub (Ifptr p) (Ifptr q))). apply vmatch_lub_r. eapply A; eauto.
+  apply pmatch_lub_r. eapply B; eauto.
+Qed.
+
+Lemma bmatch_lub_l:
+  forall m b x y, bmatch m b x -> bmatch m b (blub x y).
+Proof.
+  intros. destruct H as [BM1 BM2]. split; unfold blub; simpl.
+- apply smatch_lub_l; auto.
+- intros.
+  assert (SUMMARY: vmatch v (vnormalize chunk (Ifptr (plub (ab_summary x) (ab_summary y))))
+).
+  { exploit smatch_lub_l; eauto. instantiate (1 := ab_summary y).
+    intros [SUMM _]. eapply vnormalize_cast; eauto. }
+  exploit BM2; eauto.
+  unfold ablock_load; simpl. rewrite ZTree.gcombine by auto.
+  unfold combine_acontents;
+  destruct (ab_contents x)##ofs as [[chunkx avx]|], (ab_contents y)##ofs as [[chunky avy]|]; auto.
+  destruct (chunk_eq chunkx chunky); auto. subst chunky.
+  destruct (chunk_compat chunk chunkx); auto.
+  intros. eapply vmatch_ge; eauto. apply vnormalize_monotone. apply vge_lub_l.
+Qed.
+
+Lemma bmatch_lub_r:
+  forall m b x y, bmatch m b y -> bmatch m b (blub x y).
+Proof.
+  intros. destruct H as [BM1 BM2]. split; unfold blub; simpl.
+- apply smatch_lub_r; auto.
+- intros.
+  assert (SUMMARY: vmatch v (vnormalize chunk (Ifptr (plub (ab_summary x) (ab_summary y))))
+).
+  { exploit smatch_lub_r; eauto. instantiate (1 := ab_summary x).
+    intros [SUMM _]. eapply vnormalize_cast; eauto. }
+  exploit BM2; eauto.
+  unfold ablock_load; simpl. rewrite ZTree.gcombine by auto.
+  unfold combine_acontents;
+  destruct (ab_contents x)##ofs as [[chunkx avx]|], (ab_contents y)##ofs as [[chunky avy]|]; auto.
+  destruct (chunk_eq chunkx chunky); auto. subst chunky.
+  destruct (chunk_compat chunk chunkx); auto.
+  intros. eapply vmatch_ge; eauto. apply vnormalize_monotone. apply vge_lub_r.
+Qed.
+
+(** * Abstracting read-only global variables *)
+
+Definition romem := PTree.t ablock.
+
+Definition romatch  (m: mem) (rm: romem) : Prop :=
+  forall b id ab,
+  bc b = BCglob id ->
+  rm!id = Some ab ->
+  pge Glob ab.(ab_summary)
+  /\ bmatch m b ab
+  /\ forall ofs, ~Mem.perm m b ofs Max Writable.
+
+Lemma romatch_store:
+  forall chunk m b ofs v m' rm,
+  Mem.store chunk m b ofs v = Some m' ->
+  romatch m rm ->
+  romatch m' rm.
+Proof.
+  intros; red; intros. exploit H0; eauto. intros (A & B & C). split; auto. split.
+- exploit Mem.store_valid_access_3; eauto. intros [P _].
+  apply bmatch_inv with m; auto.
++ intros. eapply Mem.loadbytes_store_other; eauto.
+  left. red; intros; subst b0. elim (C ofs). apply Mem.perm_cur_max.
+  apply P. generalize (size_chunk_pos chunk); omega.
+- intros; red; intros; elim (C ofs0). eauto with mem.
+Qed.
+
+Lemma romatch_storebytes:
+  forall m b ofs bytes m' rm,
+  Mem.storebytes m b ofs bytes = Some m' ->
+  romatch m rm ->
+  romatch m' rm.
+Proof.
+  intros; red; intros. exploit H0; eauto. intros (A & B & C). split; auto. split.
+- apply bmatch_inv with m; auto.
+  intros. eapply Mem.loadbytes_storebytes_disjoint; eauto.
+  destruct (eq_block b0 b); auto. subst b0. right; red; unfold Intv.In; simpl; red; intros.
+  elim (C x). apply Mem.perm_cur_max. eapply Mem.storebytes_range_perm; eauto.
+- intros; red; intros; elim (C ofs0). eauto with mem.
+Qed.
+
+Lemma romatch_ext:
+  forall m rm m',
+  romatch m rm ->
+  (forall b id ofs n bytes, bc b = BCglob id -> Mem.loadbytes m' b ofs n = Some bytes -> Mem.loadbytes m b ofs n = Some bytes) ->
+  (forall b id ofs p, bc b = BCglob id -> Mem.perm m' b ofs Max p -> Mem.perm m b ofs Max p) ->
+  romatch m' rm.
+Proof.
+  intros; red; intros. exploit H; eauto. intros (A & B & C).
+  split. auto.
+  split. apply bmatch_ext with m; auto. intros. eapply H0; eauto.
+  intros; red; intros. elim (C ofs). eapply H1; eauto.
+Qed.
+
+Lemma romatch_free:
+  forall m b lo hi m' rm,
+  Mem.free m b lo hi = Some m' ->
+  romatch m rm ->
+  romatch m' rm.
+Proof.
+  intros. apply romatch_ext with m; auto.
+  intros. eapply Mem.loadbytes_free_2; eauto.
+  intros. eauto with mem.
+Qed.
+
+Lemma romatch_alloc:
+  forall m b lo hi m' rm,
+  Mem.alloc m lo hi = (m', b) ->
+  bc_below bc (Mem.nextblock m) ->
+  romatch m rm ->
+  romatch m' rm.
+Proof.
+  intros. apply romatch_ext with m; auto.
+  intros. rewrite <- H3; symmetry. eapply Mem.loadbytes_alloc_unchanged; eauto.
+  apply H0. congruence.
+  intros. eapply Mem.perm_alloc_4; eauto. apply Mem.valid_not_valid_diff with m; eauto with mem.
+  apply H0. congruence.
+Qed.
+
+(** * Abstracting memory states *)
+
+Record amem : Type := AMem {
+  am_stack: ablock;
+  am_glob: PTree.t ablock;
+  am_nonstack: aptr;
+  am_top: aptr
+}.
+
+Record mmatch (m: mem) (am: amem) : Prop := mk_mem_match {
+  mmatch_stack: forall b,
+    bc b = BCstack ->
+    bmatch m b am.(am_stack);
+  mmatch_glob: forall id ab b,
+    bc b = BCglob id ->
+    am.(am_glob)!id = Some ab ->
+    bmatch m b ab;
+  mmatch_nonstack: forall b,
+    bc b <> BCstack -> bc b <> BCinvalid ->
+    smatch m b am.(am_nonstack);
+  mmatch_top: forall b,
+    bc b <> BCinvalid ->
+    smatch m b am.(am_top);
+  mmatch_below:
+    bc_below bc (Mem.nextblock m)
+}.
+
+Definition minit (p: aptr) :=
+  {| am_stack := ablock_init p;
+     am_glob := PTree.empty _;
+     am_nonstack := p;
+     am_top := p |}.
+
+Definition mbot := minit Pbot.
+Definition mtop := minit Ptop.
+
+Definition load (chunk: memory_chunk) (rm: romem) (m: amem) (p: aptr) : aval :=
+  match p with
+  | Pbot => if va_strict tt then Vbot else Vtop
+  | Gl id ofs =>
+      match rm!id with
+      | Some ab => ablock_load chunk ab (Ptrofs.unsigned ofs)
+      | None =>
+          match m.(am_glob)!id with
+          | Some ab => ablock_load chunk ab (Ptrofs.unsigned ofs)
+          | None => vnormalize chunk (Ifptr m.(am_nonstack))
+          end
+      end
+  | Glo id =>
+      match rm!id with
+      | Some ab => ablock_load_anywhere chunk ab
+      | None =>
+          match m.(am_glob)!id with
+          | Some ab => ablock_load_anywhere chunk ab
+          | None => vnormalize chunk (Ifptr m.(am_nonstack))
+          end
+      end
+  | Stk ofs => ablock_load chunk m.(am_stack) (Ptrofs.unsigned ofs)
+  | Stack => ablock_load_anywhere chunk m.(am_stack)
+  | Glob | Nonstack => vnormalize chunk (Ifptr m.(am_nonstack))
+  | Ptop => vnormalize chunk (Ifptr m.(am_top))
+  end.
+
+Definition loadv (chunk: memory_chunk) (rm: romem) (m: amem) (addr: aval) : aval :=
+  load chunk rm m (aptr_of_aval addr).
+
+Definition store (chunk: memory_chunk) (m: amem) (p: aptr) (av: aval) : amem :=
+  {| am_stack :=
+       match p with
+       | Stk ofs      => ablock_store chunk m.(am_stack) (Ptrofs.unsigned ofs) av
+       | Stack | Ptop => ablock_store_anywhere chunk m.(am_stack) av
+       | _ => m.(am_stack)
+       end;
+     am_glob :=
+       match p with
+       | Gl id ofs =>
+           let ab := match m.(am_glob)!id with Some ab => ab | None => ablock_init m.(am_nonstack) end in
+           PTree.set id (ablock_store chunk ab (Ptrofs.unsigned ofs) av) m.(am_glob)
+       | Glo id =>
+           let ab := match m.(am_glob)!id with Some ab => ab | None => ablock_init m.(am_nonstack) end in
+           PTree.set id (ablock_store_anywhere chunk ab av) m.(am_glob)
+       | Glob | Nonstack | Ptop => PTree.empty _
+       | _ => m.(am_glob)
+       end;
+     am_nonstack :=
+       match p with
+       | Gl _ _ | Glo _ | Glob | Nonstack | Ptop => vplub av m.(am_nonstack)
+       | _ => m.(am_nonstack)
+       end;
+     am_top := vplub av m.(am_top)
+  |}.
+
+Definition storev (chunk: memory_chunk) (m: amem) (addr: aval) (v: aval): amem :=
+  store chunk m (aptr_of_aval addr) v.
+
+Definition loadbytes (m: amem) (rm: romem) (p: aptr) : aptr :=
+  match p with
+  | Pbot => if va_strict tt then Pbot else Ptop
+  | Gl id _ | Glo id =>
+      match rm!id with
+      | Some ab => ablock_loadbytes ab
+      | None =>
+          match m.(am_glob)!id with
+          | Some ab => ablock_loadbytes ab
+          | None => m.(am_nonstack)
+          end
+      end
+  | Stk _ | Stack => ablock_loadbytes m.(am_stack)
+  | Glob | Nonstack => m.(am_nonstack)
+  | Ptop => m.(am_top)
+  end.
+
+Definition storebytes (m: amem) (dst: aptr) (sz: Z) (p: aptr) : amem :=
+  {| am_stack :=
+       match dst with
+       | Stk ofs      => ablock_storebytes m.(am_stack) p (Ptrofs.unsigned ofs) sz
+       | Stack | Ptop => ablock_storebytes_anywhere m.(am_stack) p
+       | _ => m.(am_stack)
+       end;
+     am_glob :=
+       match dst with
+       | Gl id ofs =>
+           let ab := match m.(am_glob)!id with Some ab => ab | None => ablock_init m.(am_nonstack) end in
+           PTree.set id (ablock_storebytes ab p (Ptrofs.unsigned ofs) sz) m.(am_glob)
+       | Glo id =>
+           let ab := match m.(am_glob)!id with Some ab => ab | None => ablock_init m.(am_nonstack) end in
+           PTree.set id (ablock_storebytes_anywhere ab p) m.(am_glob)
+       | Glob | Nonstack | Ptop => PTree.empty _
+       | _ => m.(am_glob)
+       end;
+     am_nonstack :=
+       match dst with
+       | Gl _ _ | Glo _ | Glob | Nonstack | Ptop => plub p m.(am_nonstack)
+       | _ => m.(am_nonstack)
+       end;
+     am_top := plub p m.(am_top)
+  |}.
+
+Theorem load_sound:
+  forall chunk m b ofs v rm am p,
+  Mem.load chunk m b (Ptrofs.unsigned ofs) = Some v ->
+  romatch m rm ->
+  mmatch m am ->
+  pmatch b ofs p ->
+  vmatch v (load chunk rm am p).
+Proof.
+  intros. unfold load. inv H2.
+- (* Gl id ofs *)
+  destruct (rm!id) as [ab|] eqn:RM.
+  eapply ablock_load_sound; eauto. eapply H0; eauto.
+  destruct (am_glob am)!id as [ab|] eqn:AM.
+  eapply ablock_load_sound; eauto. eapply mmatch_glob; eauto.
+  eapply vnormalize_cast; eauto. eapply mmatch_nonstack; eauto; congruence.
+- (* Glo id *)
+  destruct (rm!id) as [ab|] eqn:RM.
+  eapply ablock_load_anywhere_sound; eauto. eapply H0; eauto.
+  destruct (am_glob am)!id as [ab|] eqn:AM.
+  eapply ablock_load_anywhere_sound; eauto. eapply mmatch_glob; eauto.
+  eapply vnormalize_cast; eauto. eapply mmatch_nonstack; eauto; congruence.
+- (* Glob *)
+  eapply vnormalize_cast; eauto. eapply mmatch_nonstack; eauto. congruence. congruence.
+- (* Stk ofs *)
+  eapply ablock_load_sound; eauto. eapply mmatch_stack; eauto.
+- (* Stack *)
+  eapply ablock_load_anywhere_sound; eauto. eapply mmatch_stack; eauto.
+- (* Nonstack *)
+  eapply vnormalize_cast; eauto. eapply mmatch_nonstack; eauto.
+- (* Top *)
+  eapply vnormalize_cast; eauto. eapply mmatch_top; eauto.
+Qed.
+
+Theorem loadv_sound:
+  forall chunk m addr v rm am aaddr,
+  Mem.loadv chunk m addr = Some v ->
+  romatch m rm ->
+  mmatch m am ->
+  vmatch addr aaddr ->
+  vmatch v (loadv chunk rm am aaddr).
+Proof.
+  intros. destruct addr; simpl in H; try discriminate.
+  eapply load_sound; eauto. apply match_aptr_of_aval; auto.
+Qed.
+
+Theorem store_sound:
+  forall chunk m b ofs v m' am p av,
+  Mem.store chunk m b (Ptrofs.unsigned ofs) v = Some m' ->
+  mmatch m am ->
+  pmatch b ofs p ->
+  vmatch v av ->
+  mmatch m' (store chunk am p av).
+Proof.
+  intros until av; intros STORE MM PM VM.
+  unfold store; constructor; simpl; intros.
+- (* Stack *)
+  assert (DFL: bc b <> BCstack -> bmatch m' b0 (am_stack am)).
+  { intros. apply bmatch_inv with m. eapply mmatch_stack; eauto.
+    intros. eapply Mem.loadbytes_store_other; eauto. left; congruence. }
+  inv PM; try (apply DFL; congruence).
+  + assert (b0 = b) by (eapply bc_stack; eauto). subst b0.
+    eapply ablock_store_sound; eauto. eapply mmatch_stack; eauto.
+  + assert (b0 = b) by (eapply bc_stack; eauto). subst b0.
+    eapply ablock_store_anywhere_sound; eauto. eapply mmatch_stack; eauto.
+  + eapply ablock_store_anywhere_sound; eauto. eapply mmatch_stack; eauto.
+
+- (* Globals *)
+  rename b0 into b'.
+  assert (DFL: bc b <> BCglob id -> (am_glob am)!id = Some ab ->
+               bmatch m' b' ab).
+  { intros. apply bmatch_inv with m. eapply mmatch_glob; eauto.
+    intros. eapply Mem.loadbytes_store_other; eauto. left; congruence. }
+  inv PM.
+  + rewrite PTree.gsspec in H0. destruct (peq id id0).
+    subst id0; inv H0.
+    assert (b' = b) by (eapply bc_glob; eauto). subst b'.
+    eapply ablock_store_sound; eauto.
+    destruct (am_glob am)!id as [ab0|] eqn:GL.
+    eapply mmatch_glob; eauto.
+    apply ablock_init_sound. eapply mmatch_nonstack; eauto; congruence.
+    eapply DFL; eauto. congruence.
+  + rewrite PTree.gsspec in H0. destruct (peq id id0).
+    subst id0; inv H0.
+    assert (b' = b) by (eapply bc_glob; eauto). subst b'.
+    eapply ablock_store_anywhere_sound; eauto.
+    destruct (am_glob am)!id as [ab0|] eqn:GL.
+    eapply mmatch_glob; eauto.
+    apply ablock_init_sound. eapply mmatch_nonstack; eauto; congruence.
+    eapply DFL; eauto. congruence.
+  + rewrite PTree.gempty in H0; congruence.
+  + eapply DFL; eauto. congruence.
+  + eapply DFL; eauto. congruence.
+  + rewrite PTree.gempty in H0; congruence.
+  + rewrite PTree.gempty in H0; congruence.
+
+- (* Nonstack *)
+  assert (DFL: smatch m' b0 (vplub av (am_nonstack am))).
+  { eapply smatch_store; eauto. eapply mmatch_nonstack; eauto. }
+  assert (STK: bc b = BCstack -> smatch m' b0 (am_nonstack am)).
+  { intros. apply smatch_inv with m. eapply mmatch_nonstack; eauto; congruence.
+    intros. eapply Mem.loadbytes_store_other; eauto. left. congruence.
+  }
+  inv PM; (apply DFL || apply STK; congruence).
+
+- (* Top *)
+  eapply smatch_store; eauto. eapply mmatch_top; eauto.
+
+- (* Below *)
+  erewrite Mem.nextblock_store by eauto. eapply mmatch_below; eauto.
+Qed.
+
+Theorem storev_sound:
+  forall chunk m addr v m' am aaddr av,
+  Mem.storev chunk m addr v = Some m' ->
+  mmatch m am ->
+  vmatch addr aaddr ->
+  vmatch v av ->
+  mmatch m' (storev chunk am aaddr av).
+Proof.
+  intros. destruct addr; simpl in H; try discriminate.
+  eapply store_sound; eauto. apply match_aptr_of_aval; auto.
+Qed.
+
+Theorem loadbytes_sound:
+  forall m b ofs sz bytes am rm p,
+  Mem.loadbytes m b (Ptrofs.unsigned ofs) sz = Some bytes ->
+  romatch m rm ->
+  mmatch m am ->
+  pmatch b ofs p ->
+  forall  b' ofs' q i, In (Fragment (Vptr b' ofs') q i) bytes -> pmatch b' ofs' (loadbytes am rm p).
+Proof.
+  intros. unfold loadbytes; inv H2.
+- (* Gl id ofs *)
+  destruct (rm!id) as [ab|] eqn:RM.
+  exploit H0; eauto. intros (A & B & C). eapply ablock_loadbytes_sound; eauto.
+  destruct (am_glob am)!id as [ab|] eqn:GL.
+  eapply ablock_loadbytes_sound; eauto. eapply mmatch_glob; eauto.
+  eapply smatch_loadbytes; eauto. eapply mmatch_nonstack; eauto with va.
+- (* Glo id *)
+  destruct (rm!id) as [ab|] eqn:RM.
+  exploit H0; eauto. intros (A & B & C). eapply ablock_loadbytes_sound; eauto.
+  destruct (am_glob am)!id as [ab|] eqn:GL.
+  eapply ablock_loadbytes_sound; eauto. eapply mmatch_glob; eauto.
+  eapply smatch_loadbytes; eauto. eapply mmatch_nonstack; eauto with va.
+- (* Glob *)
+  eapply smatch_loadbytes; eauto. eapply mmatch_nonstack; eauto with va.
+- (* Stk ofs *)
+  eapply ablock_loadbytes_sound; eauto. eapply mmatch_stack; eauto.
+- (* Stack *)
+  eapply ablock_loadbytes_sound; eauto. eapply mmatch_stack; eauto.
+- (* Nonstack *)
+  eapply smatch_loadbytes; eauto. eapply mmatch_nonstack; eauto with va.
+- (* Top *)
+  eapply smatch_loadbytes; eauto. eapply mmatch_top; eauto with va.
+Qed.
+
+Theorem storebytes_sound:
+  forall m b ofs bytes m' am p sz q,
+  Mem.storebytes m b (Ptrofs.unsigned ofs) bytes = Some m' ->
+  mmatch m am ->
+  pmatch b ofs p ->
+  length bytes = Z.to_nat sz ->
+  (forall b' ofs' qt i, In (Fragment (Vptr b' ofs') qt i) bytes -> pmatch b' ofs' q) ->
+  mmatch m' (storebytes am p sz q).
+Proof.
+  intros until q; intros STORE MM PM LENGTH BYTES.
+  unfold storebytes; constructor; simpl; intros.
+- (* Stack *)
+  assert (DFL: bc b <> BCstack -> bmatch m' b0 (am_stack am)).
+  { intros. apply bmatch_inv with m. eapply mmatch_stack; eauto.
+    intros. eapply Mem.loadbytes_storebytes_other; eauto. left; congruence. }
+  inv PM; try (apply DFL; congruence).
+  + assert (b0 = b) by (eapply bc_stack; eauto). subst b0.
+    eapply ablock_storebytes_sound; eauto. eapply mmatch_stack; eauto.
+  + assert (b0 = b) by (eapply bc_stack; eauto). subst b0.
+    eapply ablock_storebytes_anywhere_sound; eauto. eapply mmatch_stack; eauto.
+  + eapply ablock_storebytes_anywhere_sound; eauto. eapply mmatch_stack; eauto.
+
+- (* Globals *)
+  rename b0 into b'.
+  assert (DFL: bc b <> BCglob id -> (am_glob am)!id = Some ab ->
+               bmatch m' b' ab).
+  { intros. apply bmatch_inv with m. eapply mmatch_glob; eauto.
+    intros. eapply Mem.loadbytes_storebytes_other; eauto. left; congruence. }
+  inv PM.
+  + rewrite PTree.gsspec in H0. destruct (peq id id0).
+    subst id0; inv H0.
+    assert (b' = b) by (eapply bc_glob; eauto). subst b'.
+    eapply ablock_storebytes_sound; eauto.
+    destruct (am_glob am)!id as [ab0|] eqn:GL.
+    eapply mmatch_glob; eauto.
+    apply ablock_init_sound. eapply mmatch_nonstack; eauto; congruence.
+    eapply DFL; eauto. congruence.
+  + rewrite PTree.gsspec in H0. destruct (peq id id0).
+    subst id0; inv H0.
+    assert (b' = b) by (eapply bc_glob; eauto). subst b'.
+    eapply ablock_storebytes_anywhere_sound; eauto.
+    destruct (am_glob am)!id as [ab0|] eqn:GL.
+    eapply mmatch_glob; eauto.
+    apply ablock_init_sound. eapply mmatch_nonstack; eauto; congruence.
+    eapply DFL; eauto. congruence.
+  + rewrite PTree.gempty in H0; congruence.
+  + eapply DFL; eauto. congruence.
+  + eapply DFL; eauto. congruence.
+  + rewrite PTree.gempty in H0; congruence.
+  + rewrite PTree.gempty in H0; congruence.
+
+- (* Nonstack *)
+  assert (DFL: smatch m' b0 (plub q (am_nonstack am))).
+  { eapply smatch_storebytes; eauto. eapply mmatch_nonstack; eauto. }
+  assert (STK: bc b = BCstack -> smatch m' b0 (am_nonstack am)).
+  { intros. apply smatch_inv with m. eapply mmatch_nonstack; eauto; congruence.
+    intros. eapply Mem.loadbytes_storebytes_other; eauto. left. congruence.
+  }
+  inv PM; (apply DFL || apply STK; congruence).
+
+- (* Top *)
+  eapply smatch_storebytes; eauto. eapply mmatch_top; eauto.
+
+- (* Below *)
+  erewrite Mem.nextblock_storebytes by eauto. eapply mmatch_below; eauto.
+Qed.
+
+Lemma mmatch_ext:
+  forall m am m',
+  mmatch m am ->
+  (forall b ofs n bytes, bc b <> BCinvalid -> n >= 0 -> Mem.loadbytes m' b ofs n = Some bytes -> Mem.loadbytes m b ofs n = Some bytes) ->
+  Ple (Mem.nextblock m) (Mem.nextblock m') ->
+  mmatch m' am.
+Proof.
+  intros. inv H. constructor; intros.
+- apply bmatch_ext with m; auto with va.
+- apply bmatch_ext with m; eauto with va.
+- apply smatch_ext with m; auto with va.
+- apply smatch_ext with m; auto with va.
+- red; intros. exploit mmatch_below0; eauto. xomega.
+Qed.
+
+Lemma mmatch_free:
+  forall m b lo hi m' am,
+  Mem.free m b lo hi = Some m' ->
+  mmatch m am ->
+  mmatch m' am.
+Proof.
+  intros. apply mmatch_ext with m; auto.
+  intros. eapply Mem.loadbytes_free_2; eauto.
+  erewrite <- Mem.nextblock_free by eauto. xomega.
+Qed.
+
+Lemma mmatch_top':
+  forall m am, mmatch m am -> mmatch m mtop.
+Proof.
+  intros. constructor; simpl; intros.
+- apply ablock_init_sound. apply smatch_ge with (ab_summary (am_stack am)).
+  eapply mmatch_stack; eauto. constructor.
+- rewrite PTree.gempty in H1; discriminate.
+- eapply smatch_ge. eapply mmatch_nonstack; eauto. constructor.
+- eapply smatch_ge. eapply mmatch_top; eauto. constructor.
+- eapply mmatch_below; eauto.
+Qed.
+
+(** Boolean equality *)
+
+Definition mbeq (m1 m2: amem) : bool :=
+  eq_aptr m1.(am_top) m2.(am_top)
+  && eq_aptr m1.(am_nonstack) m2.(am_nonstack)
+  && bbeq m1.(am_stack) m2.(am_stack)
+  && PTree.beq bbeq m1.(am_glob) m2.(am_glob).
+
+Lemma mbeq_sound:
+  forall m1 m2, mbeq m1 m2 = true -> forall m, mmatch m m1 <-> mmatch m m2.
+Proof.
+  unfold mbeq; intros. InvBooleans. rewrite PTree.beq_correct in H1.
+  split; intros M; inv M; constructor; intros.
+- erewrite <- bbeq_sound; eauto.
+- specialize (H1 id). rewrite H4 in H1. destruct (am_glob m1)!id eqn:G; try contradiction.
+  erewrite <- bbeq_sound; eauto.
+- rewrite <- H; eauto.
+- rewrite <- H0; eauto.
+- auto.
+- erewrite bbeq_sound; eauto.
+- specialize (H1 id). rewrite H4 in H1. destruct (am_glob m2)!id eqn:G; try contradiction.
+  erewrite bbeq_sound; eauto.
+- rewrite H; eauto.
+- rewrite H0; eauto.
+- auto.
+Qed.
+
+(** Least upper bound *)
+
+Definition combine_ablock (ob1 ob2: option ablock) : option ablock :=
+  match ob1, ob2 with
+  | Some b1, Some b2 => Some (blub b1 b2)
+  | _, _ => None
+  end.
+
+Definition mlub (m1 m2: amem) : amem :=
+{| am_stack := blub m1.(am_stack) m2.(am_stack);
+   am_glob  := PTree.combine combine_ablock m1.(am_glob) m2.(am_glob);
+   am_nonstack := plub m1.(am_nonstack) m2.(am_nonstack);
+   am_top := plub m1.(am_top) m2.(am_top) |}.
+
+Lemma mmatch_lub_l:
+  forall m x y, mmatch m x -> mmatch m (mlub x y).
+Proof.
+  intros. inv H. constructor; simpl; intros.
+- apply bmatch_lub_l; auto.
+- rewrite PTree.gcombine in H0 by auto. unfold combine_ablock in H0.
+  destruct (am_glob x)!id as [b1|] eqn:G1;
+  destruct (am_glob y)!id as [b2|] eqn:G2;
+  inv H0.
+  apply bmatch_lub_l; eauto.
+- apply smatch_lub_l; auto.
+- apply smatch_lub_l; auto.
+- auto.
+Qed.
+
+Lemma mmatch_lub_r:
+  forall m x y, mmatch m y -> mmatch m (mlub x y).
+Proof.
+  intros. inv H. constructor; simpl; intros.
+- apply bmatch_lub_r; auto.
+- rewrite PTree.gcombine in H0 by auto. unfold combine_ablock in H0.
+  destruct (am_glob x)!id as [b1|] eqn:G1;
+  destruct (am_glob y)!id as [b2|] eqn:G2;
+  inv H0.
+  apply bmatch_lub_r; eauto.
+- apply smatch_lub_r; auto.
+- apply smatch_lub_r; auto.
+- auto.
 Qed.
 
 End MATCH.
+
+(** * Monotonicity properties when the block classification changes. *)
+
+Lemma genv_match_exten:
+  forall ge (bc1 bc2: block_classification),
+  genv_match bc1 ge ->
+  (forall b id, bc1 b = BCglob id <-> bc2 b = BCglob id) ->
+  (forall b, bc1 b = BCother -> bc2 b = BCother) ->
+  genv_match bc2 ge.
+Proof.
+  intros. destruct H as [A B]. split; intros.
+- rewrite <- H0. eauto.
+- exploit B; eauto. destruct (bc1 b) eqn:BC1.
+  + intuition congruence.
+  + rewrite H0 in BC1. intuition congruence.
+  + intuition congruence.
+  + erewrite H1 by eauto. intuition congruence.
+Qed.
+
+Lemma romatch_exten:
+  forall (bc1 bc2: block_classification) m rm,
+  romatch bc1 m rm ->
+  (forall b id, bc2 b = BCglob id <-> bc1 b = BCglob id) ->
+  romatch bc2 m rm.
+Proof.
+  intros; red; intros. rewrite H0 in H1. exploit H; eauto. intros (A & B & C).
+  split; auto. split; auto.
+  assert (PM: forall b ofs p, pmatch bc1 b ofs p -> pmatch bc1 b ofs (ab_summary ab) -> pmatch bc2 b ofs p).
+  {
+    intros.
+    assert (pmatch bc1 b0 ofs Glob) by (eapply pmatch_ge; eauto).
+    inv H5.
+    assert (bc2 b0 = BCglob id0) by (rewrite H0; auto).
+    inv H3; econstructor; eauto with va.
+  }
+  assert (VM: forall v x, vmatch bc1 v x -> vmatch bc1 v (Ifptr (ab_summary ab)) -> vmatch bc2 v x).
+  {
+    intros. inv H3; constructor; auto; inv H4; eapply PM; eauto.
+  }
+  destruct B as [[B1 B2] B3]. split. split.
+- intros. apply VM; eauto.
+- intros. apply PM; eauto.
+- intros. apply VM; eauto.
+Qed.
+
+Definition bc_incr (bc1 bc2: block_classification) : Prop :=
+  forall b, bc1 b <> BCinvalid -> bc2 b = bc1 b.
+
+Section MATCH_INCR.
+
+Variables bc1 bc2: block_classification.
+Hypothesis INCR: bc_incr bc1 bc2.
+
+Lemma pmatch_incr: forall b ofs p, pmatch bc1 b ofs p -> pmatch bc2 b ofs p.
+Proof.
+  induction 1;
+  assert (bc2 b = bc1 b) by (apply INCR; congruence);
+  econstructor; eauto with va. rewrite H0; eauto.
+Qed.
+
+Lemma vmatch_incr: forall v x, vmatch bc1 v x -> vmatch bc2 v x.
+Proof.
+  induction 1; constructor; auto; apply pmatch_incr; auto.
+Qed.
+
+Lemma smatch_incr: forall m b p, smatch bc1 m b p -> smatch bc2 m b p.
+Proof.
+  intros. destruct H as [A B]. split; intros.
+  apply vmatch_incr; eauto.
+  apply pmatch_incr; eauto.
+Qed.
+
+Lemma bmatch_incr: forall m b ab, bmatch bc1 m b ab -> bmatch bc2 m b ab.
+Proof.
+  intros. destruct H as [B1 B2]. split.
+  apply smatch_incr; auto.
+  intros. apply vmatch_incr; eauto.
+Qed.
+
+End MATCH_INCR.
+
+(** * Matching and memory injections. *)
+
+Definition inj_of_bc (bc: block_classification) : meminj :=
+  fun b => match bc b with BCinvalid => None | _ => Some(b, 0) end.
+
+Lemma inj_of_bc_valid:
+  forall (bc: block_classification) b, bc b <> BCinvalid -> inj_of_bc bc b = Some(b, 0).
+Proof.
+  intros. unfold inj_of_bc. destruct (bc b); congruence.
+Qed.
+
+Lemma inj_of_bc_inv:
+  forall (bc: block_classification) b b' delta,
+  inj_of_bc bc b = Some(b', delta) -> bc b <> BCinvalid /\ b' = b /\ delta = 0.
+Proof.
+  unfold inj_of_bc; intros. destruct (bc b); intuition congruence.
+Qed.
+
+Lemma pmatch_inj:
+  forall bc b ofs p, pmatch bc b ofs p -> inj_of_bc bc b = Some(b, 0).
+Proof.
+  intros. apply inj_of_bc_valid. inv H; congruence.
+Qed.
+
+Lemma vmatch_inj:
+  forall bc v x, vmatch bc v x -> Val.inject (inj_of_bc bc) v v.
+Proof.
+  induction 1; econstructor.
+  eapply pmatch_inj; eauto. rewrite Ptrofs.add_zero; auto.
+  eapply pmatch_inj; eauto. rewrite Ptrofs.add_zero; auto.
+Qed.
+
+Lemma vmatch_list_inj:
+  forall bc vl xl, list_forall2 (vmatch bc) vl xl -> Val.inject_list (inj_of_bc bc) vl vl.
+Proof.
+  induction 1; constructor. eapply vmatch_inj; eauto. auto.
+Qed.
+
+Lemma mmatch_inj:
+  forall bc m am, mmatch bc m am -> bc_below bc (Mem.nextblock m) -> Mem.inject (inj_of_bc bc) m m.
+Proof.
+  intros. constructor. constructor.
+- (* perms *)
+  intros. exploit inj_of_bc_inv; eauto. intros (A & B & C); subst.
+  rewrite Z.add_0_r. auto.
+- (* alignment *)
+  intros. exploit inj_of_bc_inv; eauto. intros (A & B & C); subst.
+  apply Z.divide_0_r.
+- (* contents *)
+  intros. exploit inj_of_bc_inv; eauto. intros (A & B & C); subst.
+  rewrite Z.add_0_r.
+  set (mv := ZMap.get ofs (PMap.get b1 (Mem.mem_contents m))).
+  assert (Mem.loadbytes m b1 ofs 1 = Some (mv :: nil)).
+  {
+    Local Transparent Mem.loadbytes.
+    unfold Mem.loadbytes. rewrite pred_dec_true. reflexivity.
+    red; intros. replace ofs0 with ofs by omega. auto.
+  }
+  destruct mv; econstructor. destruct v; econstructor.
+  apply inj_of_bc_valid.
+  assert (PM: pmatch bc b i Ptop).
+  { exploit mmatch_top; eauto. intros [P Q].
+    eapply pmatch_top'. eapply Q; eauto. }
+  inv PM; auto.
+  rewrite Ptrofs.add_zero; auto.
+- (* free blocks *)
+  intros. unfold inj_of_bc. erewrite bc_below_invalid; eauto.
+- (* mapped blocks *)
+  intros. exploit inj_of_bc_inv; eauto. intros (A & B & C); subst.
+  apply H0; auto.
+- (* overlap *)
+  red; intros.
+  exploit inj_of_bc_inv. eexact H2. intros (A1 & B & C); subst.
+  exploit inj_of_bc_inv. eexact H3. intros (A2 & B & C); subst.
+  auto.
+- (* overflow *)
+  intros. exploit inj_of_bc_inv; eauto. intros (A & B & C); subst.
+  rewrite Z.add_0_r. split. omega. apply Ptrofs.unsigned_range_2.
+- (* perm inv *)
+  intros. exploit inj_of_bc_inv; eauto. intros (A & B & C); subst.
+  rewrite Z.add_0_r in H2. auto.
+Qed.
+
+Lemma inj_of_bc_preserves_globals:
+  forall bc ge, genv_match bc ge -> meminj_preserves_globals ge (inj_of_bc bc).
+Proof.
+  intros. destruct H as [A B].
+  split. intros. apply inj_of_bc_valid. rewrite A in H. congruence.
+  split. intros. apply inj_of_bc_valid. apply B.
+    rewrite Genv.find_var_info_iff in H. eapply Genv.genv_defs_range; eauto.
+  intros. exploit inj_of_bc_inv; eauto. intros (P & Q & R). auto.
+Qed.
+
+Lemma pmatch_inj_top:
+  forall bc b b' delta ofs, inj_of_bc bc b = Some(b', delta) -> pmatch bc b ofs Ptop.
+Proof.
+  intros. exploit inj_of_bc_inv; eauto. intros (A & B & C). constructor; auto.
+Qed.
+
+Lemma vmatch_inj_top:
+  forall bc v v', Val.inject (inj_of_bc bc) v v' -> vmatch bc v Vtop.
+Proof.
+  intros. inv H; constructor. eapply pmatch_inj_top; eauto.
+Qed.
+
+Lemma mmatch_inj_top:
+  forall bc m m', Mem.inject (inj_of_bc bc) m m' -> mmatch bc m mtop.
+Proof.
+  intros.
+  assert (SM: forall b, bc b <> BCinvalid -> smatch bc m b Ptop).
+  {
+    intros; split; intros.
+    - exploit Mem.load_inject. eauto. eauto. apply inj_of_bc_valid; auto.
+      intros (v' & A & B). eapply vmatch_inj_top; eauto.
+    - exploit Mem.loadbytes_inject. eauto. eauto. apply inj_of_bc_valid; auto.
+      intros (bytes' & A & B). inv B. inv H4. inv H8. eapply pmatch_inj_top; eauto.
+  }
+  constructor; simpl; intros.
+  - apply ablock_init_sound. apply SM. congruence.
+  - rewrite PTree.gempty in H1; discriminate.
+  - apply SM; auto.
+  - apply SM; auto.
+  - red; intros. eapply Mem.valid_block_inject_1. eapply inj_of_bc_valid; eauto. eauto.
+Qed.
+
+(** * Abstracting RTL register environments *)
 
 Module AVal <: SEMILATTICE_WITH_TOP.
 
@@ -2199,9 +4518,203 @@ Module AVal <: SEMILATTICE_WITH_TOP.
   Proof vge_lub_r.
 End AVal.
 
-Hint Constructors ValueDomain.cmatch : va.
+Module AE := LPMap(AVal).
+
+Definition aenv := AE.t.
+
+Section MATCHENV.
+
+Variable bc: block_classification.
+
+Definition ematch (e: regset) (ae: aenv) : Prop :=
+  forall r, vmatch bc e#r (AE.get r ae).
+
+Lemma ematch_ge:
+  forall e ae1 ae2,
+  ematch e ae1 -> AE.ge ae2 ae1 -> ematch e ae2.
+Proof.
+  intros; red; intros. apply vmatch_ge with (AE.get r ae1); auto. apply H0.
+Qed.
+
+Lemma ematch_update:
+  forall e ae v av r,
+  ematch e ae -> vmatch bc v av -> ematch (e#r <- v) (AE.set r av ae).
+Proof.
+  intros; red; intros. rewrite AE.gsspec. rewrite PMap.gsspec.
+  destruct (peq r0 r); auto.
+  red; intros. specialize (H xH). subst ae. simpl in H. inv H.
+  unfold AVal.eq; red; intros. subst av. inv H0.
+Qed.
+
+Fixpoint einit_regs (rl: list reg) : aenv :=
+  match rl with
+  | r1 :: rs => AE.set r1 (Ifptr Nonstack) (einit_regs rs)
+  | nil => AE.top
+  end.
+
+Lemma ematch_init:
+  forall rl vl,
+  (forall v, In v vl -> vmatch bc v (Ifptr Nonstack)) ->
+  ematch (init_regs vl rl) (einit_regs rl).
+Proof.
+  induction rl; simpl; intros.
+- red; intros. rewrite Regmap.gi. simpl AE.get. rewrite PTree.gempty.
+  constructor.
+- destruct vl as [ | v1 vs ].
+  + assert (ematch (init_regs nil rl) (einit_regs rl)).
+    { apply IHrl. simpl; tauto. }
+    replace (init_regs nil rl) with (Regmap.init Vundef) in H0 by (destruct rl; auto).
+    red; intros. rewrite AE.gsspec. destruct (peq r a).
+    rewrite Regmap.gi. constructor.
+    apply H0.
+    red; intros EQ; rewrite EQ in H0. specialize (H0 xH). simpl in H0. inv H0.
+    unfold AVal.eq, AVal.bot. congruence.
+  + assert (ematch (init_regs vs rl) (einit_regs rl)).
+    { apply IHrl. eauto with coqlib. }
+    red; intros. rewrite Regmap.gsspec. rewrite AE.gsspec. destruct (peq r a).
+    auto with coqlib.
+    apply H0.
+    red; intros EQ; rewrite EQ in H0. specialize (H0 xH). simpl in H0. inv H0.
+    unfold AVal.eq, AVal.bot. congruence.
+Qed.
+
+Fixpoint eforget (rl: list reg) (ae: aenv) {struct rl} : aenv :=
+  match rl with
+  | nil => ae
+  | r1 :: rs => eforget rs (AE.set r1 Vtop ae)
+  end.
+
+Lemma eforget_ge:
+  forall rl ae, AE.ge (eforget rl ae) ae.
+Proof.
+  unfold AE.ge; intros. revert rl ae; induction rl; intros; simpl.
+  apply AVal.ge_refl. apply AVal.eq_refl.
+  destruct ae. unfold AE.get at 2. apply AVal.ge_bot.
+  eapply AVal.ge_trans. apply IHrl. rewrite AE.gsspec.
+  destruct (peq p a). apply AVal.ge_top. apply AVal.ge_refl. apply AVal.eq_refl.
+  congruence.
+  unfold AVal.eq, Vtop, AVal.bot. congruence.
+Qed.
+
+Lemma ematch_forget:
+  forall e rl ae, ematch e ae -> ematch e (eforget rl ae).
+Proof.
+  intros. eapply ematch_ge; eauto. apply eforget_ge.
+Qed.
+
+End MATCHENV.
+
+Lemma ematch_incr:
+  forall bc bc' e ae, ematch bc e ae -> bc_incr bc bc' -> ematch bc' e ae.
+Proof.
+  intros; red; intros. apply vmatch_incr with bc; auto.
+Qed.
+
+(** * Lattice for dataflow analysis *)
+
+Module VA <: SEMILATTICE.
+
+  Inductive t' := Bot | State (ae: aenv) (am: amem).
+  Definition t := t'.
+
+  Definition eq (x y: t) :=
+    match x, y with
+    | Bot, Bot => True
+    | State ae1 am1, State ae2 am2 =>
+        AE.eq ae1 ae2 /\ forall bc m, mmatch bc m am1 <-> mmatch bc m am2
+    | _, _ => False
+    end.
+
+  Lemma eq_refl: forall x, eq x x.
+  Proof.
+    destruct x; simpl. auto. split. apply AE.eq_refl. tauto.
+  Qed.
+  Lemma eq_sym: forall x y, eq x y -> eq y x.
+  Proof.
+    destruct x, y; simpl; auto. intros [A B].
+    split. apply AE.eq_sym; auto. intros. rewrite B. tauto.
+  Qed.
+  Lemma eq_trans: forall x y z, eq x y -> eq y z -> eq x z.
+  Proof.
+    destruct x, y, z; simpl; try tauto. intros [A B] [C D]; split.
+    eapply AE.eq_trans; eauto.
+    intros. rewrite B; auto.
+  Qed.
+
+  Definition beq (x y: t) : bool :=
+    match x, y with
+    | Bot, Bot => true
+    | State ae1 am1, State ae2 am2 => AE.beq ae1 ae2 && mbeq am1 am2
+    | _, _ => false
+    end.
+
+  Lemma beq_correct: forall x y, beq x y = true -> eq x y.
+  Proof.
+    destruct x, y; simpl; intros.
+    auto.
+    congruence.
+    congruence.
+    InvBooleans; split.
+    apply AE.beq_correct; auto.
+    intros. apply mbeq_sound; auto.
+  Qed.
+
+  Definition ge (x y: t) : Prop :=
+    match x, y with
+    | _, Bot => True
+    | Bot, _ => False
+    | State ae1 am1, State ae2 am2 => AE.ge ae1 ae2 /\ forall bc m, mmatch bc m am2 -> mmatch bc m am1
+    end.
+
+  Lemma ge_refl: forall x y, eq x y -> ge x y.
+  Proof.
+    destruct x, y; simpl; try tauto. intros [A B]; split.
+    apply AE.ge_refl; auto.
+    intros. rewrite B; auto.
+  Qed.
+  Lemma ge_trans: forall x y z, ge x y -> ge y z -> ge x z.
+  Proof.
+    destruct x, y, z; simpl; try tauto. intros [A B] [C D]; split.
+    eapply AE.ge_trans; eauto.
+    eauto.
+  Qed.
+
+  Definition bot : t := Bot.
+  Lemma ge_bot: forall x, ge x bot.
+  Proof.
+    destruct x; simpl; auto.
+  Qed.
+
+  Definition lub (x y: t) : t :=
+    match x, y with
+    | Bot, _ => y
+    | _, Bot => x
+    | State ae1 am1, State ae2 am2 => State (AE.lub ae1 ae2) (mlub am1 am2)
+    end.
+
+  Lemma ge_lub_left: forall x y, ge (lub x y) x.
+  Proof.
+    destruct x, y.
+    apply ge_refl; apply eq_refl.
+    simpl. auto.
+    apply ge_refl; apply eq_refl.
+    simpl. split. apply AE.ge_lub_left. intros; apply mmatch_lub_l; auto.
+  Qed.
+  Lemma ge_lub_right: forall x y, ge (lub x y) y.
+  Proof.
+    destruct x, y.
+    apply ge_refl; apply eq_refl.
+    apply ge_refl; apply eq_refl.
+    simpl. auto.
+    simpl. split. apply AE.ge_lub_right. intros; apply mmatch_lub_r; auto.
+  Qed.
+
+End VA.
+
+Hint Constructors cmatch : va.
+Hint Constructors pmatch: va.
 Hint Constructors vmatch: va.
-Hint Resolve 
+Hint Resolve cnot_sound symbol_address_sound
        shl_sound shru_sound shr_sound
        and_sound or_sound xor_sound notint_sound
        ror_sound rolm_sound
@@ -2213,11 +4726,13 @@ Hint Resolve
        negl_sound addl_sound subl_sound
        mull_sound mullhs_sound mullhu_sound
        divls_sound divlu_sound modls_sound modlu_sound shrxl_sound
+       offset_ptr_sound
        negf_sound absf_sound
        addf_sound subf_sound mulf_sound divf_sound
        negfs_sound absfs_sound
        addfs_sound subfs_sound mulfs_sound divfs_sound
        zero_ext_sound sign_ext_sound longofint_sound longofintu_sound
+       zero_ext_l_sound sign_ext_l_sound
        singleoffloat_sound floatofsingle_sound
        intoffloat_sound intuoffloat_sound floatofint_sound floatofintu_sound
        intofsingle_sound intuofsingle_sound singleofint_sound singleofintu_sound
