riscV/ValueAOpSSA.v
@@ -12,10 +12,9 @@
 
 Require Import Coqlib Compopts.
 Require Import AST Integers Floats Values Memory Globalenvs.
-Require Import Op SSA  ValueDomain ValueDomainSSA.
+Require Import Op SSA ValueDomainSSA.
 
-
-(** Value analysis for x86_64 operators *)
+(** Value analysis for RISC V operators *)
 
 Definition eval_static_condition (cond: condition) (vl: list aval): abool :=
   match cond, vl with
@@ -31,58 +30,33 @@ Definition eval_static_condition (cond: condition) (vl: list aval): abool :=
   | Cnotcompf c, v1 :: v2 :: nil => cnot (cmpf_bool c v1 v2)
   | Ccompfs c, v1 :: v2 :: nil => cmpfs_bool c v1 v2
   | Cnotcompfs c, v1 :: v2 :: nil => cnot (cmpfs_bool c v1 v2)
-  | Cmaskzero n, v1 :: nil => maskzero v1 n
-  | Cmasknotzero n, v1 :: nil => cnot (maskzero v1 n)
   | _, _ => Bnone
   end.
 
-Definition eval_static_addressing_32 (addr: addressing) (vl: list aval): aval :=
-  match addr, vl with
-  | Aindexed n, v1::nil => add v1 (I (Int.repr n))
-  | Aindexed2 n, v1::v2::nil => add (add v1 v2) (I (Int.repr n))
-  | Ascaled sc ofs, v1::nil => add (mul v1 (I (Int.repr sc))) (I (Int.repr ofs))
-  | Aindexed2scaled sc ofs, v1::v2::nil => add v1 (add (mul v2 (I (Int.repr sc))) (I (Int.repr ofs)))
-  | Aglobal _ _, nil => Vtop
-  | Abased _ _, _::nil => Vtop
-  | Abasedscaled _ _ _, _::nil => Vtop
-  | Ainstack _, nil => Vtop
-  | _, _ => Vbot
-  end.
-
-Definition eval_static_addressing_64 (addr: addressing) (vl: list aval): aval :=
-  match addr, vl with
-  | Aindexed n, v1::nil => addl v1 (L (Int64.repr n))
-  | Aindexed2 n, v1::v2::nil => addl (addl v1 v2) (L (Int64.repr n))
-  | Ascaled sc ofs, v1::nil => addl (mull v1 (L (Int64.repr sc))) (L (Int64.repr ofs))
-  | Aindexed2scaled sc ofs, v1::v2::nil => addl v1 (addl (mull v2 (L (Int64.repr sc))) (L (Int64.repr ofs)))
-  | Aglobal _ _, nil => Vtop
-  | Abased _ _, _::nil => Vtop
-  | Abasedscaled _ _ _, _::nil => Vtop
-  | Ainstack _, nil => Vtop
-  | _, _ => Vbot
-  end.
-
 Definition eval_static_addressing (addr: addressing) (vl: list aval): aval :=
-  if Archi.ptr64
-  then eval_static_addressing_64 addr vl
-  else eval_static_addressing_32 addr vl.
+  match addr, vl with
+  | Aindexed n, v1::nil => offset_ptr v1 n
+  | Aglobal s ofs, nil => Ptr (Gl s ofs)
+  | Ainstack ofs, nil => Vtop
+  | _, _ => Vbot
+  end.
 
 Definition eval_static_operation (op: operation) (vl: list aval): aval :=
   match op, vl with
   | Omove, v1::nil => v1
   | Ointconst n, nil => I n
   | Olongconst n, nil => L n
-  | Ofloatconst n, nil => if propagate_float_constants tt then F n else Vtop
-  | Osingleconst n, nil => if propagate_float_constants tt then FS n else Vtop
-  | Oindirectsymbol id, nil => Vtop
+  | Ofloatconst n, nil => if propagate_float_constants tt then F n else ntop
+  | Osingleconst n, nil => if propagate_float_constants tt then FS n else ntop
+  | Oaddrsymbol id ofs, nil => Ptr (Gl id ofs)
+  | Oaddrstack ofs, nil => Vtop
   | Ocast8signed, v1 :: nil => sign_ext 8 v1
-  | Ocast8unsigned, v1 :: nil => zero_ext 8 v1
   | Ocast16signed, v1 :: nil => sign_ext 16 v1
-  | Ocast16unsigned, v1 :: nil => zero_ext 16 v1
+  | Oadd, v1::v2::nil => add v1 v2
+  | Oaddimm n, v1::nil => add v1 (I n)
   | Oneg, v1::nil => neg v1
   | Osub, v1::v2::nil => sub v1 v2
   | Omul, v1::v2::nil => mul v1 v2
-  | Omulimm n, v1::nil => mul v1 (I n)
   | Omulhs, v1::v2::nil => mulhs v1 v2
   | Omulhu, v1::v2::nil => mulhu v1 v2
   | Odiv, v1::v2::nil => divs v1 v2
@@ -95,27 +69,23 @@ Definition eval_static_operation (op: operation) (vl: list aval): aval :=
   | Oorimm n, v1::nil => or v1 (I n)
   | Oxor, v1::v2::nil => xor v1 v2
   | Oxorimm n, v1::nil => xor v1 (I n)
-  | Onot, v1::nil => notint v1
   | Oshl, v1::v2::nil => shl v1 v2
   | Oshlimm n, v1::nil => shl v1 (I n)
   | Oshr, v1::v2::nil => shr v1 v2
   | Oshrimm n, v1::nil => shr v1 (I n)
-  | Oshrximm n, v1::nil => shrx v1 (I n)
   | Oshru, v1::v2::nil => shru v1 v2
   | Oshruimm n, v1::nil => shru v1 (I n)
-  | Ororimm n, v1::nil => ror v1 (I n)
-  | Oshldimm n, v1::v2::nil => or (shl v1 (I n)) (shru v2 (I (Int.sub Int.iwordsize n)))
-  | Olea addr, _ => eval_static_addressing_32 addr vl
+  | Oshrximm n, v1::nil => shrx v1 (I n)
   | Omakelong, v1::v2::nil => longofwords v1 v2
   | Olowlong, v1::nil => loword v1
   | Ohighlong, v1::nil => hiword v1
   | Ocast32signed, v1::nil => longofint v1
   | Ocast32unsigned, v1::nil => longofintu v1
-  | Onegl, v1::nil => negl v1
+  | Oaddl, v1::v2::nil => addl v1 v2
   | Oaddlimm n, v1::nil => addl v1 (L n)
+  | Onegl, v1::nil => negl v1
   | Osubl, v1::v2::nil => subl v1 v2
   | Omull, v1::v2::nil => mull v1 v2
-  | Omullimm n, v1::nil => mull v1 (L n)
   | Omullhs, v1::v2::nil => mullhs v1 v2
   | Omullhu, v1::v2::nil => mullhu v1 v2
   | Odivl, v1::v2::nil => divls v1 v2
@@ -128,16 +98,13 @@ Definition eval_static_operation (op: operation) (vl: list aval): aval :=
   | Oorlimm n, v1::nil => orl v1 (L n)
   | Oxorl, v1::v2::nil => xorl v1 v2
   | Oxorlimm n, v1::nil => xorl v1 (L n)
-  | Onotl, v1::nil => notl v1
   | Oshll, v1::v2::nil => shll v1 v2
   | Oshllimm n, v1::nil => shll v1 (I n)
   | Oshrl, v1::v2::nil => shrl v1 v2
   | Oshrlimm n, v1::nil => shrl v1 (I n)
-  | Oshrxlimm n, v1::nil => shrxl v1 (I n)
   | Oshrlu, v1::v2::nil => shrlu v1 v2
   | Oshrluimm n, v1::nil => shrlu v1 (I n)
-  | Ororlimm n, v1::nil => rorl v1 (I n)
-  | Oleal addr, _ => eval_static_addressing_64 addr vl
+  | Oshrxlimm n, v1::nil => shrxl v1 (I n)
   | Onegf, v1::nil => negf v1
   | Oabsf, v1::nil => absf v1
   | Oaddf, v1::v2::nil => addf v1 v2
@@ -153,23 +120,36 @@ Definition eval_static_operation (op: operation) (vl: list aval): aval :=
   | Osingleoffloat, v1::nil => singleoffloat v1
   | Ofloatofsingle, v1::nil => floatofsingle v1
   | Ointoffloat, v1::nil => intoffloat v1
+  | Ointuoffloat, v1::nil => intuoffloat v1
   | Ofloatofint, v1::nil => floatofint v1
+  | Ofloatofintu, v1::nil => floatofintu v1
   | Ointofsingle, v1::nil => intofsingle v1
+  | Ointuofsingle, v1::nil => intuofsingle v1
   | Osingleofint, v1::nil => singleofint v1
+  | Osingleofintu, v1::nil => singleofintu v1
   | Olongoffloat, v1::nil => longoffloat v1
+  | Olonguoffloat, v1::nil => longuoffloat v1
   | Ofloatoflong, v1::nil => floatoflong v1
+  | Ofloatoflongu, v1::nil => floatoflongu v1
   | Olongofsingle, v1::nil => longofsingle v1
+  | Olonguofsingle, v1::nil => longuofsingle v1
   | Osingleoflong, v1::nil => singleoflong v1
+  | Osingleoflongu, v1::nil => singleoflongu v1
   | Ocmp c, _ => of_optbool (eval_static_condition c vl)
-  | Osel _ _ , _ => Vtop 
   | _, _ => Vbot
   end.
 
 Section SOUNDNESS.
 
+Variable bc: block_classification.
+Variable ge: genv.
+Hypothesis GENV: genv_match bc ge.
+Variable sp: block.
+Hypothesis STACK: bc sp <> BCinvalid.
+
 Theorem eval_static_condition_sound:
   forall cond vargs m aargs,
-  list_forall2 vmatch vargs aargs ->
+  list_forall2 (vmatch bc) vargs aargs ->
   cmatch (eval_condition cond vargs m) (eval_static_condition cond aargs).
 Proof.
   intros until aargs; intros VM. inv VM.
@@ -181,6 +161,24 @@ Proof.
   destruct cond; auto with va.
 Qed.
 
+Lemma symbol_address_sound:
+  forall id ofs,
+  vmatch bc (Genv.symbol_address ge id ofs) (Ptr (Gl id ofs)).
+Proof.
+  intros; apply symbol_address_sound; apply GENV.
+Qed.
+
+Lemma symbol_address_sound_2:
+  forall id ofs,
+  vmatch bc (Genv.symbol_address ge id ofs) (Ifptr (Gl id ofs)).
+Proof.
+  intros. unfold Genv.symbol_address. destruct (Genv.find_symbol ge id) as [b|] eqn:F.
+  constructor. constructor. apply GENV; auto.
+  constructor.
+Qed.
+
+Hint Resolve symbol_address_sound symbol_address_sound_2: va.
+
 Ltac InvHyps :=
   match goal with
   | [H: None = Some _ |- _ ] => discriminate
@@ -191,49 +189,31 @@ Ltac InvHyps :=
   | _ => idtac
   end.
 
-Theorem eval_static_addressing_32_sound:
-  forall (ge: genv) sp addr vargs vres aargs,
-  eval_addressing32 ge sp addr vargs = Some vres ->
-  list_forall2 vmatch vargs aargs ->
-  vmatch vres (eval_static_addressing_32 addr aargs).
-Proof.
-  unfold eval_addressing32, eval_static_addressing_32; intros;
-  destruct addr; InvHyps; eauto with va.
-Qed.
-
-Theorem eval_static_addressing_64_sound:
-  forall (ge: genv) sp addr vargs vres aargs,
-  eval_addressing64 ge sp addr vargs = Some vres ->
-  list_forall2 vmatch vargs aargs ->
-  vmatch vres (eval_static_addressing_64 addr aargs).
-Proof.
-  unfold eval_addressing64, eval_static_addressing_64; intros;
-  destruct addr; InvHyps; eauto with va.
-Qed.
-
 Theorem eval_static_addressing_sound:
-  forall (ge: genv) sp addr vargs vres aargs,
-  eval_addressing ge sp addr vargs = Some vres ->
-  list_forall2 vmatch vargs aargs ->
-  vmatch vres (eval_static_addressing addr aargs).
+  forall addr vargs vres aargs,
+  eval_addressing ge (Vptr sp Ptrofs.zero) addr vargs = Some vres ->
+  list_forall2 (vmatch bc) vargs aargs ->
+  vmatch bc vres (eval_static_addressing addr aargs).
 Proof.
-  unfold eval_addressing, eval_static_addressing; intros.
-  destruct Archi.ptr64; eauto using eval_static_addressing_32_sound, eval_static_addressing_64_sound.
+  unfold eval_addressing, eval_static_addressing; intros;
+  destruct addr; InvHyps; eauto with va.
+  rewrite Ptrofs.add_zero_l; eauto with va.
+  constructor; constructor; auto.
 Qed.
 
 Theorem eval_static_operation_sound:
-  forall (ge: genv) sp op vargs m vres aargs,
-  eval_operation ge sp op vargs m = Some vres ->
-  list_forall2 vmatch vargs aargs ->
-  vmatch vres (eval_static_operation op aargs).
+  forall op vargs m vres aargs,
+  eval_operation ge (Vptr sp Ptrofs.zero) op vargs m = Some vres ->
+  list_forall2 (vmatch bc) vargs aargs ->
+  vmatch bc vres (eval_static_operation op aargs).
 Proof.
   unfold eval_operation, eval_static_operation; intros;
   destruct op; InvHyps; eauto with va.
   destruct (propagate_float_constants tt); constructor.
   destruct (propagate_float_constants tt); constructor.
-  eapply eval_static_addressing_32_sound; eauto.
-  eapply eval_static_addressing_64_sound; eauto.
-  apply of_optbool_sound. eapply eval_static_condition_sound; eauto.  
+  rewrite Ptrofs.add_zero_l; eauto with va.
+  constructor; constructor; auto.
+  apply of_optbool_sound. eapply eval_static_condition_sound; eauto.
 Qed.
 
 End SOUNDNESS.
